@prefix : <http://ontology.asam.net/ontologies/OpenXOntology.owl#> .
@prefix owl: <http://www.w3.org/2002/07/owl#> .
@prefix rdf: <http://www.w3.org/1999/02/22-rdf-syntax-ns#> .
@prefix xml: <http://www.w3.org/XML/1998/namespace> .
@prefix xsd: <http://www.w3.org/2001/XMLSchema#> .
@prefix rdfs: <http://www.w3.org/2000/01/rdf-schema#> .
@base <http://ontology.asam.net/ontologies/OpenXOntology.owl> .

<http://ontology.asam.net/ontologies/OpenXOntology.owl> rdf:type owl:Ontology ;
                                                         owl:versionIRI <http://ontology.asam.net/ontologies/OpenXOntology.owl/1.0.0> ;
                                                         rdfs:comment "Parent commit (prerelease info only!): 1e655fa506e00981628317cf4f248235f8f38863" ;
                                                         rdfs:label "ASAM OpenXOntology" ;
                                                         owl:versionInfo "Version 1.0.0" ,
                                                                         "license: This ontology is the copyrighted property of ASAM e.V. Any use is limited to the scope described in the license terms (https://www.asam.net/license). In alteration to the regular license terms, ASAM allows unrestricted distribution of this standard. §2 (1) of ASAM’s regular license terms is therefore substituted by the following clause: 'The licensor grants everyone a basic, non-exclusive and unlimited license to use the standard ASAM OpenXOntology.'" .


#################################################################
#    Annotation properties
#################################################################

###  http://swrl.stanford.edu/ontologies/3.3/swrla.owl#isRuleEnabled
<http://swrl.stanford.edu/ontologies/3.3/swrla.owl#isRuleEnabled> rdf:type owl:AnnotationProperty .


#################################################################
#    Object Properties
#################################################################

###  http://ontology.asam.net/ontologies/Core#aggregatedInto
<http://ontology.asam.net/ontologies/Core#aggregatedInto> rdf:type owl:ObjectProperty ,
                                                                   owl:AsymmetricProperty ;
                                                          rdfs:domain <http://ontology.asam.net/ontologies/Core#SpatioTemporalExtent> ;
                                                          rdfs:range <http://ontology.asam.net/ontologies/Core#SpatioTemporalExtent> ;
                                                          rdfs:comment "DEF: A relationship type where a SpatioTemporalExtent may be aggregated into one or more others. This object property has the same meaning as the class Aggregation, but a different representation." ,
                                                                       "HQDM aggregated_into" .


###  http://ontology.asam.net/ontologies/Core#appliesTo
<http://ontology.asam.net/ontologies/Core#appliesTo> rdf:type owl:ObjectProperty ;
                                                     rdfs:comment "DEF: This relation is used to describe that a specification or regularity applies to a particular object. For example, this relation can be used to describe which lanes a speed limit sign applies to." .


###  http://ontology.asam.net/ontologies/Core#approximatelyEqualTo
<http://ontology.asam.net/ontologies/Core#approximatelyEqualTo> rdf:type owl:ObjectProperty ;
                                                                rdfs:subPropertyOf <http://ontology.asam.net/ontologies/Core#hasQuantityRelation> ;
                                                                rdf:type owl:SymmetricProperty ;
                                                                rdfs:domain <http://ontology.asam.net/ontologies/Core#PhysicalQuantity> ;
                                                                rdfs:range <http://ontology.asam.net/ontologies/Core#PhysicalQuantity> ;
                                                                rdfs:comment "DEF: A hasQuantityRelation relationship type, where the value for the second quantity is within the range of the first quantity. The deviation between the values is no greater than +/- 10% of the first value." .


###  http://ontology.asam.net/ontologies/Core#beginningOf
<http://ontology.asam.net/ontologies/Core#beginningOf> rdf:type owl:ObjectProperty ;
                                                       rdfs:subPropertyOf <http://ontology.asam.net/ontologies/Core#temporalPartOf> ;
                                                       owl:inverseOf <http://ontology.asam.net/ontologies/Core#hasBeginning> ;
                                                       rdfs:domain <http://ontology.asam.net/ontologies/Core#Event> ;
                                                       rdfs:comment "DEF: A temporalPartOf relationship type where a SpatioTemporalExtent has exactly one event that is its beginning." ,
                                                                    "HQDM beginning" .


###  http://ontology.asam.net/ontologies/Core#behind
<http://ontology.asam.net/ontologies/Core#behind> rdf:type owl:ObjectProperty ;
                                                  rdfs:subPropertyOf <http://ontology.asam.net/ontologies/Core#hasRelativePosition> ;
                                                  owl:inverseOf <http://ontology.asam.net/ontologies/Core#inFrontOf> ;
                                                  rdf:type owl:AsymmetricProperty ;
                                                  rdfs:comment "DEF: A hasRelativePosition relationship type where the first PhysicalObject is behind the second PhysicalObject." .


###  http://ontology.asam.net/ontologies/Core#behindConnectedTo
<http://ontology.asam.net/ontologies/Core#behindConnectedTo> rdf:type owl:ObjectProperty ;
                                                             rdfs:subPropertyOf <http://ontology.asam.net/ontologies/Core#longitudinalConnectedTo> ;
                                                             rdfs:comment "DEF: A longitudinalConnectedTo relationship type where two PhysicalObjects are connected and the first PhysicalObject is behind the second PhysicalObject." .


###  http://ontology.asam.net/ontologies/Core#behindLeftOf
<http://ontology.asam.net/ontologies/Core#behindLeftOf> rdf:type owl:ObjectProperty ;
                                                        rdfs:subPropertyOf <http://ontology.asam.net/ontologies/Core#hasRelativePosition> ;
                                                        owl:inverseOf <http://ontology.asam.net/ontologies/Core#frontRightOf> ;
                                                        rdf:type owl:AsymmetricProperty ;
                                                        rdfs:comment "DEF: A hasRelativePosition relationship type where the first PhysicalObject is behind and to the left of the second PhysicalObject." .


###  http://ontology.asam.net/ontologies/Core#behindRightOf
<http://ontology.asam.net/ontologies/Core#behindRightOf> rdf:type owl:ObjectProperty ;
                                                         rdfs:subPropertyOf <http://ontology.asam.net/ontologies/Core#hasRelativePosition> ;
                                                         owl:inverseOf <http://ontology.asam.net/ontologies/Core#frontLeftOf> ;
                                                         rdf:type owl:AsymmetricProperty ;
                                                         rdfs:comment "DEF: A hasRelativePosition relationship type where the first PhysicalObject is behind and to the right of the second PhysicalObject." .


###  http://ontology.asam.net/ontologies/Core#causes
<http://ontology.asam.net/ontologies/Core#causes> rdf:type owl:ObjectProperty ;
                                                  rdfs:domain <http://ontology.asam.net/ontologies/Core#ActivityState> ;
                                                  rdfs:range <http://ontology.asam.net/ontologies/Core#Event> ;
                                                  rdfs:comment "DEF: A relationship type where each activity is the cause of one or more events." ,
                                                               "HQDM causes" .


###  http://ontology.asam.net/ontologies/Core#componentOf
<http://ontology.asam.net/ontologies/Core#componentOf> rdf:type owl:ObjectProperty ;
                                                       rdfs:subPropertyOf <http://ontology.asam.net/ontologies/Core#partOf> ;
                                                       owl:inverseOf <http://ontology.asam.net/ontologies/Core#hasComponent> ;
                                                       rdf:type owl:FunctionalProperty ;
                                                       rdfs:domain <http://ontology.asam.net/ontologies/Core#SystemComponentState> ;
                                                       rdfs:range <http://ontology.asam.net/ontologies/Core#SystemState> ;
                                                       rdfs:comment "DEF: A partOf relationship type where each SystemComponent is partOf exactly one System." ,
                                                                    "HQDM component_of" .


###  http://ontology.asam.net/ontologies/Core#connectedTo
<http://ontology.asam.net/ontologies/Core#connectedTo> rdf:type owl:ObjectProperty ,
                                                                owl:SymmetricProperty ;
                                                       rdfs:domain <http://ontology.asam.net/ontologies/Core#PhysicalObjectState> ;
                                                       rdfs:range <http://ontology.asam.net/ontologies/Core#PhysicalObjectState> ;
                                                       rdfs:comment "DEF: A relationship type where two physical object have a spatial connection and touch each other. Spatial connections create bridges for the transfer of energy or other things between the objects. This object property has the same meaning as the class SpatialConnection, but a different representation." .


###  http://ontology.asam.net/ontologies/Core#defines
<http://ontology.asam.net/ontologies/Core#defines> rdf:type owl:ObjectProperty ,
                                                            owl:TransitiveProperty ;
                                                   rdfs:domain <http://ontology.asam.net/ontologies/Core#PhysicalQuantity> ;
                                                   rdfs:range <http://ontology.asam.net/ontologies/Core#PhysicalQuantity> ;
                                                   rdfs:comment "DEF: A relationship type that relates two numeric parameters. It expresses that one parameter value is determined by the other parameter value." .


###  http://ontology.asam.net/ontologies/Core#endingOf
<http://ontology.asam.net/ontologies/Core#endingOf> rdf:type owl:ObjectProperty ;
                                                    rdfs:subPropertyOf <http://ontology.asam.net/ontologies/Core#temporalPartOf> ;
                                                    owl:inverseOf <http://ontology.asam.net/ontologies/Core#hasEnding> ;
                                                    rdfs:domain <http://ontology.asam.net/ontologies/Core#Event> ;
                                                    rdfs:comment "DEF: A temporalPartOf relationship type where a SpatioTemporalExtent has exactly one event that is its ending." ,
                                                                 "HQDM ending" .


###  http://ontology.asam.net/ontologies/Core#frontConnectedTo
<http://ontology.asam.net/ontologies/Core#frontConnectedTo> rdf:type owl:ObjectProperty ;
                                                            rdfs:subPropertyOf <http://ontology.asam.net/ontologies/Core#longitudinalConnectedTo> ;
                                                            rdfs:comment "DEF: A longitudinalConnectedTo relationship type where two PhysicalObjects are connected and the first PhysicalObject is in front of the second PhysicalObject." .


###  http://ontology.asam.net/ontologies/Core#frontLeftOf
<http://ontology.asam.net/ontologies/Core#frontLeftOf> rdf:type owl:ObjectProperty ;
                                                       rdfs:subPropertyOf <http://ontology.asam.net/ontologies/Core#hasRelativePosition> ;
                                                       rdf:type owl:AsymmetricProperty ;
                                                       rdfs:comment "DEF: A hasRelativePosition relationship type where the first PhysicalObject is in front and to the left of the second PhysicalObject." .


###  http://ontology.asam.net/ontologies/Core#frontRightOf
<http://ontology.asam.net/ontologies/Core#frontRightOf> rdf:type owl:ObjectProperty ;
                                                        rdfs:subPropertyOf <http://ontology.asam.net/ontologies/Core#hasRelativePosition> ;
                                                        rdf:type owl:AsymmetricProperty ;
                                                        rdfs:comment "DEF: A hasRelativePosition relationship type where the first PhysicalObject is in front and to the right of the second PhysicalObject." .


###  http://ontology.asam.net/ontologies/Core#hasAngle
<http://ontology.asam.net/ontologies/Core#hasAngle> rdf:type owl:ObjectProperty ;
                                                    rdfs:subPropertyOf <http://ontology.asam.net/ontologies/Core#hasQuantity> ;
                                                    rdfs:range <http://ontology.asam.net/ontologies/Core#AngleQuantity> ;
                                                    rdfs:comment "DEF: A hasQuantity relationship type that specifies an angle quantity of something." .


###  http://ontology.asam.net/ontologies/Core#hasBeginning
<http://ontology.asam.net/ontologies/Core#hasBeginning> rdf:type owl:ObjectProperty ;
                                                        rdfs:subPropertyOf <http://ontology.asam.net/ontologies/Core#hasTemporalPart> ;
                                                        rdfs:range <http://ontology.asam.net/ontologies/Core#Event> ;
                                                        rdfs:comment "DEF: Inverse relationship of beginningOf" .


###  http://ontology.asam.net/ontologies/Core#hasColor
<http://ontology.asam.net/ontologies/Core#hasColor> rdf:type owl:ObjectProperty ;
                                                    rdfs:subPropertyOf <http://ontology.asam.net/ontologies/Core#hasProperty> ;
                                                    rdfs:comment "DEF: A hasPropertyrelationship type that specifies the color of something." .


###  http://ontology.asam.net/ontologies/Core#hasComponent
<http://ontology.asam.net/ontologies/Core#hasComponent> rdf:type owl:ObjectProperty ;
                                                        rdfs:subPropertyOf <http://ontology.asam.net/ontologies/Core#hasPart> ;
                                                        rdfs:comment "DEF: Inverse relationship of componentOf" .


###  http://ontology.asam.net/ontologies/Core#hasDirection
<http://ontology.asam.net/ontologies/Core#hasDirection> rdf:type owl:ObjectProperty ;
                                                        rdfs:subPropertyOf <http://ontology.asam.net/ontologies/Core#hasQuantity> ;
                                                        rdfs:range <http://ontology.asam.net/ontologies/Core#DirectionQuantity> ;
                                                        rdfs:comment "DEF: A hasQuantity relationship type that specifies a direction quantity of something." .


###  http://ontology.asam.net/ontologies/Core#hasDistance
<http://ontology.asam.net/ontologies/Core#hasDistance> rdf:type owl:ObjectProperty ;
                                                       rdfs:subPropertyOf <http://ontology.asam.net/ontologies/Core#hasLength> ;
                                                       rdfs:comment "DEF: A hasQuantity relationship type that specifies a distance quantity of something." .


###  http://ontology.asam.net/ontologies/Core#hasEnding
<http://ontology.asam.net/ontologies/Core#hasEnding> rdf:type owl:ObjectProperty ;
                                                     rdfs:subPropertyOf <http://ontology.asam.net/ontologies/Core#hasTemporalPart> ;
                                                     rdfs:range <http://ontology.asam.net/ontologies/Core#Event> ;
                                                     rdfs:comment "DEF: Inverse relationship of endingOf" .


###  http://ontology.asam.net/ontologies/Core#hasGeometry
<http://ontology.asam.net/ontologies/Core#hasGeometry> rdf:type owl:ObjectProperty ;
                                                       rdfs:subPropertyOf <http://ontology.asam.net/ontologies/Core#hasProperty> ;
                                                       rdfs:range <http://ontology.asam.net/ontologies/Core#Geometry> ;
                                                       rdfs:comment "DEF: A hasProperty relationship type that specifies the geometry of something, usually a physical object." .


###  http://ontology.asam.net/ontologies/Core#hasHeading
<http://ontology.asam.net/ontologies/Core#hasHeading> rdf:type owl:ObjectProperty ;
                                                      rdfs:subPropertyOf <http://ontology.asam.net/ontologies/Core#hasDirection> ;
                                                      rdfs:domain <http://ontology.asam.net/ontologies/Core#PhysicalObjectState> ;
                                                      rdfs:comment "DEF: A hasQuantity relationship type that specifies a direction that a moving object is heading in. This property is required for defining leftOf, rightOf, etc." .


###  http://ontology.asam.net/ontologies/Core#hasLength
<http://ontology.asam.net/ontologies/Core#hasLength> rdf:type owl:ObjectProperty ;
                                                     rdfs:subPropertyOf <http://ontology.asam.net/ontologies/Core#hasQuantity> ;
                                                     rdfs:range <http://ontology.asam.net/ontologies/Core#LengthQuantity> ;
                                                     rdfs:comment "DEF: A hasQuantity relationship type that specifies the length quantity of something." .


###  http://ontology.asam.net/ontologies/Core#hasMember
<http://ontology.asam.net/ontologies/Core#hasMember> rdf:type owl:ObjectProperty ;
                                                     owl:inverseOf <http://ontology.asam.net/ontologies/Core#memberOf> ;
                                                     rdf:type owl:AsymmetricProperty ;
                                                     rdfs:domain <http://ontology.asam.net/ontologies/Core#Set> ;
                                                     rdfs:comment "DEF: A relationship type stating that a Set has a particular thing as a member. A set can have anything of the respective type as a member." ,
                                                                  "EXAMPLES: A SetOfActivityStates can have an ActivityState as a member." .


###  http://ontology.asam.net/ontologies/Core#hasObject
<http://ontology.asam.net/ontologies/Core#hasObject> rdf:type owl:ObjectProperty ;
                                                     rdfs:subPropertyOf <http://ontology.asam.net/ontologies/Core#hasParticipant> ;
                                                     owl:inverseOf <http://ontology.asam.net/ontologies/Core#objectOf> ;
                                                     rdfs:comment "DEF: A hasParticipant relationship type that relates some activity to a physical object as object of the activity. The object is a non-actor participant. Inverse relationship of objectOf." .


###  http://ontology.asam.net/ontologies/Core#hasPart
<http://ontology.asam.net/ontologies/Core#hasPart> rdf:type owl:ObjectProperty ;
                                                   owl:inverseOf <http://ontology.asam.net/ontologies/Core#partOf> ;
                                                   rdf:type owl:AsymmetricProperty ;
                                                   rdfs:domain <http://ontology.asam.net/ontologies/Core#SpatioTemporalExtent> ;
                                                   rdfs:range <http://ontology.asam.net/ontologies/Core#SpatioTemporalExtent> ;
                                                   rdfs:comment "DEF: A relationship type where a SpatioTemporalExtent may consist of one or more others. Inverse relationship of partOf." ,
                                                                "HQDM consists_of" .


###  http://ontology.asam.net/ontologies/Core#hasParticipant
<http://ontology.asam.net/ontologies/Core#hasParticipant> rdf:type owl:ObjectProperty ;
                                                          rdfs:subPropertyOf <http://ontology.asam.net/ontologies/Core#hasPart> ;
                                                          owl:inverseOf <http://ontology.asam.net/ontologies/Core#participantOf> ;
                                                          rdfs:domain <http://ontology.asam.net/ontologies/Core#ActivityState> ;
                                                          rdfs:range <http://ontology.asam.net/ontologies/Core#Participant> ;
                                                          rdfs:comment "DEF: A hasPart relationship type where an ActivityState hasPart one or more Participants." ,
                                                                       "HQDM consists_of_participant" .


###  http://ontology.asam.net/ontologies/Core#hasProperty
<http://ontology.asam.net/ontologies/Core#hasProperty> rdf:type owl:ObjectProperty ;
                                                       rdfs:range <http://ontology.asam.net/ontologies/Core#PhysicalProperty> ;
                                                       rdfs:comment "DEF: Relationship type for specifying properties of particular things" .


###  http://ontology.asam.net/ontologies/Core#hasQuantity
<http://ontology.asam.net/ontologies/Core#hasQuantity> rdf:type owl:ObjectProperty ;
                                                       rdfs:subPropertyOf <http://ontology.asam.net/ontologies/Core#hasProperty> ;
                                                       rdfs:range <http://ontology.asam.net/ontologies/Core#PhysicalQuantity> ;
                                                       rdfs:comment "DEF: A relationship type for specifying quantities of particular things" .


###  http://ontology.asam.net/ontologies/Core#hasQuantityRelation
<http://ontology.asam.net/ontologies/Core#hasQuantityRelation> rdf:type owl:ObjectProperty ;
                                                               rdfs:domain <http://ontology.asam.net/ontologies/Core#PhysicalQuantity> ;
                                                               rdfs:range <http://ontology.asam.net/ontologies/Core#PhysicalQuantity> ;
                                                               rdfs:comment "DEF: A relationship type for basic arithmetic relationships between quantities" .


###  http://ontology.asam.net/ontologies/Core#hasRelationDirection
<http://ontology.asam.net/ontologies/Core#hasRelationDirection> rdf:type owl:ObjectProperty ;
                                                                rdfs:subPropertyOf <http://ontology.asam.net/ontologies/Core#hasDirection> ,
                                                                                   <http://ontology.asam.net/ontologies/Core#relationProperty> ;
                                                                rdfs:domain <http://ontology.asam.net/ontologies/Core#SpatialRelation> ;
                                                                rdfs:range <http://ontology.asam.net/ontologies/Core#DirectionQuantity> ;
                                                                rdfs:comment "DEF: A hasQuantity relationship type that specifies the direction of a spatial relation." .


###  http://ontology.asam.net/ontologies/Core#hasRelativePosition
<http://ontology.asam.net/ontologies/Core#hasRelativePosition> rdf:type owl:ObjectProperty ;
                                                               rdfs:domain <http://ontology.asam.net/ontologies/Core#PhysicalObjectState> ;
                                                               rdfs:range <http://ontology.asam.net/ontologies/Core#PhysicalObjectState> ;
                                                               rdfs:comment "DEF: Object properties derived from SpatialRelation" .


###  http://ontology.asam.net/ontologies/Core#hasRelativeTime
<http://ontology.asam.net/ontologies/Core#hasRelativeTime> rdf:type owl:ObjectProperty ;
                                                           rdfs:domain <http://ontology.asam.net/ontologies/Core#Event> ;
                                                           rdfs:range <http://ontology.asam.net/ontologies/Core#Event> ;
                                                           rdfs:comment "DEF: Object properties derived from TemporalRelation" .


###  http://ontology.asam.net/ontologies/Core#hasSpatialObject
<http://ontology.asam.net/ontologies/Core#hasSpatialObject> rdf:type owl:ObjectProperty ;
                                                            rdfs:subPropertyOf <http://ontology.asam.net/ontologies/Core#relationProperty> ;
                                                            rdf:type owl:FunctionalProperty ,
                                                                     owl:InverseFunctionalProperty ;
                                                            rdfs:domain <http://ontology.asam.net/ontologies/Core#SpatialRelation> ;
                                                            rdfs:range <http://ontology.asam.net/ontologies/Core#PhysicalObjectState> ;
                                                            rdfs:comment "DEF: A relationProperty designating the object, destination, or \"recepient\" in a SpatialRelation." .


###  http://ontology.asam.net/ontologies/Core#hasSpatialSubject
<http://ontology.asam.net/ontologies/Core#hasSpatialSubject> rdf:type owl:ObjectProperty ;
                                                             rdfs:subPropertyOf <http://ontology.asam.net/ontologies/Core#relationProperty> ;
                                                             rdf:type owl:FunctionalProperty ,
                                                                      owl:InverseFunctionalProperty ;
                                                             rdfs:domain <http://ontology.asam.net/ontologies/Core#SpatialRelation> ;
                                                             rdfs:range <http://ontology.asam.net/ontologies/Core#PhysicalObjectState> ;
                                                             rdfs:comment "DEF: A relationProperty designating the subject, origin, or \"owner\" in a SpatialRelation." .


###  http://ontology.asam.net/ontologies/Core#hasSpeed
<http://ontology.asam.net/ontologies/Core#hasSpeed> rdf:type owl:ObjectProperty ;
                                                    rdfs:subPropertyOf <http://ontology.asam.net/ontologies/Core#hasQuantity> ;
                                                    rdfs:range <http://ontology.asam.net/ontologies/Core#SpeedQuantity> ;
                                                    rdfs:comment "DEF: A hasQuantity relationship type that specifies speed." .


###  http://ontology.asam.net/ontologies/Core#hasSubject
<http://ontology.asam.net/ontologies/Core#hasSubject> rdf:type owl:ObjectProperty ;
                                                      rdfs:subPropertyOf <http://ontology.asam.net/ontologies/Core#hasParticipant> ;
                                                      owl:inverseOf <http://ontology.asam.net/ontologies/Core#subjectOf> ;
                                                      rdfs:comment "DEF: A hasParticipant relationship type that relates some activity to a physical object as subject of the activity. The subject is an actor participant. Inverse relationship of subjectOf." .


###  http://ontology.asam.net/ontologies/Core#hasTemporalPart
<http://ontology.asam.net/ontologies/Core#hasTemporalPart> rdf:type owl:ObjectProperty ;
                                                           rdfs:subPropertyOf <http://ontology.asam.net/ontologies/Core#hasPart> ;
                                                           owl:inverseOf <http://ontology.asam.net/ontologies/Core#temporalPartOf> ;
                                                           rdfs:comment "DEF: A hasPart relationship type where one spatio-temporal extent has another spatio-temporal extent as a temporal part.  This implies that the temporal extent of the part is within the temporal extent of the whole. Inverse relationship of temporalPartOf." .


###  http://ontology.asam.net/ontologies/Core#inFrontOf
<http://ontology.asam.net/ontologies/Core#inFrontOf> rdf:type owl:ObjectProperty ;
                                                     rdfs:subPropertyOf <http://ontology.asam.net/ontologies/Core#hasRelativePosition> ;
                                                     rdf:type owl:AsymmetricProperty ;
                                                     rdfs:comment "DEF: A hasRelativePosition relationship type where the first PhysicalObject is in front of the second PhysicalObject." .


###  http://ontology.asam.net/ontologies/Core#intendedRole
<http://ontology.asam.net/ontologies/Core#intendedRole> rdf:type owl:ObjectProperty ;
                                                        rdfs:domain <http://ontology.asam.net/ontologies/Core#FunctionalObjectState> ;
                                                        rdfs:range <http://ontology.asam.net/ontologies/Core#Role> ;
                                                        rdfs:comment "DEF: A relationship type where a FunctionalObject has one or more intended role(s)." ,
                                                                     "HQDM intended_role" .


###  http://ontology.asam.net/ontologies/Core#involves
<http://ontology.asam.net/ontologies/Core#involves> rdf:type owl:ObjectProperty ;
                                                    rdfs:subPropertyOf <http://ontology.asam.net/ontologies/Core#relationProperty> ;
                                                    rdf:type owl:FunctionalProperty ,
                                                             owl:InverseFunctionalProperty ;
                                                    rdfs:domain <http://ontology.asam.net/ontologies/Core#DefinedRelationship> ;
                                                    rdfs:range <http://ontology.asam.net/ontologies/Core#Classification> ;
                                                    rdfs:comment "DEF: A relationProperty that states that the classification of some thing in a role is involved in a relationship." ,
                                                                 "HQDM involves" .


###  http://ontology.asam.net/ontologies/Core#latitudinalConnectedTo
<http://ontology.asam.net/ontologies/Core#latitudinalConnectedTo> rdf:type owl:ObjectProperty ;
                                                                  rdfs:subPropertyOf <http://ontology.asam.net/ontologies/Core#connectedTo> ;
                                                                  rdfs:comment "DEF: A connectedTo relationship type where the connection is in the latitudinal (East-West) direction with reference to the reference coordinate system." .


###  http://ontology.asam.net/ontologies/Core#leftConnectedTo
<http://ontology.asam.net/ontologies/Core#leftConnectedTo> rdf:type owl:ObjectProperty ;
                                                           rdfs:subPropertyOf <http://ontology.asam.net/ontologies/Core#latitudinalConnectedTo> ;
                                                           rdfs:comment "DEF: A latitudinalConnectedTo relationship type where two PhysicalObjects are connected and the first PhysicalObject is to the left of the second PhysicalObject." .


###  http://ontology.asam.net/ontologies/Core#leftOf
<http://ontology.asam.net/ontologies/Core#leftOf> rdf:type owl:ObjectProperty ;
                                                  rdfs:subPropertyOf <http://ontology.asam.net/ontologies/Core#hasRelativePosition> ;
                                                  owl:inverseOf <http://ontology.asam.net/ontologies/Core#rightOf> ;
                                                  rdf:type owl:AsymmetricProperty ;
                                                  rdfs:comment "DEF: A hasRelativePosition relationship type where the first PhysicalObject is to the left of the second PhysicalObject." .


###  http://ontology.asam.net/ontologies/Core#locatedOn
<http://ontology.asam.net/ontologies/Core#locatedOn> rdf:type owl:ObjectProperty ,
                                                              owl:AsymmetricProperty ;
                                                     rdfs:domain <http://ontology.asam.net/ontologies/Core#PhysicalObjectState> ;
                                                     rdfs:comment "DEF: Object property version of RelativeLocation. Note that when using \"locatedOn\", it is not possible to describe the actual position of the located object on the location object (you need a RelativeLocation for that)." .


###  http://ontology.asam.net/ontologies/Core#longitudinalConnectedTo
<http://ontology.asam.net/ontologies/Core#longitudinalConnectedTo> rdf:type owl:ObjectProperty ;
                                                                   rdfs:subPropertyOf <http://ontology.asam.net/ontologies/Core#connectedTo> ;
                                                                   rdfs:comment "DEF: A connectedTo relationship type where the connection is in the longitudinal (North-South) direction with reference to the reference coordinate system." .


###  http://ontology.asam.net/ontologies/Core#memberOf
<http://ontology.asam.net/ontologies/Core#memberOf> rdf:type owl:ObjectProperty ,
                                                             owl:AsymmetricProperty ;
                                                    rdfs:range <http://ontology.asam.net/ontologies/Core#Set> ;
                                                    rdfs:comment "DEF: A relationship type stating that a thing is a member of some Set. A set can have anything of the respective type as a member, even other Sets." ,
                                                                 "EXAMPLES: A SetOfActivityStates can have an ActivityState as a member." .


###  http://ontology.asam.net/ontologies/Core#objectOf
<http://ontology.asam.net/ontologies/Core#objectOf> rdf:type owl:ObjectProperty ;
                                                    rdfs:subPropertyOf <http://ontology.asam.net/ontologies/Core#participantOf> ;
                                                    rdfs:comment "DEF: A participantOf relationship type that relates some physical object as object to some activity. The object is a non-actor participant." .


###  http://ontology.asam.net/ontologies/Core#occursAfter
<http://ontology.asam.net/ontologies/Core#occursAfter> rdf:type owl:ObjectProperty ;
                                                       rdfs:subPropertyOf <http://ontology.asam.net/ontologies/Core#occursAtDifferentTime> ;
                                                       owl:inverseOf <http://ontology.asam.net/ontologies/Core#occursBefore> ;
                                                       rdfs:comment "DEF: A hasRelativeTime relationship type specifying that the first event (marking the beginning or ending of some activity of physical object) occurs after the second event." .


###  http://ontology.asam.net/ontologies/Core#occursAtDifferentTime
<http://ontology.asam.net/ontologies/Core#occursAtDifferentTime> rdf:type owl:ObjectProperty ;
                                                                 rdfs:subPropertyOf <http://ontology.asam.net/ontologies/Core#hasRelativeTime> ;
                                                                 rdf:type owl:AsymmetricProperty ;
                                                                 rdfs:comment "DEF: A hasRelativeTime relationship type specifying that the first event (marking the beginning or ending of some activity of physical object) occurs at a different time from the second event." .


###  http://ontology.asam.net/ontologies/Core#occursAtSameTime
<http://ontology.asam.net/ontologies/Core#occursAtSameTime> rdf:type owl:ObjectProperty ;
                                                            rdfs:subPropertyOf <http://ontology.asam.net/ontologies/Core#hasRelativeTime> ;
                                                            rdf:type owl:SymmetricProperty ;
                                                            rdfs:comment "DEF: A hasRelativeTime relationship type specifying that the first event (marking the beginning or ending of some activity of physical object) occurs at the same this as the second event. Note that when two events occur at the same time, the events are both parts of the same PointInTime" .


###  http://ontology.asam.net/ontologies/Core#occursBefore
<http://ontology.asam.net/ontologies/Core#occursBefore> rdf:type owl:ObjectProperty ;
                                                        rdfs:subPropertyOf <http://ontology.asam.net/ontologies/Core#occursAtDifferentTime> ;
                                                        rdfs:comment "DEF: A hasRelativeTime relationship type specifying that the first event (marking the beginning or ending of some activity of physical object) occurs before the second event" .


###  http://ontology.asam.net/ontologies/Core#part
<http://ontology.asam.net/ontologies/Core#part> rdf:type owl:ObjectProperty ;
                                                rdfs:subPropertyOf <http://ontology.asam.net/ontologies/Core#relationProperty> ;
                                                rdf:type owl:FunctionalProperty ,
                                                         owl:InverseFunctionalProperty ;
                                                rdfs:domain <http://ontology.asam.net/ontologies/Core#Aggregation> ;
                                                rdfs:range <http://ontology.asam.net/ontologies/Core#SpatioTemporalExtent> ;
                                                rdfs:comment "DEF: A relationProperty that states that each Aggregation has exactly one spatioTemporalExtent that is the part in the Aggregation." ,
                                                             "HQDM part" .


###  http://ontology.asam.net/ontologies/Core#partOf
<http://ontology.asam.net/ontologies/Core#partOf> rdf:type owl:ObjectProperty ;
                                                  rdfs:subPropertyOf <http://ontology.asam.net/ontologies/Core#aggregatedInto> ;
                                                  rdfs:comment "DEF: An aggregatedInto relationship type where a SpatioTemporalExtent may be part of another and the whole has emergent properties and is more than just the sum of its parts. This object property has the same meaning as the class Composition, but a different representation." ,
                                                               "HQDM part__of" .


###  http://ontology.asam.net/ontologies/Core#partOfPossibleWorld
<http://ontology.asam.net/ontologies/Core#partOfPossibleWorld> rdf:type owl:ObjectProperty ;
                                                               rdfs:subPropertyOf <http://ontology.asam.net/ontologies/Core#partOf> ;
                                                               rdfs:range <http://ontology.asam.net/ontologies/Core#PossibleWorld> ;
                                                               rdfs:comment "DEF: A partOf relationship type where a SpatioTemporalExtent may be partOf one or more PossibleWorld." ,
                                                                            "HQDM part_of_possible_world" .


###  http://ontology.asam.net/ontologies/Core#participantOf
<http://ontology.asam.net/ontologies/Core#participantOf> rdf:type owl:ObjectProperty ;
                                                         rdfs:subPropertyOf <http://ontology.asam.net/ontologies/Core#partOf> ;
                                                         rdfs:domain <http://ontology.asam.net/ontologies/Core#Participant> ;
                                                         rdfs:range <http://ontology.asam.net/ontologies/Core#ActivityState> ;
                                                         rdfs:comment "DEF: A relationship stating the participation of a physical object in an activity." ,
                                                                      "HQDM participant_in" .


###  http://ontology.asam.net/ontologies/Core#quantityEqualTo
<http://ontology.asam.net/ontologies/Core#quantityEqualTo> rdf:type owl:ObjectProperty ;
                                                           rdfs:subPropertyOf <http://ontology.asam.net/ontologies/Core#hasQuantityRelation> ;
                                                           rdf:type owl:SymmetricProperty ;
                                                           rdfs:domain <http://ontology.asam.net/ontologies/Core#PhysicalQuantity> ;
                                                           rdfs:range <http://ontology.asam.net/ontologies/Core#PhysicalQuantity> ;
                                                           rdfs:comment "DEF: A hasQuantityRelation relationship type, where the value for the second quantity is equal to the value of the first quantity." .


###  http://ontology.asam.net/ontologies/Core#quantityGreaterThan
<http://ontology.asam.net/ontologies/Core#quantityGreaterThan> rdf:type owl:ObjectProperty ;
                                                               rdfs:subPropertyOf <http://ontology.asam.net/ontologies/Core#hasQuantityRelation> ;
                                                               owl:inverseOf <http://ontology.asam.net/ontologies/Core#quantityLessThanOrEqualTo> ;
                                                               rdf:type owl:TransitiveProperty ;
                                                               rdfs:domain <http://ontology.asam.net/ontologies/Core#PhysicalQuantity> ;
                                                               rdfs:range <http://ontology.asam.net/ontologies/Core#PhysicalQuantity> ;
                                                               rdfs:comment "DEF: A hasQuantityRelation relationship type, where the value for the second quantity is strictly greater than the value of the first quantity." .


###  http://ontology.asam.net/ontologies/Core#quantityGreaterThanOrEqualTo
<http://ontology.asam.net/ontologies/Core#quantityGreaterThanOrEqualTo> rdf:type owl:ObjectProperty ;
                                                                        rdfs:subPropertyOf <http://ontology.asam.net/ontologies/Core#hasQuantityRelation> ;
                                                                        owl:inverseOf <http://ontology.asam.net/ontologies/Core#quantityLessThan> ;
                                                                        rdf:type owl:TransitiveProperty ;
                                                                        rdfs:domain <http://ontology.asam.net/ontologies/Core#PhysicalQuantity> ;
                                                                        rdfs:range <http://ontology.asam.net/ontologies/Core#PhysicalQuantity> ;
                                                                        rdfs:comment "DEF: A hasQuantityRelation relationship type, where the value for the second quantity is greater than or equal to the value of the first quantity." .


###  http://ontology.asam.net/ontologies/Core#quantityLessThan
<http://ontology.asam.net/ontologies/Core#quantityLessThan> rdf:type owl:ObjectProperty ;
                                                            rdfs:subPropertyOf <http://ontology.asam.net/ontologies/Core#hasQuantityRelation> ;
                                                            rdf:type owl:TransitiveProperty ;
                                                            rdfs:domain <http://ontology.asam.net/ontologies/Core#PhysicalQuantity> ;
                                                            rdfs:range <http://ontology.asam.net/ontologies/Core#PhysicalQuantity> ;
                                                            rdfs:comment "DEF: A hasQuantityRelation relationship type, where the value for the second quantity is strictly less than the value of the first quantity." .


###  http://ontology.asam.net/ontologies/Core#quantityLessThanOrEqualTo
<http://ontology.asam.net/ontologies/Core#quantityLessThanOrEqualTo> rdf:type owl:ObjectProperty ;
                                                                     rdfs:subPropertyOf <http://ontology.asam.net/ontologies/Core#hasQuantityRelation> ;
                                                                     rdf:type owl:TransitiveProperty ;
                                                                     rdfs:domain <http://ontology.asam.net/ontologies/Core#PhysicalQuantity> ;
                                                                     rdfs:range <http://ontology.asam.net/ontologies/Core#PhysicalQuantity> ;
                                                                     rdfs:comment "DEF: A hasQuantityRelation relationship type, where the value for the second quantity is less than or equal to the value of the first quantity." .


###  http://ontology.asam.net/ontologies/Core#quantityNotEqualTo
<http://ontology.asam.net/ontologies/Core#quantityNotEqualTo> rdf:type owl:ObjectProperty ;
                                                              rdfs:subPropertyOf <http://ontology.asam.net/ontologies/Core#hasQuantityRelation> ;
                                                              rdf:type owl:SymmetricProperty ;
                                                              rdfs:domain <http://ontology.asam.net/ontologies/Core#PhysicalQuantity> ;
                                                              rdfs:range <http://ontology.asam.net/ontologies/Core#PhysicalQuantity> ;
                                                              rdfs:comment "DEF: A hasQuantityRelation relationship type, where the value for the second quantity is not equal to the value of the first quantity." .


###  http://ontology.asam.net/ontologies/Core#relationProperty
<http://ontology.asam.net/ontologies/Core#relationProperty> rdf:type owl:ObjectProperty ;
                                                            rdfs:domain <http://ontology.asam.net/ontologies/Core#Relationship> ;
                                                            rdfs:comment "DEF: Relationship types that are generally used only to define other properties, for example, using SWRL." .


###  http://ontology.asam.net/ontologies/Core#rightConnectedTo
<http://ontology.asam.net/ontologies/Core#rightConnectedTo> rdf:type owl:ObjectProperty ;
                                                            rdfs:subPropertyOf <http://ontology.asam.net/ontologies/Core#latitudinalConnectedTo> ;
                                                            rdfs:comment "DEF: A latitudinalConnectedTo relationship type where two PhysicalObjects are connected and the first PhysicalObject is to the right of the second PhysicalObject." .


###  http://ontology.asam.net/ontologies/Core#rightOf
<http://ontology.asam.net/ontologies/Core#rightOf> rdf:type owl:ObjectProperty ;
                                                   rdfs:subPropertyOf <http://ontology.asam.net/ontologies/Core#hasRelativePosition> ;
                                                   rdf:type owl:AsymmetricProperty ;
                                                   rdfs:comment "DEF: A hasRelativePosition relationship type where the first PhysicalObject is to the right of the second PhysicalObject." .


###  http://ontology.asam.net/ontologies/Core#rolePlayedBy
<http://ontology.asam.net/ontologies/Core#rolePlayedBy> rdf:type owl:ObjectProperty ;
                                                        rdfs:subPropertyOf <http://ontology.asam.net/ontologies/Core#relationProperty> ;
                                                        rdfs:domain <http://ontology.asam.net/ontologies/Core#Role> ;
                                                        rdfs:range <http://ontology.asam.net/ontologies/Core#Participant> ;
                                                        rdfs:comment "DEF: A relationProperty that states that a Role is the role of some Participant." .


###  http://ontology.asam.net/ontologies/Core#roleUsedIn
<http://ontology.asam.net/ontologies/Core#roleUsedIn> rdf:type owl:ObjectProperty ;
                                                      rdfs:subPropertyOf <http://ontology.asam.net/ontologies/Core#relationProperty> ;
                                                      rdfs:domain <http://ontology.asam.net/ontologies/Core#Role> ;
                                                      rdfs:range <http://ontology.asam.net/ontologies/Core#ActivityState> ;
                                                      rdfs:comment "DEF: A relationProperty that states that a Role is used in an Activity." .


###  http://ontology.asam.net/ontologies/Core#subjectOf
<http://ontology.asam.net/ontologies/Core#subjectOf> rdf:type owl:ObjectProperty ;
                                                     rdfs:subPropertyOf <http://ontology.asam.net/ontologies/Core#participantOf> ;
                                                     rdfs:comment "DEF: A participantOf relationship type that relates some physical object as subject to some activity. The subject is an actor participant." .


###  http://ontology.asam.net/ontologies/Core#temporalPartOf
<http://ontology.asam.net/ontologies/Core#temporalPartOf> rdf:type owl:ObjectProperty ;
                                                          rdfs:subPropertyOf <http://ontology.asam.net/ontologies/Core#partOf> ;
                                                          rdfs:comment "DEF: A partOf relationship type where a SpatioTemporalExtent may be a temporal part of one or more other SpatioTemporalExtent. This object property has the same meaning as the class TemporalComposition, but a different representation." ,
                                                                       "HQDM temporal__part_of" .


###  http://ontology.asam.net/ontologies/Core#whole
<http://ontology.asam.net/ontologies/Core#whole> rdf:type owl:ObjectProperty ;
                                                 rdfs:subPropertyOf <http://ontology.asam.net/ontologies/Core#relationProperty> ;
                                                 rdf:type owl:FunctionalProperty ,
                                                          owl:InverseFunctionalProperty ;
                                                 rdfs:domain <http://ontology.asam.net/ontologies/Core#Aggregation> ;
                                                 rdfs:range <http://ontology.asam.net/ontologies/Core#SpatioTemporalExtent> ;
                                                 rdfs:comment "DEF: A relationProperty that states that each Aggregation has exactly one spatioTemporalExtent that is the whole in the Aggregation." ,
                                                              "HQDM whole" .


###  http://ontology.asam.net/ontologies/OpenXOntology.owl#HQDM_aggregated_into
:HQDM_aggregated_into rdf:type owl:ObjectProperty ;
                      rdfs:comment """A relationship type where a spatio_temporal_extent may be aggregated into one or more others.
Note: This has the same meaning as, but different representation to, the aggregation entity type""" .


###  http://ontology.asam.net/ontologies/OpenXOntology.owl#HQDM_beginning
:HQDM_beginning rdf:type owl:ObjectProperty ;
                rdfs:subPropertyOf :HQDM_temporal_part_of ;
                rdfs:comment "A part_of relationship type where a spatio_temporal_extent has exactly one event that is its beginning." .


###  http://ontology.asam.net/ontologies/OpenXOntology.owl#HQDM_causes
:HQDM_causes rdf:type owl:ObjectProperty ;
             rdfs:comment "A relationship type where each activity is the cause of one or more event." .


###  http://ontology.asam.net/ontologies/OpenXOntology.owl#HQDM_classifier
:HQDM_classifier rdf:type owl:ObjectProperty ,
                          owl:FunctionalProperty ,
                          owl:InverseFunctionalProperty ;
                 rdfs:comment "only used for reified classification relationships" .


###  http://ontology.asam.net/ontologies/OpenXOntology.owl#HQDM_component_of
:HQDM_component_of rdf:type owl:ObjectProperty ;
                   rdfs:subPropertyOf :HQDM_part_of ;
                   rdf:type owl:FunctionalProperty ;
                   rdfs:comment "A part_of relationship type where each system_component is part_of exactly one system." .


###  http://ontology.asam.net/ontologies/OpenXOntology.owl#HQDM_consists_of
:HQDM_consists_of rdf:type owl:ObjectProperty ;
                  owl:inverseOf :HQDM_part_of ;
                  rdfs:comment """A relationship type where a spatio_temporal_extent may consist of one or more others.
Note: This is the inverse of part__of""" .


###  http://ontology.asam.net/ontologies/OpenXOntology.owl#HQDM_consists_of_participant
:HQDM_consists_of_participant rdf:type owl:ObjectProperty ;
                              rdfs:subPropertyOf :HQDM_consists_of ;
                              owl:inverseOf :HQDM_participant_in ;
                              rdfs:comment "A consists_of relationship type where an activity consists_of one or more participants." ,
                                           "note the domain should be the union of activity and association" .


###  http://ontology.asam.net/ontologies/OpenXOntology.owl#HQDM_determines
:HQDM_determines rdf:type owl:ObjectProperty ;
                 rdfs:range owl:Thing ;
                 rdfs:comment "A relationship type where an activity may determine one or more thing to be the case." .


###  http://ontology.asam.net/ontologies/OpenXOntology.owl#HQDM_ending
:HQDM_ending rdf:type owl:ObjectProperty ;
             rdfs:subPropertyOf :HQDM_temporal_part_of ;
             rdfs:comment "A part_of relationship type where a spatio_temporal_extent has exactly one event that is its ending." ,
                          "from text 11.2: beginning and ending are examples of the temporal_composition relationship" .


###  http://ontology.asam.net/ontologies/OpenXOntology.owl#HQDM_has_member
:HQDM_has_member rdf:type owl:ObjectProperty ;
                 owl:inverseOf :HQDM_member_of .


###  http://ontology.asam.net/ontologies/OpenXOntology.owl#HQDM_intended_role
:HQDM_intended_role rdf:type owl:ObjectProperty ;
                    rdfs:comment "A relationship type where a functional_object has one or more intended role(s)" .


###  http://ontology.asam.net/ontologies/OpenXOntology.owl#HQDM_involves
:HQDM_involves rdf:type owl:ObjectProperty ;
               rdfs:comment "A meta-relationship type where the classification of some thing in a role is involved in a relationship." .


###  http://ontology.asam.net/ontologies/OpenXOntology.owl#HQDM_member
:HQDM_member rdf:type owl:ObjectProperty ,
                      owl:FunctionalProperty ,
                      owl:InverseFunctionalProperty ;
             rdfs:range owl:Thing ;
             rdfs:comment "only used for reified classification relationships" .


###  http://ontology.asam.net/ontologies/OpenXOntology.owl#HQDM_member_of
:HQDM_member_of rdf:type owl:ObjectProperty ;
                rdfs:domain owl:Thing ;
                rdfs:comment "note that a class can be a member_of a class_of_class, etc." .


###  http://ontology.asam.net/ontologies/OpenXOntology.owl#HQDM_member_of_kind
:HQDM_member_of_kind rdf:type owl:ObjectProperty ;
                     rdfs:comment """A member_of relationship type where each defined_relationship is a member_of exactly one kind_of_relationship_with_signature.

Note: member_of_kind is only for assigning kinds (sets of things that have common characteristics = concepts in ISO704) to  things (including relationships, so not just spatio-temporal extents)""" .


###  http://ontology.asam.net/ontologies/OpenXOntology.owl#HQDM_part
:HQDM_part rdf:type owl:ObjectProperty ,
                    owl:FunctionalProperty ,
                    owl:InverseFunctionalProperty ;
           rdfs:comment "from text 11.2: Each aggregation has exactly one spatio_temporal_extent that is the part in the aggregation." ,
                        "only used for reified whole-part relationships" .


###  http://ontology.asam.net/ontologies/OpenXOntology.owl#HQDM_part__of_by_class
:HQDM_part__of_by_class rdf:type owl:ObjectProperty ;
                        rdfs:comment "A relationship type where a member_of a class_of_spatio_temporal_extent is part_of a member_of some class_of_spatio_temporal_extent." .


###  http://ontology.asam.net/ontologies/OpenXOntology.owl#HQDM_part_of
:HQDM_part_of rdf:type owl:ObjectProperty ;
              rdfs:subPropertyOf :HQDM_aggregated_into ;
              rdfs:comment """An aggregated_into relationship type where a spatio_temporal_extent may be part of another and the whole has emergent properties and is more than just the sum of its parts
Note: This relationship has the same meaning but is a different representation of the composition entity type.""" .


###  http://ontology.asam.net/ontologies/OpenXOntology.owl#HQDM_participant_in
:HQDM_participant_in rdf:type owl:ObjectProperty ;
                     rdfs:comment "main relationship for stating the participation of a physical object in an activity" .


###  http://ontology.asam.net/ontologies/OpenXOntology.owl#HQDM_references
:HQDM_references rdf:type owl:ObjectProperty ;
                 rdfs:range owl:Thing ;
                 rdfs:comment "A relationship type where an activity may reference one or more thing." .


###  http://ontology.asam.net/ontologies/OpenXOntology.owl#HQDM_temporal_part_of
:HQDM_temporal_part_of rdf:type owl:ObjectProperty ;
                       rdfs:subPropertyOf :HQDM_part_of ;
                       rdfs:comment """A part_of relationship type where a spatio_temporal_extent may be a temporal part of one or more other spatio_temporal_extent.

Note: this is temporal_composition represented as a relationship instead of an entity type""" ,
                                    "from text 11.2: not all properties (classes of states) of temporal wholes are inherited by temporal parts (ex. the property of being a whole life individual) - these classes  are not temporally dissective" .


###  http://ontology.asam.net/ontologies/OpenXOntology.owl#HQDM_whole
:HQDM_whole rdf:type owl:ObjectProperty ,
                     owl:FunctionalProperty ,
                     owl:InverseFunctionalProperty ;
            rdfs:comment "From text 11.2: Each aggregation has exactly one spatio_temporal_extent that is the whole in the aggregation." ,
                         "only used for reified whole-part relationships" .


###  http://ontology.asam.net/ontologies/OpenXOntology.owl#part_of_possible_world
:part_of_possible_world rdf:type owl:ObjectProperty ;
                        rdfs:subPropertyOf :HQDM_part_of ;
                        rdfs:comment """A part_of relationship type where a spatio_temporal_extent may be part_of one or more possible_world.
Note: The relationship is optional because a possible_world is not part_of any other spatio_temporal_extent.""" .


#################################################################
#    Data properties
#################################################################

###  http://ontology.asam.net/ontologies/Core#hasValue
<http://ontology.asam.net/ontologies/Core#hasValue> rdf:type owl:DatatypeProperty ;
                                                    rdfs:domain <http://ontology.asam.net/ontologies/Core#PhysicalQuantity> ;
                                                    rdfs:range xsd:float ;
                                                    rdfs:comment "DEF: a datatype property for specifying the numerical value of a quantity as a float. Note that this is a temporary solution to the specification of quantities in OxO." .


###  http://ontology.asam.net/ontologies/OpenXOntology.owl#HQDM_has_real_value
:HQDM_has_real_value rdf:type owl:DatatypeProperty ,
                              owl:FunctionalProperty ;
                     rdfs:range owl:real ;
                     rdfs:comment """called value_ in HQDM
A relationship type where an identification_of_physical_quantity consists of exactly one REAL as its value.
Note 1: The members of the data type REAL provide an identification of a real number.
Note 2: The relationship name has been renamed from consists of by class to value.""" .


#################################################################
#    Classes
#################################################################

###  http://ontology.asam.net/ontologies/Core#AbstractObject
<http://ontology.asam.net/ontologies/Core#AbstractObject> rdf:type owl:Class ;
                                                          rdfs:subClassOf <http://ontology.asam.net/ontologies/Core#CoreConcepts> ;
                                                          owl:disjointWith <http://ontology.asam.net/ontologies/Core#SpatioTemporalExtent> ;
                                                          rdfs:comment "DEF: A thing that does not exist in space or time. Abstract objects are used to express characteristics of spatio-temporal extents, such as properties and roles." ,
                                                                       "EXAMPLES: not applicable." ,
                                                                       "HQDM abstract_object" ,
                                                                       "USAGE: This class will generally not be used directly in the OpenX domain." .


###  http://ontology.asam.net/ontologies/Core#ActivityState
<http://ontology.asam.net/ontologies/Core#ActivityState> rdf:type owl:Class ;
                                                         rdfs:subClassOf <http://ontology.asam.net/ontologies/Core#State> ,
                                                                         [ rdf:type owl:Restriction ;
                                                                           owl:onProperty <http://ontology.asam.net/ontologies/Core#causes> ;
                                                                           owl:someValuesFrom <http://ontology.asam.net/ontologies/Core#Event>
                                                                         ] ,
                                                                         [ rdf:type owl:Restriction ;
                                                                           owl:onProperty <http://ontology.asam.net/ontologies/Core#hasParticipant> ;
                                                                           owl:someValuesFrom <http://ontology.asam.net/ontologies/Core#Participant>
                                                                         ] ,
                                                                         [ rdf:type owl:Restriction ;
                                                                           owl:onProperty <http://ontology.asam.net/ontologies/Core#memberOf> ;
                                                                           owl:allValuesFrom <http://ontology.asam.net/ontologies/Core#SetOfActivityStates>
                                                                         ] ;
                                                         rdfs:comment "DEF: A State that represents the whole life of an activity or a temporal part of an activity. Activities consist of their participants, which are members of PhysicalObjectState, and cause some event. The end event of an activity state is caused by that activity, which implies that the activity describes some change between the start event and end event." ,
                                                                      "EXAMPLES: the movements of a cloud or an animal crossing a road." ,
                                                                      "HQDM state_of_activity" ,
                                                                      "USAGE: Use this class for (temporal parts of) activities that are not the direct result of some intent, for example, a person's intent." .


###  http://ontology.asam.net/ontologies/Core#Aggregation
<http://ontology.asam.net/ontologies/Core#Aggregation> rdf:type owl:Class ;
                                                       rdfs:subClassOf <http://ontology.asam.net/ontologies/Core#Relationship> ;
                                                       rdfs:comment "DEF: A Relationship where the whole is at least the sum of the parts. Basis for object property aggregatedInto." ,
                                                                    "EXAMPLES: not applicable." ,
                                                                    "HQDM aggregation" ,
                                                                    "USAGE: This class will generally not be used directly in the OpenX domain." .


###  http://ontology.asam.net/ontologies/Core#AngleQuantity
<http://ontology.asam.net/ontologies/Core#AngleQuantity> rdf:type owl:Class ;
                                                         rdfs:subClassOf <http://ontology.asam.net/ontologies/Core#PhysicalQuantity> ;
                                                         rdfs:comment "DEF: A PhysicalQuantity that is an angle value in degrees, between 0 and 360." ,
                                                                      "EXAMPLES:" ,
                                                                      "USAGE: Use this class instead of DirectionQuantity when specifying angles that are not actual directions respective to some coordinate system." .


###  http://ontology.asam.net/ontologies/Core#BiologicalObjectState
<http://ontology.asam.net/ontologies/Core#BiologicalObjectState> rdf:type owl:Class ;
                                                                 rdfs:subClassOf <http://ontology.asam.net/ontologies/Core#PhysicalObjectState> ;
                                                                 rdfs:comment "DEF: A PhysicalObjectState that sustains itself and reproduces. A BiologicalObjectState may represent the whole life of the object or a temporal part of it." ,
                                                                              "EXAMPLES: a BiologicalObjectState that is not an OrdinaryBiologicalObjectState would be one that survives the replacement of all of its parts, so an example might be my dog (which might be a completely different dog over time)." ,
                                                                              "HQDM state_of_biological_object" ,
                                                                              "USAGE: generally use OrdinaryBiologicalObjectState instead of this class" .


###  http://ontology.asam.net/ontologies/Core#Classification
<http://ontology.asam.net/ontologies/Core#Classification> rdf:type owl:Class ;
                                                          rdfs:subClassOf <http://ontology.asam.net/ontologies/Core#Relationship> ;
                                                          rdfs:comment "DEF: A Relationship where a thing is a member of a class. Basis for object properties memberOf and hasMember." ,
                                                                       "EXAMPLES: not applicable." ,
                                                                       "HQDM classification" ,
                                                                       "USAGE: This class will generally not be used directly in the OpenX domain." .


###  http://ontology.asam.net/ontologies/Core#Composition
<http://ontology.asam.net/ontologies/Core#Composition> rdf:type owl:Class ;
                                                       rdfs:subClassOf <http://ontology.asam.net/ontologies/Core#Aggregation> ;
                                                       rdfs:comment "DEF: An Aggregation where the whole is an arrangement of the parts that results in emergent properties. Basis for object properties partOf and hasPart." ,
                                                                    "EXAMPLES: not applicable." ,
                                                                    "HQDM composition" ,
                                                                    "USAGE: This class will generally not be used directly in the OpenX domain." .


###  http://ontology.asam.net/ontologies/Core#ConnectionRelation
<http://ontology.asam.net/ontologies/Core#ConnectionRelation> rdf:type owl:Class ;
                                                              rdfs:subClassOf <http://ontology.asam.net/ontologies/Core#DefinedRelationship> ;
                                                              rdfs:comment "DEF: A DefinedRelationship for relations between things that are connected in any way, physically or otherwise. Basis for the object property connectedTo." ,
                                                                           "EXAMPLES:" ,
                                                                           "USAGE: Use this class to express a connection between two things as a reified relationship, e.g. in order to specify characteristics such as the angle of the connection." .


###  http://ontology.asam.net/ontologies/Core#CoreConcepts
<http://ontology.asam.net/ontologies/Core#CoreConcepts> rdf:type owl:Class ;
                                                        rdfs:comment "DEF: Top-level container that separates core concepts in the OpenXOntology. The CoreConcepts define basic concepts, such as physical objects, states, and events. The core ontology of ASAM OpenXOntology corresponds to a top-level ontology or upper ontology. The core ontology of ASAM OpenXOntology is based on HQDM." .


###  http://ontology.asam.net/ontologies/Core#DefinedRelationship
<http://ontology.asam.net/ontologies/Core#DefinedRelationship> rdf:type owl:Class ;
                                                               rdfs:subClassOf <http://ontology.asam.net/ontologies/Core#Relationship> ;
                                                               rdfs:comment "DEF: A Relationship of a certain kind. This may be temporal, spatial, compositional, or other other relationships." ,
                                                                            "EXAMPLES: not applicable." ,
                                                                            "HQDM defined_relationship" ,
                                                                            "USAGE: This class will generally not be used directly in the OpenX domain." .


###  http://ontology.asam.net/ontologies/Core#DirectionQuantity
<http://ontology.asam.net/ontologies/Core#DirectionQuantity> rdf:type owl:Class ;
                                                             rdfs:subClassOf <http://ontology.asam.net/ontologies/Core#PhysicalQuantity> ;
                                                             rdfs:comment "DEF: A PhysicalQuantity that defines a direction in degrees, between 0 and 360. May be used to quantify the direction of a vector described by a SpatialRelation, a SeparationDistance, or similar." ,
                                                                          "EXAMPLES:" ,
                                                                          "USAGE: Use this class instead of AngleQuantity when specifying actual directions respective to some coordinate system." .


###  http://ontology.asam.net/ontologies/Core#Event
<http://ontology.asam.net/ontologies/Core#Event> rdf:type owl:Class ;
                                                 rdfs:subClassOf <http://ontology.asam.net/ontologies/Core#SpatioTemporalExtent> ,
                                                                 [ rdf:type owl:Restriction ;
                                                                   owl:onProperty <http://ontology.asam.net/ontologies/Core#memberOf> ;
                                                                   owl:allValuesFrom <http://ontology.asam.net/ontologies/Core#SetOfEvents>
                                                                 ] ;
                                                 owl:disjointWith <http://ontology.asam.net/ontologies/Core#State> ;
                                                 rdfs:comment "DEF: A SpatioTemporalExtent with a time extension of zero, but with an extension in space. Events mark changes in states and are used for something instantaneous." ,
                                                              "EXAMPLES:" ,
                                                              "HQDM event" ,
                                                              "USAGE: Use this class to specify the state and/or end of activities and temporal parts of physical objects." .


###  http://ontology.asam.net/ontologies/Core#FunctionalObjectState
<http://ontology.asam.net/ontologies/Core#FunctionalObjectState> rdf:type owl:Class ;
                                                                 rdfs:subClassOf <http://ontology.asam.net/ontologies/Core#IntentionallyConstructedObjectState> ,
                                                                                 <http://ontology.asam.net/ontologies/Core#PhysicalObjectState> ,
                                                                                 [ rdf:type owl:Restriction ;
                                                                                   owl:onProperty <http://ontology.asam.net/ontologies/Core#intendedRole> ;
                                                                                   owl:someValuesFrom <http://ontology.asam.net/ontologies/Core#Role>
                                                                                 ] ;
                                                                 rdfs:comment "DEF: An IntentionallyConstructedObjectState and PhysicalObjectState that has an intendedRole. A FunctionalObjectState may represent the whole life of the object or a temporal part of it." ,
                                                                              "EXAMPLES: a FunctionalObjectState that is not an OrdinaryFunctionalObjectState would be one that survives the replacement of all of its parts, so an example might be my car (which might be a completely different car over time)." ,
                                                                              "HQDM state_of_functional_object" ,
                                                                              "USAGE: generally use OrdinaryFunctionalObjectState instead of this class" .


###  http://ontology.asam.net/ontologies/Core#FunctionalSystemComponentState
<http://ontology.asam.net/ontologies/Core#FunctionalSystemComponentState> rdf:type owl:Class ;
                                                                          rdfs:subClassOf <http://ontology.asam.net/ontologies/Core#FunctionalObjectState> ,
                                                                                          <http://ontology.asam.net/ontologies/Core#SystemComponentState> ,
                                                                                          [ rdf:type owl:Restriction ;
                                                                                            owl:onProperty <http://ontology.asam.net/ontologies/Core#componentOf> ;
                                                                                            owl:qualifiedCardinality "1"^^xsd:nonNegativeInteger ;
                                                                                            owl:onClass <http://ontology.asam.net/ontologies/Core#FunctionalSystemState>
                                                                                          ] ;
                                                                          rdfs:comment "DEF: An IntentionallyConstructedObjectState that represents a replaceable component of a FunctionalSystem. The object property componentOf is used to relate the object to the FunctionalSystem. A FunctionalSystemComponentState may be the whole life of the component or a temporal part of it." ,
                                                                                       "EXAMPLES: markings of road or engines of vehicles" ,
                                                                                       "HQDM state_of_functional_system_component" ,
                                                                                       "USAGE: Use this class to represent the components of things that were created for a specific purpose, for example markings of road or engines of vehicles." .


###  http://ontology.asam.net/ontologies/Core#FunctionalSystemState
<http://ontology.asam.net/ontologies/Core#FunctionalSystemState> rdf:type owl:Class ;
                                                                 rdfs:subClassOf <http://ontology.asam.net/ontologies/Core#OrdinaryFunctionalObjectState> ,
                                                                                 <http://ontology.asam.net/ontologies/Core#SystemState> ;
                                                                 rdfs:comment "DEF: An OrdinaryFunctionalObjectState that is also a SystemState." ,
                                                                              "EXAMPLES: Vehicles, traffic infrastructure, buildings, traffic lights." ,
                                                                              "HQDM state_of_functional_system" ,
                                                                              "USAGE: Use this class for describing (temporal parts) of concrete (actual, materialized) systems that cease to exist when all of their parts are removed.  Often combined with OrdinaryBiologicalObjectState or OrdinaryFunctionalObjectState" .


###  http://ontology.asam.net/ontologies/Core#Geometry
<http://ontology.asam.net/ontologies/Core#Geometry> rdf:type owl:Class ;
                                                    rdfs:subClassOf <http://ontology.asam.net/ontologies/Core#PhysicalProperty> ;
                                                    rdfs:comment "DEF: A PhysicalProperty that describes a spatial characteristic of an Object in a 1D, 2D or 3D space. Unlike \"shape\", which only refers to the outer surface, \"geometry\" can include other characteristics, e.g. different kind of projections like cross section, road geometry." ,
                                                                 "EXAMPLES:" ,
                                                                 "USAGE:" .


###  http://ontology.asam.net/ontologies/Core#InstalledFunctionalSystemComponent
<http://ontology.asam.net/ontologies/Core#InstalledFunctionalSystemComponent> rdf:type owl:Class ;
                                                                              rdfs:subClassOf <http://ontology.asam.net/ontologies/Core#FunctionalSystemComponentState> ,
                                                                                              <http://ontology.asam.net/ontologies/Core#InstalledObject> ,
                                                                                              <http://ontology.asam.net/ontologies/Core#OrdinaryFunctionalObjectState> ;
                                                                              rdfs:comment "DEF: An InstalledObject that is also a OrdinaryFunctionalObjectState and a FunctionalSystemComponentState." ,
                                                                                           "EXAMPLES: the particular tire that was installed on car42's right front wheel between time1 and time2" ,
                                                                                           "HQDM installed_functional_system_component" ,
                                                                                           "USAGE: Use this class for describing the actual, materialized installed components of a system." .


###  http://ontology.asam.net/ontologies/Core#InstalledObject
<http://ontology.asam.net/ontologies/Core#InstalledObject> rdf:type owl:Class ;
                                                           rdfs:subClassOf <http://ontology.asam.net/ontologies/Core#OrdinaryPhysicalObjectState> ;
                                                           rdfs:comment "DEF: An OrdinaryPhysicalObjectState that is installed in a system, meaning that is also a SystemComponentState. The state of the ordinary physical object is the temporal part that covers the time from when the ordinary physical object is installed in the system to when it is removed." ,
                                                                        "EXAMPLES: The time that the traffic sign with the serial number 42 is installed at a specific location on highway 66. (note that this would actually be an InstalledFunctionalSystemComponent because the highway is a FunctionalSystem)." ,
                                                                        "HQDM installed_object" ,
                                                                        "USAGE: Use this class to describe the temporal part of a physical object when it is the actual component of a system." .


###  http://ontology.asam.net/ontologies/Core#IntentionallyConstructedActivityState
<http://ontology.asam.net/ontologies/Core#IntentionallyConstructedActivityState> rdf:type owl:Class ;
                                                                                 rdfs:subClassOf <http://ontology.asam.net/ontologies/Core#ActivityState> ,
                                                                                                 <http://ontology.asam.net/ontologies/Core#IntentionallyConstructedObjectState> ;
                                                                                 rdfs:comment "DEF: An ActivityState that is also an IntentionallyConstructedObjectState." ,
                                                                                              "EXAMPLES: the changing of a signal state by a device in an intelligent transportation system" ,
                                                                                              "USAGE: Use this class to describe planned activities by single persons or intelligent devices, such as the changing of a signal state by a device in an intelligent transportation system." .


###  http://ontology.asam.net/ontologies/Core#IntentionallyConstructedObjectState
<http://ontology.asam.net/ontologies/Core#IntentionallyConstructedObjectState> rdf:type owl:Class ;
                                                                               rdfs:subClassOf <http://ontology.asam.net/ontologies/Core#State> ;
                                                                               rdfs:comment "DEF: A State that exists because of an act of will or agreement. That means that IntentionallyConstructedObjects are constructed intentionally by one or more things that have intent, usually humans or robots." ,
                                                                                            "EXAMPLES: an idea, a design, or a component specification" ,
                                                                                            "HQDM state_of_intentionally_constructed_object" ,
                                                                                            "USAGE: Generally use FunctionalObjectState or one of its subclasses rather than this class. However, a thing that was created by humans for some purpose but does not exist materially, such as an idea, a design, or a component specification, would be a IntentionallyConstructedObjectState but not a FunctionalObjectState." .


###  http://ontology.asam.net/ontologies/Core#LengthQuantity
<http://ontology.asam.net/ontologies/Core#LengthQuantity> rdf:type owl:Class ;
                                                          rdfs:subClassOf <http://ontology.asam.net/ontologies/Core#PhysicalQuantity> ;
                                                          rdfs:comment "DEF: A PhysicalQuantity that is a length value in meters." ,
                                                                       "EXAMPLES:" ,
                                                                       "USAGE:" .


###  http://ontology.asam.net/ontologies/Core#OrdinaryBiologicalObjectState
<http://ontology.asam.net/ontologies/Core#OrdinaryBiologicalObjectState> rdf:type owl:Class ;
                                                                         rdfs:subClassOf <http://ontology.asam.net/ontologies/Core#BiologicalObjectState> ,
                                                                                         <http://ontology.asam.net/ontologies/Core#OrdinaryPhysicalObjectState> ;
                                                                         rdfs:comment "DEF: A BiologicalObjectState that describes biological objects that do not survive changing all their parts at once.  An OrdinaryBiologicalObjectState may represent the whole life of the object or a temporal part of it." ,
                                                                                      "EXAMPLES: humans, animals, and trees" ,
                                                                                      "HQDM state_of_ordinary_biological_object" ,
                                                                                      "USAGE: Use this class for describing temporal parts of living things that cease to exist when all of their parts are removed." .


###  http://ontology.asam.net/ontologies/Core#OrdinaryFunctionalObjectState
<http://ontology.asam.net/ontologies/Core#OrdinaryFunctionalObjectState> rdf:type owl:Class ;
                                                                         rdfs:subClassOf <http://ontology.asam.net/ontologies/Core#FunctionalObjectState> ,
                                                                                         <http://ontology.asam.net/ontologies/Core#OrdinaryPhysicalObjectState> ;
                                                                         rdfs:comment "DEF: A FunctionalObjectState that describes functional objects that do not survive changing all their parts at once.  An OrdinaryFunctionalObjectState may represent the whole life of the object or a temporal part of it." ,
                                                                                      "EXAMPLES: A steel bar with no components and is not a component of any other thing but was created for a specific purpose could be an OrdinaryFunctionalObjectState." ,
                                                                                      "HQDM state_of_ordinary_functional_object" ,
                                                                                      "USAGE: Use this class for temporal parts of manufactured things that were constructed for some purpose and that cease to exist when all of their parts are removed.  However, if the thing is a system and/or a system component, it is preferable to use the corresponding subclass." .


###  http://ontology.asam.net/ontologies/Core#OrdinaryPhysicalObjectState
<http://ontology.asam.net/ontologies/Core#OrdinaryPhysicalObjectState> rdf:type owl:Class ;
                                                                       rdfs:subClassOf <http://ontology.asam.net/ontologies/Core#PhysicalObjectState> ;
                                                                       rdfs:comment "DEF: A PhysicalObjectState that describes physical objects that do not survive changing all their parts at once.  An OrdinaryPhysicalObjectState may represent the whole life of the object or a temporal part of it." ,
                                                                                    "EXAMPLES: cloud, raindrop, rock, sunlight" ,
                                                                                    "HQDM state_of_ordinary_physical_object" ,
                                                                                    "USAGE: Use this class for temporal parts of physical objects that cease to exist when all of their parts are removed and that are neither biological objects (OrdinaryBiologicalObjectState) nor manufactured things constructed for some purpose (OrdinaryFunctionalObjectState)." .


###  http://ontology.asam.net/ontologies/Core#Participant
<http://ontology.asam.net/ontologies/Core#Participant> rdf:type owl:Class ;
                                                       rdfs:subClassOf <http://ontology.asam.net/ontologies/Core#PhysicalObjectState> ,
                                                                       [ rdf:type owl:Restriction ;
                                                                         owl:onProperty <http://ontology.asam.net/ontologies/Core#memberOf> ;
                                                                         owl:allValuesFrom <http://ontology.asam.net/ontologies/Core#SetOfParticipants>
                                                                       ] ,
                                                                       [ rdf:type owl:Restriction ;
                                                                         owl:onProperty <http://ontology.asam.net/ontologies/Core#participantOf> ;
                                                                         owl:allValuesFrom <http://ontology.asam.net/ontologies/Core#ActivityState>
                                                                       ] ;
                                                       rdfs:comment "DEF: A PhysicalObjectState that represents a participant of an ActivityState. The ActivityState consists of these Participants, where each Participant is a member of the Role in which it is participating." ,
                                                                    "EXAMPLES: The state (temporal part) of a vehicle that is making a left turn." ,
                                                                    "HQDM participant" ,
                                                                    "USAGE: Use this class for describing the temporal part of physical objects that are participating in activities.  Usually combined with OrdinaryBiologicalObjectState or OrdinaryFunctionalObjectState" .


###  http://ontology.asam.net/ontologies/Core#PeriodOfTime
<http://ontology.asam.net/ontologies/Core#PeriodOfTime> rdf:type owl:Class ;
                                                        rdfs:subClassOf <http://ontology.asam.net/ontologies/Core#State> ,
                                                                        [ rdf:type owl:Restriction ;
                                                                          owl:onProperty <http://ontology.asam.net/ontologies/Core#temporalPartOf> ;
                                                                          owl:allValuesFrom <http://ontology.asam.net/ontologies/Core#PossibleWorld>
                                                                        ] ;
                                                        rdfs:comment "DEF: A State that is a temporal part of some PossibleWorld. That means the period of time is a temporal duration of some possible world, which could be the actual world." ,
                                                                     "EXAMPLES:" ,
                                                                     "HQDM period_of_time" ,
                                                                     "USAGE:" .


###  http://ontology.asam.net/ontologies/Core#PhysicalObjectState
<http://ontology.asam.net/ontologies/Core#PhysicalObjectState> rdf:type owl:Class ;
                                                               rdfs:subClassOf <http://ontology.asam.net/ontologies/Core#State> ,
                                                                               [ rdf:type owl:Restriction ;
                                                                                 owl:onProperty <http://ontology.asam.net/ontologies/Core#memberOf> ;
                                                                                 owl:allValuesFrom <http://ontology.asam.net/ontologies/Core#SetOfPhysicalObjectStates>
                                                                               ] ,
                                                                               [ rdf:type owl:Restriction ;
                                                                                 owl:onProperty <http://ontology.asam.net/ontologies/Core#temporalPartOf> ;
                                                                                 owl:allValuesFrom <http://ontology.asam.net/ontologies/Core#WholeLifePhysicalObject>
                                                                               ] ;
                                                               rdfs:comment "DEF: A State that consists of a distribution of matter and/or energy. A PhysicalObjectState is understood to have a bounded distribution, and so it can be identified as that parcel of matter and/or energy over time.  A PhysicalObjectState can be thought of as characterizing what does not change over time of a State." ,
                                                                            "EXAMPLES:" ,
                                                                            "HQDM state_of_physical_object" ,
                                                                            "USAGE: Generally use a subclass of this class." .


###  http://ontology.asam.net/ontologies/Core#PhysicalProperty
<http://ontology.asam.net/ontologies/Core#PhysicalProperty> rdf:type owl:Class ;
                                                            rdfs:subClassOf <http://ontology.asam.net/ontologies/Core#SetOfStates> ;
                                                            rdfs:comment "DEF: A SetOfStates is some characteristic that is the same for each state that possesses it (is a memberOf it). More accurately, a PhysicalProperty is a Set that groups states by a specific characteristic, but PhysicalProperty is understood to be the specific characteristic shared by its members." ,
                                                                         "EXAMPLES: The color red is a PhysicalProperty." ,
                                                                         "HQDM physical_property" ,
                                                                         "USAGE: Use this class for physical properties of both physical objects, for example mass and length, and activities, for example speed and duration." .


###  http://ontology.asam.net/ontologies/Core#PhysicalQuantity
<http://ontology.asam.net/ontologies/Core#PhysicalQuantity> rdf:type owl:Class ;
                                                            rdfs:subClassOf <http://ontology.asam.net/ontologies/Core#PhysicalProperty> ;
                                                            rdfs:comment "DEF: A PhysicalProperty that represents a measurable quantity of a characteristic. " ,
                                                                         "EXAMPLES: length, speed, and angle." ,
                                                                         "HQDM physical_quantity" ,
                                                                         "USAGE:" .


###  http://ontology.asam.net/ontologies/Core#PointInTime
<http://ontology.asam.net/ontologies/Core#PointInTime> rdf:type owl:Class ;
                                                       rdfs:subClassOf <http://ontology.asam.net/ontologies/Core#Event> ;
                                                       rdfs:comment "DEF: An Event that is the whole of space at an instant from some viewpoint." ,
                                                                    "EXAMPLES:" ,
                                                                    "HQDM point_in_time" ,
                                                                    "USAGE:" .


###  http://ontology.asam.net/ontologies/Core#PossibleWorld
<http://ontology.asam.net/ontologies/Core#PossibleWorld> rdf:type owl:Class ;
                                                         rdfs:subClassOf <http://ontology.asam.net/ontologies/Core#PeriodOfTime> ,
                                                                         <http://ontology.asam.net/ontologies/Core#WholeLifeIndividual> ;
                                                         rdfs:comment "DEF: A WholeLifeIndividual that is a complete spatio-temporal history of some possible world. The actual world is one of the possible worlds." ,
                                                                      "EXAMPLES: a description could contain two PossibleWorlds, the possible world where carA stopped at the pedestrian crossing and where carA did not stop. " ,
                                                                      "HQDM possible_world" ,
                                                                      "USAGE: Use this class to model modality (modal realism rather than modal logic), such as several possible planned futures or alternative pasts. " .


###  http://ontology.asam.net/ontologies/Core#Relationship
<http://ontology.asam.net/ontologies/Core#Relationship> rdf:type owl:Class ;
                                                        rdfs:subClassOf <http://ontology.asam.net/ontologies/Core#AbstractObject> ;
                                                        rdfs:comment "DEF: Relationships form the basis for many object properties." ,
                                                                     "EXAMPLES: not applicable." ,
                                                                     "HQDM relationship" ,
                                                                     "USAGE: This class will generally not be used directly in the OpenX domain." .


###  http://ontology.asam.net/ontologies/Core#RelativeLocation
<http://ontology.asam.net/ontologies/Core#RelativeLocation> rdf:type owl:Class ;
                                                            rdfs:subClassOf <http://ontology.asam.net/ontologies/Core#SpatialRelation> ;
                                                            rdfs:comment "DEF: A SpatialRelation that describes that the subject is located on the object. Basis for the object property locatedOn." ,
                                                                         "EXAMPLES:" ,
                                                                         "USAGE: Use this class to express the location of one thing with respect to another as a reified relationship, e.g. in order to specify characteristics such as the precise position of location." .


###  http://ontology.asam.net/ontologies/Core#Role
<http://ontology.asam.net/ontologies/Core#Role> rdf:type owl:Class ;
                                                rdfs:subClassOf <http://ontology.asam.net/ontologies/Core#SetOfParticipants> ;
                                                rdfs:comment "DEF: A SetOfParticipants where each member participates in the same way in an ActivityState. In HQDM, a role is a kind of participant.  So subclasses of Participant are members of the class Role, including TrafficParticipant, Owner, Employer, and Asset." ,
                                                             "EXAMPLES: subclasses of Participant, including TrafficParticipant, Owner, Employer, and Asset" ,
                                                             "HQDM role" ,
                                                             "USAGE:" .


###  http://ontology.asam.net/ontologies/Core#SeparationDistance
<http://ontology.asam.net/ontologies/Core#SeparationDistance> rdf:type owl:Class ;
                                                              rdfs:subClassOf <http://ontology.asam.net/ontologies/Core#SpatialRelation> ,
                                                                              [ rdf:type owl:Restriction ;
                                                                                owl:onProperty <http://ontology.asam.net/ontologies/Core#hasDistance> ;
                                                                                owl:someValuesFrom <http://ontology.asam.net/ontologies/Core#LengthQuantity>
                                                                              ] ;
                                                              rdfs:comment "DEF: A SpatialRelation that also describes a distance between two connected objects. Gives a complete description of a vector and an exact relative position." ,
                                                                           "EXAMPLES:" ,
                                                                           "USAGE: Use this class to express the separation distance between two things as a reified relationship, e.g. in order to specify characteristics such as the distance and direction of the separation." .


###  http://ontology.asam.net/ontologies/Core#Set
<http://ontology.asam.net/ontologies/Core#Set> rdf:type owl:Class ;
                                               rdfs:subClassOf <http://ontology.asam.net/ontologies/Core#AbstractObject> ;
                                               rdfs:comment "DEF: An AbstractObject that has members and whose identity is defined by those members. The members may be other sets as well as specific spatio-temporal extents." ,
                                                            "EXAMPLES: not applicable." ,
                                                            "HQDM class" ,
                                                            "USAGE: This class will generally not be used directly in the OpenX domain." .


###  http://ontology.asam.net/ontologies/Core#SetOfActivityStates
<http://ontology.asam.net/ontologies/Core#SetOfActivityStates> rdf:type owl:Class ;
                                                               rdfs:subClassOf <http://ontology.asam.net/ontologies/Core#SetOfStates> ;
                                                               rdfs:comment "DEF: A SetOfStates that groups activities." ,
                                                                            "EXAMPLES:" ,
                                                                            "HQDM class_of_state_of_activity" ,
                                                                            "USAGE: Use this class to describe specific sets or kinds of ActivityStates that are not available already as subclasses of ActivityState." .


###  http://ontology.asam.net/ontologies/Core#SetOfEvents
<http://ontology.asam.net/ontologies/Core#SetOfEvents> rdf:type owl:Class ;
                                                       rdfs:subClassOf <http://ontology.asam.net/ontologies/Core#SetOfSpatioTemporalExtents> ;
                                                       rdfs:comment "DEF: A SetOfSpatioTemporalExtents that groups kinds of events. " ,
                                                                    "EXAMPLES: triggered and absolute events, start and end events, etc." ,
                                                                    "HQDM class_of_event" ,
                                                                    "USAGE: Use this class to describe specific sets or kinds of Events that are not available already as subclasses of Event." .


###  http://ontology.asam.net/ontologies/Core#SetOfParticipants
<http://ontology.asam.net/ontologies/Core#SetOfParticipants> rdf:type owl:Class ;
                                                             rdfs:subClassOf <http://ontology.asam.net/ontologies/Core#SetOfPhysicalObjectStates> ;
                                                             rdfs:comment "DEF: A SetOfPhysicalObjectStates that groups participants of activities." ,
                                                                          "EXAMPLES:" ,
                                                                          "HQDM class_of_participant" ,
                                                                          "USAGE: Generally use Role rather than this class." .


###  http://ontology.asam.net/ontologies/Core#SetOfPhysicalObjectStates
<http://ontology.asam.net/ontologies/Core#SetOfPhysicalObjectStates> rdf:type owl:Class ;
                                                                     rdfs:subClassOf <http://ontology.asam.net/ontologies/Core#SetOfStates> ;
                                                                     rdfs:comment "DEF: A SetOfStates that groups physical object states." ,
                                                                                  "EXAMPLES:" ,
                                                                                  "HQDM class_of_state_of_physical_object_state" ,
                                                                                  "USAGE: Use this class to describe specific sets or kinds of PhysicalObjectStates that are not available already as subclasses of PhysicalObjectState." .


###  http://ontology.asam.net/ontologies/Core#SetOfSpatioTemporalExtents
<http://ontology.asam.net/ontologies/Core#SetOfSpatioTemporalExtents> rdf:type owl:Class ;
                                                                      rdfs:subClassOf <http://ontology.asam.net/ontologies/Core#Set> ;
                                                                      rdfs:comment "DEF: A Set whose members are spatio-temporal extents." ,
                                                                                   "EXAMPLES:" ,
                                                                                   "HQDM class_of_spatio_temporal_extent" ,
                                                                                   "USAGE: Use this class to describe specific sets or kinds of SpatioTemporalExtents that are not available already as subclasses of SpatioTemporalExtent." .


###  http://ontology.asam.net/ontologies/Core#SetOfStates
<http://ontology.asam.net/ontologies/Core#SetOfStates> rdf:type owl:Class ;
                                                       rdfs:subClassOf <http://ontology.asam.net/ontologies/Core#SetOfSpatioTemporalExtents> ;
                                                       rdfs:comment "DEF: A SetOfSpatioTemporalExtents that groups states." ,
                                                                    "EXAMPLES:" ,
                                                                    "HQDM class_of_state" ,
                                                                    "USAGE: Use this class to describe specific sets or kinds of States that are not available already as subclasses of State." .


###  http://ontology.asam.net/ontologies/Core#SetOfWholeLifeIndividuals
<http://ontology.asam.net/ontologies/Core#SetOfWholeLifeIndividuals> rdf:type owl:Class ;
                                                                     rdfs:subClassOf <http://ontology.asam.net/ontologies/Core#SetOfStates> ;
                                                                     rdfs:comment "DEF: A SetOfStates that groups whole-life individuals." ,
                                                                                  "EXAMPLES:" ,
                                                                                  "HQDM class_of_individual" ,
                                                                                  "USAGE: Use this class to describe specific sets or kinds of WholeLifeIndividuals that are not available already as subclasses of WholeLifeIndividual." .


###  http://ontology.asam.net/ontologies/Core#SociallyConstructedActivityState
<http://ontology.asam.net/ontologies/Core#SociallyConstructedActivityState> rdf:type owl:Class ;
                                                                            rdfs:subClassOf <http://ontology.asam.net/ontologies/Core#IntentionallyConstructedActivityState> ,
                                                                                            <http://ontology.asam.net/ontologies/Core#SociallyConstructedObjectState> ;
                                                                            rdfs:comment "DEF: An ActivityState that is also a SociallyConstructedObjectState." ,
                                                                                         "EXAMPLES: planned activities between multiple people such as meetings; the coordination of multiple traffic signals in an intelligent transportation system." ,
                                                                                         "HQDM state_of_socially_constructed_activity" ,
                                                                                         "USAGE: Use this class to describe planned activities by a group of persons or intelligent devices." .


###  http://ontology.asam.net/ontologies/Core#SociallyConstructedObjectState
<http://ontology.asam.net/ontologies/Core#SociallyConstructedObjectState> rdf:type owl:Class ;
                                                                          rdfs:subClassOf <http://ontology.asam.net/ontologies/Core#IntentionallyConstructedObjectState> ;
                                                                          rdfs:comment "DEF: An IntentionallyConstructedObjectState that is necessarily constructed by agreement of or acceptance by many people." ,
                                                                                       "EXAMPLES: contracts, companies, and money" ,
                                                                                       "HQDM state_of_socially_constructed_object" ,
                                                                                       "USAGE:" .


###  http://ontology.asam.net/ontologies/Core#SpatialConnection
<http://ontology.asam.net/ontologies/Core#SpatialConnection> rdf:type owl:Class ;
                                                             rdfs:subClassOf <http://ontology.asam.net/ontologies/Core#ConnectionRelation> ,
                                                                             <http://ontology.asam.net/ontologies/Core#SpatialRelation> ;
                                                             rdfs:comment "DEF: A ConnectionRelation for relations between things that touch. Spatial connections create bridges for the transfer of energy or other things between the objects. Basis for the object property connectedTo." ,
                                                                          "EXAMPLES:" ,
                                                                          "USAGE: Use this class to express a spatial connection between two things as a reified relationship, e.g. in order to specify characteristics such as the surface area of the connecting surface." .


###  http://ontology.asam.net/ontologies/Core#SpatialLocation
<http://ontology.asam.net/ontologies/Core#SpatialLocation> rdf:type owl:Class ;
                                                           rdfs:subClassOf <http://ontology.asam.net/ontologies/Core#State> ;
                                                           rdfs:comment "DEF: A State that describes the relative continuity of a position, an area or a space that is important in a defined context. The type of description of a SpatialLocation can be topological, topographical, coordinates, or any other type." ,
                                                                        "EXAMPLES: the position of an object, a country where certain regulations apply." ,
                                                                        "USAGE:" .


###  http://ontology.asam.net/ontologies/Core#SpatialRelation
<http://ontology.asam.net/ontologies/Core#SpatialRelation> rdf:type owl:Class ;
                                                           rdfs:subClassOf <http://ontology.asam.net/ontologies/Core#DefinedRelationship> ,
                                                                           [ rdf:type owl:Restriction ;
                                                                             owl:onProperty <http://ontology.asam.net/ontologies/Core#hasRelationDirection> ;
                                                                             owl:someValuesFrom <http://ontology.asam.net/ontologies/Core#DirectionQuantity>
                                                                           ] ,
                                                                           [ rdf:type owl:Restriction ;
                                                                             owl:onProperty <http://ontology.asam.net/ontologies/Core#hasSpatialObject> ;
                                                                             owl:someValuesFrom <http://ontology.asam.net/ontologies/Core#PhysicalObjectState>
                                                                           ] ,
                                                                           [ rdf:type owl:Restriction ;
                                                                             owl:onProperty <http://ontology.asam.net/ontologies/Core#hasSpatialSubject> ;
                                                                             owl:someValuesFrom <http://ontology.asam.net/ontologies/Core#PhysicalObjectState>
                                                                           ] ;
                                                           owl:disjointWith <http://ontology.asam.net/ontologies/Core#TemporalRelation> ;
                                                           rdfs:comment "DEF: A DefinedRelationship between two physical objects that describes their directional relationship, not the distance. Basis for object properties such as rightOf, leftOf, inFrontOf, behind, etc." ,
                                                                        "EXAMPLES:" ,
                                                                        "USAGE: Use this class to express a general spatial relation between two things as a reified relationship, giving only the direction of the relationship." .


###  http://ontology.asam.net/ontologies/Core#SpatioTemporalExtent
<http://ontology.asam.net/ontologies/Core#SpatioTemporalExtent> rdf:type owl:Class ;
                                                                rdfs:subClassOf <http://ontology.asam.net/ontologies/Core#CoreConcepts> ,
                                                                                [ rdf:type owl:Restriction ;
                                                                                  owl:onProperty <http://ontology.asam.net/ontologies/Core#partOfPossibleWorld> ;
                                                                                  owl:someValuesFrom <http://ontology.asam.net/ontologies/Core#PossibleWorld>
                                                                                ] ,
                                                                                [ rdf:type owl:Restriction ;
                                                                                  owl:onProperty <http://ontology.asam.net/ontologies/Core#memberOf> ;
                                                                                  owl:allValuesFrom <http://ontology.asam.net/ontologies/Core#SetOfSpatioTemporalExtents>
                                                                                ] ,
                                                                                [ rdf:type owl:Restriction ;
                                                                                  owl:onProperty <http://ontology.asam.net/ontologies/Core#hasBeginning> ;
                                                                                  owl:qualifiedCardinality "1"^^xsd:nonNegativeInteger ;
                                                                                  owl:onClass <http://ontology.asam.net/ontologies/Core#Event>
                                                                                ] ,
                                                                                [ rdf:type owl:Restriction ;
                                                                                  owl:onProperty <http://ontology.asam.net/ontologies/Core#hasEnding> ;
                                                                                  owl:qualifiedCardinality "1"^^xsd:nonNegativeInteger ;
                                                                                  owl:onClass <http://ontology.asam.net/ontologies/Core#Event>
                                                                                ] ;
                                                                rdfs:comment "DEF: A thing that exists in time and space, meaning in four dimensions. Each spatio-temporal extent has a start event and an end event." ,
                                                                             "EXAMPLES: not applicable." ,
                                                                             "HQDM spatio_temporal_extent" ,
                                                                             "USAGE: This class will generally not be used directly in the OpenX domain." .


###  http://ontology.asam.net/ontologies/Core#SpeedQuantity
<http://ontology.asam.net/ontologies/Core#SpeedQuantity> rdf:type owl:Class ;
                                                         rdfs:subClassOf <http://ontology.asam.net/ontologies/Core#PhysicalQuantity> ;
                                                         rdfs:comment "DEF: A PhysicalQuantity that is a speed value in meters per second." ,
                                                                      "EXAMPLES:" ,
                                                                      "USAGE:" .


###  http://ontology.asam.net/ontologies/Core#State
<http://ontology.asam.net/ontologies/Core#State> rdf:type owl:Class ;
                                                 rdfs:subClassOf <http://ontology.asam.net/ontologies/Core#SpatioTemporalExtent> ,
                                                                 [ rdf:type owl:Restriction ;
                                                                   owl:onProperty <http://ontology.asam.net/ontologies/Core#temporalPartOf> ;
                                                                   owl:someValuesFrom <http://ontology.asam.net/ontologies/Core#WholeLifeIndividual>
                                                                 ] ,
                                                                 [ rdf:type owl:Restriction ;
                                                                   owl:onProperty <http://ontology.asam.net/ontologies/Core#memberOf> ;
                                                                   owl:allValuesFrom <http://ontology.asam.net/ontologies/Core#SetOfStates>
                                                                 ] ;
                                                 rdfs:comment "DEF: A SpatioTemporalExtent with non-zero extension in both space and time. Used to describe, for example, the state of a vehicle, a person, or a manufactured system like a factory. States can apply to the whole life of a thing or represent temporal parts of a thing," ,
                                                              "EXAMPLES:" ,
                                                              "HQDM state" ,
                                                              "USAGE: Use this class to describe the temporal part of a whole-life individual to which some property applies or to describe the temporal part of a whole-life individual that participates in an activity." .


###  http://ontology.asam.net/ontologies/Core#SystemComponentState
<http://ontology.asam.net/ontologies/Core#SystemComponentState> rdf:type owl:Class ;
                                                                rdfs:subClassOf <http://ontology.asam.net/ontologies/Core#PhysicalObjectState> ,
                                                                                [ rdf:type owl:Restriction ;
                                                                                  owl:onProperty <http://ontology.asam.net/ontologies/Core#componentOf> ;
                                                                                  owl:qualifiedCardinality "1"^^xsd:nonNegativeInteger ;
                                                                                  owl:onClass <http://ontology.asam.net/ontologies/Core#SystemState>
                                                                                ] ;
                                                                rdfs:comment "DEF: A PhysicalObjectState that represents a component of a system. The state may represent the whole life of the component or a temporal part of it. The state can be completely replaced without losing its identity. A SystemComponentState can only exist when the System exists.  On the other hand, the OrdinaryPhysicalObject that is installed as the component may exist before or after the System." ,
                                                                             "EXAMPLES: vehicles and pedestrians are components of the traffic system (actually FunctionalSystemComponentStates - not WholeLifeIndividuals because the whole life of a vehicle or pedestrian would include temporal parts that are not components of the same traffic system)" ,
                                                                             "HQDM state_of_system_component" ,
                                                                             "USAGE: Use this class only for physical objects that are components of systems that do not have specific functions (are not FunctionalSystems)" .


###  http://ontology.asam.net/ontologies/Core#SystemState
<http://ontology.asam.net/ontologies/Core#SystemState> rdf:type owl:Class ;
                                                       rdfs:subClassOf <http://ontology.asam.net/ontologies/Core#OrdinaryPhysicalObjectState> ;
                                                       rdfs:comment "DEF: An OrdinaryPhysicalObjectState that represents a concrete materialized system. Systems are defined as an organized or connected group of physical objects. A SystemState may represent the whole life of the system or a temporal part of it." ,
                                                                    "EXAMPLES: A natural weather system." ,
                                                                    "HQDM state_of_system" ,
                                                                    "USAGE: Use this class only for systems that do not have specific functions" .


###  http://ontology.asam.net/ontologies/Core#TemporalComposition
<http://ontology.asam.net/ontologies/Core#TemporalComposition> rdf:type owl:Class ;
                                                               rdfs:subClassOf <http://ontology.asam.net/ontologies/Core#Composition> ;
                                                               rdfs:comment "DEF: A Composition where the part is the entire whole spatially, but part of the whole temporally." ,
                                                                            "EXAMPLES: not applicable." ,
                                                                            "USAGE: This class will generally not be used directly in the OpenX domain." .


###  http://ontology.asam.net/ontologies/Core#TemporalRelation
<http://ontology.asam.net/ontologies/Core#TemporalRelation> rdf:type owl:Class ;
                                                            rdfs:subClassOf <http://ontology.asam.net/ontologies/Core#DefinedRelationship> ;
                                                            rdfs:comment "DEF: A DefinedRelationship that describes a temporal relationship between two things, usually between events. Basis for the object properties occursBefore, occursAfter, and similar." ,
                                                                         "EXAMPLES: not applicable." ,
                                                                         "USAGE: This class will generally not be used directly in the OpenX domain." .


###  http://ontology.asam.net/ontologies/Core#WholeLifeActivity
<http://ontology.asam.net/ontologies/Core#WholeLifeActivity> rdf:type owl:Class ;
                                                             rdfs:subClassOf <http://ontology.asam.net/ontologies/Core#ActivityState> ,
                                                                             <http://ontology.asam.net/ontologies/Core#WholeLifeIndividual> ;
                                                             rdfs:comment "DEF: An ActivityState that represents the whole life of the activity." ,
                                                                          "EXAMPLES: the entire activity of overtaking another vehicle." ,
                                                                          "HQDM activity" ,
                                                                          "USAGE: Use this class for an activity that is its temporal whole." .


###  http://ontology.asam.net/ontologies/Core#WholeLifeBiologicalObject
<http://ontology.asam.net/ontologies/Core#WholeLifeBiologicalObject> rdf:type owl:Class ;
                                                                     rdfs:subClassOf <http://ontology.asam.net/ontologies/Core#BiologicalObjectState> ,
                                                                                     <http://ontology.asam.net/ontologies/Core#WholeLifePhysicalObject> ;
                                                                     rdfs:comment "DEF: A BiologicalObjectState that represents the whole life of the biological object." ,
                                                                                  "EXAMPLES: a person from their birth to their death." ,
                                                                                  "HQDM biological_object" ,
                                                                                  "USAGE: Use this class for a biological object that is its temporal whole. Note that usually it is preferable to use the subclass WholeLifeOrdinaryBiologicalObject." .


###  http://ontology.asam.net/ontologies/Core#WholeLifeFunctionalObject
<http://ontology.asam.net/ontologies/Core#WholeLifeFunctionalObject> rdf:type owl:Class ;
                                                                     rdfs:subClassOf <http://ontology.asam.net/ontologies/Core#FunctionalObjectState> ,
                                                                                     <http://ontology.asam.net/ontologies/Core#WholeLifePhysicalObject> ;
                                                                     rdfs:comment "DEF: A FunctionalObjectState that represents the whole life of the functional object." ,
                                                                                  "EXAMPLES: " ,
                                                                                  "HQDM functional_object" ,
                                                                                  "USAGE: Use this class for a functional object that is its temporal whole. Note that usually it is preferable to use the subclass WholeLifeOrdinaryFunctionalObject." .


###  http://ontology.asam.net/ontologies/Core#WholeLifeFunctionalSystem
<http://ontology.asam.net/ontologies/Core#WholeLifeFunctionalSystem> rdf:type owl:Class ;
                                                                     rdfs:subClassOf <http://ontology.asam.net/ontologies/Core#FunctionalSystemState> ,
                                                                                     <http://ontology.asam.net/ontologies/Core#WholeLifeSystem> ;
                                                                     rdfs:comment "DEF: A FunctionalSystemState that represents the whole life of the functional system." ,
                                                                                  "EXAMPLES: A vehicle from when it is manufactured to when it is destroyed." ,
                                                                                  "HQDM functional_system" ,
                                                                                  "USAGE: Use this class for describing individual concrete (actual, materialized) systems that cease to exist when all of their parts are removed.  Often combined with WholeLifeOrdinaryBiologicalObject or WholeLifeOrdinaryFunctionalObject" .


###  http://ontology.asam.net/ontologies/Core#WholeLifeFunctionalSystemComponent
<http://ontology.asam.net/ontologies/Core#WholeLifeFunctionalSystemComponent> rdf:type owl:Class ;
                                                                              rdfs:subClassOf <http://ontology.asam.net/ontologies/Core#FunctionalSystemComponentState> ,
                                                                                              <http://ontology.asam.net/ontologies/Core#WholeLifeSystemComponent> ,
                                                                                              [ rdf:type owl:Restriction ;
                                                                                                owl:onProperty <http://ontology.asam.net/ontologies/Core#componentOf> ;
                                                                                                owl:qualifiedCardinality "1"^^xsd:nonNegativeInteger ;
                                                                                                owl:onClass <http://ontology.asam.net/ontologies/Core#WholeLifeFunctionalSystem>
                                                                                              ] ;
                                                                              rdfs:comment "DEF: A FunctionalSystemComponentState that represents the whole life of the functional system component." ,
                                                                                           "EXAMPLES: The component of a junction that is the a traffic light, which functions as a signal at a junction (not the individual traffic lights with their serial numbers and dates of production, but the traffic light as a functional component)." ,
                                                                                           "HQDM functional_system_component" ,
                                                                                           "USAGE: Use this class to specify the whole life of a component of a functional system, which could be temporally divided into FunctionalSystemComponentStates for each of the InstalledObjects that acted as the component over the lifetime of the functional system." .


###  http://ontology.asam.net/ontologies/Core#WholeLifeIndividual
<http://ontology.asam.net/ontologies/Core#WholeLifeIndividual> rdf:type owl:Class ;
                                                               rdfs:subClassOf <http://ontology.asam.net/ontologies/Core#State> ;
                                                               rdfs:comment "DEF: A State that is not a proper temporalPartOf any other individual of the same kind." ,
                                                                            "EXAMPLES:" ,
                                                                            "HQDM individual" ,
                                                                            "USAGE: Use this class in combination with others to designate that a particular spatio-temporal extent is \"its whole life\"" .


###  http://ontology.asam.net/ontologies/Core#WholeLifeIntentionallyConstructedActivity
<http://ontology.asam.net/ontologies/Core#WholeLifeIntentionallyConstructedActivity> rdf:type owl:Class ;
                                                                                     rdfs:subClassOf <http://ontology.asam.net/ontologies/Core#IntentionallyConstructedActivityState> ,
                                                                                                     <http://ontology.asam.net/ontologies/Core#WholeLifeActivity> ;
                                                                                     rdfs:comment "DEF: A WholeLifeIntentionallyConstructedObject that is also a WholeLifeActivity." ,
                                                                                                  "EXAMPLES:" ,
                                                                                                  "USAGE:" ,
                                                                                                  "USAGE: Use this class for an intentional constructed activity that is its temporal whole." .


###  http://ontology.asam.net/ontologies/Core#WholeLifeIntentionallyConstructedObject
<http://ontology.asam.net/ontologies/Core#WholeLifeIntentionallyConstructedObject> rdf:type owl:Class ;
                                                                                   rdfs:subClassOf <http://ontology.asam.net/ontologies/Core#IntentionallyConstructedObjectState> ,
                                                                                                   <http://ontology.asam.net/ontologies/Core#WholeLifeIndividual> ;
                                                                                   rdfs:comment "DEF: An IntentionallyConstructedObjectState that represents the whole life of the intentionally constructed object." ,
                                                                                                "EXAMPLES:" ,
                                                                                                "HQDM intentionally_constructed_object" ,
                                                                                                "USAGE: Use this class for an intentionally constructed object that is its temporal whole. Note that usually it is preferable to use one of the subclasses." .


###  http://ontology.asam.net/ontologies/Core#WholeLifeOrdinaryBiologicalObject
<http://ontology.asam.net/ontologies/Core#WholeLifeOrdinaryBiologicalObject> rdf:type owl:Class ;
                                                                             rdfs:subClassOf <http://ontology.asam.net/ontologies/Core#OrdinaryBiologicalObjectState> ,
                                                                                             <http://ontology.asam.net/ontologies/Core#WholeLifeBiologicalObject> ;
                                                                             rdfs:comment "DEF: An OrdinaryBiologicalObjectState that represents the whole life of the ordinary biological object." ,
                                                                                          "EXAMPLES: a particular person from the instant that person was born to the instant that the person dies" ,
                                                                                          "HQDM ordinary_biological_object" ,
                                                                                          "USAGE: Use this class for describing individual living things that cease to exist when all of their parts are removed." .


###  http://ontology.asam.net/ontologies/Core#WholeLifeOrdinaryFunctionalObject
<http://ontology.asam.net/ontologies/Core#WholeLifeOrdinaryFunctionalObject> rdf:type owl:Class ;
                                                                             rdfs:subClassOf <http://ontology.asam.net/ontologies/Core#OrdinaryFunctionalObjectState> ,
                                                                                             <http://ontology.asam.net/ontologies/Core#WholeLifeFunctionalObject> ;
                                                                             rdfs:comment "DEF: An OrdinaryFunctionalObjectState that represents the whole life of the ordinary functional object." ,
                                                                                          "EXAMPLES: a particular car (or traffic sign, road intersection, etc.) from the instant it is manufactured to the instant it is disassembled or otherwise ceases to be a car" ,
                                                                                          "HQDM ordinary_functional_object" ,
                                                                                          "USAGE: Use this class for describing individual manufactured things that were constructed for some purpose and that cease to exist when all of their parts are removed" .


###  http://ontology.asam.net/ontologies/Core#WholeLifeOrdinaryPhysicalObject
<http://ontology.asam.net/ontologies/Core#WholeLifeOrdinaryPhysicalObject> rdf:type owl:Class ;
                                                                           rdfs:subClassOf <http://ontology.asam.net/ontologies/Core#OrdinaryPhysicalObjectState> ,
                                                                                           <http://ontology.asam.net/ontologies/Core#WholeLifePhysicalObject> ;
                                                                           rdfs:comment "DEF: A OrdinaryPhysicalObjectState that represents the whole life of the ordinary physical object." ,
                                                                                        "EXAMPLES:" ,
                                                                                        "HQDM ordinary_physical_object" ,
                                                                                        "USAGE: Use this class for an ordinary physical object that is its temporal whole. " .


###  http://ontology.asam.net/ontologies/Core#WholeLifePhysicalObject
<http://ontology.asam.net/ontologies/Core#WholeLifePhysicalObject> rdf:type owl:Class ;
                                                                   rdfs:subClassOf <http://ontology.asam.net/ontologies/Core#PhysicalObjectState> ,
                                                                                   <http://ontology.asam.net/ontologies/Core#WholeLifeIndividual> ;
                                                                   rdfs:comment "DEF: A PhysicalObjectState that represents the whole life of the physical object." ,
                                                                                "EXAMPLES:" ,
                                                                                "HQDM physical_object" ,
                                                                                "USAGE: Use this class for a physical object that is its temporal whole. Note that it is generally preferable to use one of the subclasses." .


###  http://ontology.asam.net/ontologies/Core#WholeLifeSociallyConstructedActivity
<http://ontology.asam.net/ontologies/Core#WholeLifeSociallyConstructedActivity> rdf:type owl:Class ;
                                                                                rdfs:subClassOf <http://ontology.asam.net/ontologies/Core#SociallyConstructedActivityState> ,
                                                                                                <http://ontology.asam.net/ontologies/Core#WholeLifeIntentionallyConstructedActivity> ,
                                                                                                <http://ontology.asam.net/ontologies/Core#WholeLifeSociallyConstructedObject> ;
                                                                                rdfs:comment "DEF: A WholeLifeSociallyConstructedObject that is also a WholeLifeActivity." ,
                                                                                             "EXAMPLES:" ,
                                                                                             "HQDM socially_constructed_activity" ,
                                                                                             "USAGE: Use this class for an socially constructed activity that is its temporal whole." .


###  http://ontology.asam.net/ontologies/Core#WholeLifeSociallyConstructedObject
<http://ontology.asam.net/ontologies/Core#WholeLifeSociallyConstructedObject> rdf:type owl:Class ;
                                                                              rdfs:subClassOf <http://ontology.asam.net/ontologies/Core#SociallyConstructedObjectState> ,
                                                                                              <http://ontology.asam.net/ontologies/Core#WholeLifeIndividual> ;
                                                                              rdfs:comment "DEF: A SociallyConstructedObjectState that represents the whole life of the socially constructed object." ,
                                                                                           "EXAMPLES:" ,
                                                                                           "HQDM socially_constructed_object" ,
                                                                                           "USAGE: Use this class for an socially constructed object that is its temporal whole." .


###  http://ontology.asam.net/ontologies/Core#WholeLifeSystem
<http://ontology.asam.net/ontologies/Core#WholeLifeSystem> rdf:type owl:Class ;
                                                           rdfs:subClassOf <http://ontology.asam.net/ontologies/Core#SystemState> ,
                                                                           <http://ontology.asam.net/ontologies/Core#WholeLifeOrdinaryPhysicalObject> ;
                                                           rdfs:comment "DEF: An OrdinaryPhysicalObject that is an organized or connected group of PhysicalObjects that are SystemComponents and each have a role in how the overall system functions." ,
                                                                        "EXAMPLES: The entire life of a hurricane from when it was formed to when it ceases to exist." ,
                                                                        "HQDM system" ,
                                                                        "USAGE: Use this class for a system that is its temporal whole. Note that usually it is preferable to use the subclass WholeLifeFunctionalSystem for systems that are intentionally constructed for some purpose." .


###  http://ontology.asam.net/ontologies/Core#WholeLifeSystemComponent
<http://ontology.asam.net/ontologies/Core#WholeLifeSystemComponent> rdf:type owl:Class ;
                                                                    rdfs:subClassOf <http://ontology.asam.net/ontologies/Core#SystemComponentState> ,
                                                                                    <http://ontology.asam.net/ontologies/Core#WholeLifePhysicalObject> ,
                                                                                    [ rdf:type owl:Restriction ;
                                                                                      owl:onProperty <http://ontology.asam.net/ontologies/Core#componentOf> ;
                                                                                      owl:qualifiedCardinality "1"^^xsd:nonNegativeInteger ;
                                                                                      owl:onClass <http://ontology.asam.net/ontologies/Core#WholeLifeSystem>
                                                                                    ] ;
                                                                    rdfs:comment "DEF: A SystemComponentState that represents the whole life of the system component." ,
                                                                                 "EXAMPLES: the eye of a hurricane." ,
                                                                                 "HQDM system_component" ,
                                                                                 "USAGE: Use this class to specify the whole life of a component of a system that is not functional." .


###  http://ontology.asam.net/ontologies/Domain#Accelerate
<http://ontology.asam.net/ontologies/Domain#Accelerate> rdf:type owl:Class ;
                                                        rdfs:subClassOf <http://ontology.asam.net/ontologies/Domain#MovingActivity> ,
                                                                        <http://ontology.asam.net/ontologies/Domain#PrimitiveLevelActivity> ,
                                                                        <http://ontology.asam.net/ontologies/Domain#SingleParticipantActivity> ;
                                                        rdfs:comment "DEF: A MovingActivity with one traffic participant during which the speed of the traffic participant increases continuously."^^xsd:string .


###  http://ontology.asam.net/ontologies/Domain#ActivityByLevel
<http://ontology.asam.net/ontologies/Domain#ActivityByLevel> rdf:type owl:Class ;
                                                             rdfs:subClassOf <http://ontology.asam.net/ontologies/Domain#TrafficActivity> ;
                                                             rdfs:comment "DEF: A set of activities categorized according to the complexity of the action ranging from primitive to mission level."^^xsd:string .


###  http://ontology.asam.net/ontologies/Domain#ActivityByNumberOfParticipants
<http://ontology.asam.net/ontologies/Domain#ActivityByNumberOfParticipants> rdf:type owl:Class ;
                                                                            rdfs:subClassOf <http://ontology.asam.net/ontologies/Domain#TrafficActivity> ;
                                                                            rdfs:comment "DEF: A set of activities categorized according to the number of traffic participants involved."^^xsd:string .


###  http://ontology.asam.net/ontologies/Domain#ActivityByStateChange
<http://ontology.asam.net/ontologies/Domain#ActivityByStateChange> rdf:type owl:Class ;
                                                                   rdfs:subClassOf <http://ontology.asam.net/ontologies/Domain#TrafficActivity> ;
                                                                   rdfs:comment "DEF: A set of activities characterized by the participants moving or communicating."^^xsd:string .


###  http://ontology.asam.net/ontologies/Domain#ActivityByTrafficParticipantType
<http://ontology.asam.net/ontologies/Domain#ActivityByTrafficParticipantType> rdf:type owl:Class ;
                                                                              rdfs:subClassOf <http://ontology.asam.net/ontologies/Domain#TrafficActivity> ;
                                                                              rdfs:comment "DEF: A set of activities categorized according to the type of traffic participants."^^xsd:string .


###  http://ontology.asam.net/ontologies/Domain#AgricultureVehicle
<http://ontology.asam.net/ontologies/Domain#AgricultureVehicle> rdf:type owl:Class ;
                                                                rdfs:subClassOf <http://ontology.asam.net/ontologies/Domain#NonVRU> ,
                                                                                <http://ontology.asam.net/ontologies/Domain#Vehicle> ;
                                                                rdfs:comment "DEF: A vehicle that is specifically constructed for and used in farming."^^xsd:string ,
                                                                             "EXAMPLES: tractors, harvesters"^^xsd:string .


###  http://ontology.asam.net/ontologies/Domain#Animal
<http://ontology.asam.net/ontologies/Domain#Animal> rdf:type owl:Class ;
                                                    rdfs:subClassOf <http://ontology.asam.net/ontologies/Domain#TrafficParticipantByParticipantType> ,
                                                                    <http://ontology.asam.net/ontologies/Domain#VRU> ;
                                                    rdfs:comment "DEF: A TrafficParticipant that is a non-human biological object."^^xsd:string .


###  http://ontology.asam.net/ontologies/Domain#ArtificialLightingCondition
<http://ontology.asam.net/ontologies/Domain#ArtificialLightingCondition> rdf:type owl:Class ;
                                                                         rdfs:subClassOf <http://ontology.asam.net/ontologies/Domain#IlluminationCondition> ;
                                                                         rdfs:comment "DEF: An IlluminationCondition characterized by non-natural light from manufactured light sources, such as candles and electric lamps."^^xsd:string .


###  http://ontology.asam.net/ontologies/Domain#AutomaticAccessControlSystem
<http://ontology.asam.net/ontologies/Domain#AutomaticAccessControlSystem> rdf:type owl:Class ;
                                                                          rdfs:subClassOf <http://ontology.asam.net/ontologies/Domain#SpecialStructure> ;
                                                                          rdfs:comment "DEF: A SpecialStructure that provides detection and audit to limit who can go where. They can be combined with assured physical barriers to provide delay into a secure site or can be used with demarcation barriers, meaning half-height gates, to provide only detection"^^xsd:string .


###  http://ontology.asam.net/ontologies/Domain#BarriersOnRoadEdge
<http://ontology.asam.net/ontologies/Domain#BarriersOnRoadEdge> rdf:type owl:Class ;
                                                                rdfs:subClassOf <http://ontology.asam.net/ontologies/Domain#RoadwayEdgeElement> ;
                                                                rdfs:comment "DEF: A RoadwayEdgeElement that forms a barrier along the edge of the road."^^xsd:string .


###  http://ontology.asam.net/ontologies/Domain#Bicycle
<http://ontology.asam.net/ontologies/Domain#Bicycle> rdf:type owl:Class ;
                                                     rdfs:subClassOf <http://ontology.asam.net/ontologies/Domain#PrivateVehicle> ,
                                                                     <http://ontology.asam.net/ontologies/Domain#VRU> ;
                                                     rdfs:comment "DEF: A human-powered or motor-powered, pedal-driven, single-track Vehicle that has two wheels attached to a frame, one behind the other."^^xsd:string .


###  http://ontology.asam.net/ontologies/Domain#BorderCrossing
<http://ontology.asam.net/ontologies/Domain#BorderCrossing> rdf:type owl:Class ;
                                                            rdfs:subClassOf <http://ontology.asam.net/ontologies/Domain#SpecialStructure> ;
                                                            rdfs:comment "DEF: A SpecialStructure that is located at the border between states and that supports monitoring and regulating the movement of people, animals, and goods across the border."^^xsd:string .


###  http://ontology.asam.net/ontologies/Domain#Bridge
<http://ontology.asam.net/ontologies/Domain#Bridge> rdf:type owl:Class ;
                                                    rdfs:subClassOf <http://ontology.asam.net/ontologies/Domain#SpecialStructure> ;
                                                    rdfs:comment "DEF: A SpecialStructure built to span a physical obstacle, such as a river, a valley or a road, withouth blocking the way underneath. A bridge provides passage over the obstacle."^^xsd:string .


###  http://ontology.asam.net/ontologies/Domain#BrokenClouds
<http://ontology.asam.net/ontologies/Domain#BrokenClouds> rdf:type owl:Class ;
                                                          rdfs:subClassOf <http://ontology.asam.net/ontologies/Domain#CloudCondition> ;
                                                          rdfs:comment "DEF: BrokenClouds is a CloudCondition, is it described by the cloudinessLevel property using oktas unit, BrokenClouds is when the cloudinessLevel is 5-7 oktas."^^xsd:string .


###  http://ontology.asam.net/ontologies/Domain#BrokenLine
<http://ontology.asam.net/ontologies/Domain#BrokenLine> rdf:type owl:Class ;
                                                        rdfs:subClassOf <http://ontology.asam.net/ontologies/Domain#LaneMarking> ;
                                                        rdfs:comment "DEF: BrokenLine is a  LaneMarking that is used to mark the middle of a two lane highway to separate traffic on both directions. Drivers are supposed to keep left but can cross the broken line for overtaking if situations permit"^^xsd:string .


###  http://ontology.asam.net/ontologies/Domain#Building
<http://ontology.asam.net/ontologies/Domain#Building> rdf:type owl:Class ;
                                                      rdfs:subClassOf <http://ontology.asam.net/ontologies/Domain#FixedRoadStructure> ;
                                                      rdfs:comment "DEF: A FixedRoadStructure that is a built physical structure with a roof and walls standing more or less permanently in one place."^^xsd:string ,
                                                                   "EXAMPLES: houses and factories"^^xsd:string .


###  http://ontology.asam.net/ontologies/Domain#Bus
<http://ontology.asam.net/ontologies/Domain#Bus> rdf:type owl:Class ;
                                                 rdfs:subClassOf <http://ontology.asam.net/ontologies/Domain#NonVRU> ,
                                                                 <http://ontology.asam.net/ontologies/Domain#PublicTransportationVehicle> ;
                                                 rdfs:comment "DEF: A vehicle that is designed to carry many passengers and that usually travels along a fixed route according to a schedule."^^xsd:string ;
                                                 rdfs:label "PublicBus"^^xsd:string .


###  http://ontology.asam.net/ontologies/Domain#BusLane
<http://ontology.asam.net/ontologies/Domain#BusLane> rdf:type owl:Class ;
                                                     rdfs:subClassOf <http://ontology.asam.net/ontologies/Domain#LaneForSpecificParticipants> ;
                                                     rdfs:comment "DEF: BusLane is a  LaneForSpecificParticipants that is a lane where only buses are allowed to drive"^^xsd:string .


###  http://ontology.asam.net/ontologies/Domain#CalmWind
<http://ontology.asam.net/ontologies/Domain#CalmWind> rdf:type owl:Class ;
                                                      rdfs:subClassOf <http://ontology.asam.net/ontologies/Domain#WindCondition> ;
                                                      rdfs:comment "DEF: CalmWind is a WindCondition, is it described by the WindSpeed property using m/s, CalmWind is when the WindSpeed is 0 - 0.2 m/s."^^xsd:string .


###  http://ontology.asam.net/ontologies/Domain#Car
<http://ontology.asam.net/ontologies/Domain#Car> rdf:type owl:Class ;
                                                 rdfs:subClassOf <http://ontology.asam.net/ontologies/Domain#NonVRU> ,
                                                                 <http://ontology.asam.net/ontologies/Domain#PrivateVehicle> ;
                                                 rdfs:comment "DEF: A Vehicle that is an automobile. It is a motor-powered vehicle used for transporting a small number of people."^^xsd:string .


###  http://ontology.asam.net/ontologies/Domain#ChangeLane
<http://ontology.asam.net/ontologies/Domain#ChangeLane> rdf:type owl:Class ;
                                                        rdfs:subClassOf <http://ontology.asam.net/ontologies/Domain#DrivingActivity> ,
                                                                        <http://ontology.asam.net/ontologies/Domain#LateralActivity> ,
                                                                        <http://ontology.asam.net/ontologies/Domain#ManeuverLevelActivity> ,
                                                                        <http://ontology.asam.net/ontologies/Domain#SingleParticipantActivity> ;
                                                        rdfs:comment "DEF: An activity in which the subject vehicle starts from one lane at the beginning of the activity and drives in a different lane at the end of the activity."^^xsd:string .


###  http://ontology.asam.net/ontologies/Domain#ChangeToLeftLane
<http://ontology.asam.net/ontologies/Domain#ChangeToLeftLane> rdf:type owl:Class ;
                                                              rdfs:subClassOf <http://ontology.asam.net/ontologies/Domain#ChangeLane> ;
                                                              rdfs:comment "DEF: A ChangeLane activity where the vehicle drives in one lane at the beginning of the activity and drives in the lane left to the original lane at the end of the activity."^^xsd:string .


###  http://ontology.asam.net/ontologies/Domain#ChangeToRightLane
<http://ontology.asam.net/ontologies/Domain#ChangeToRightLane> rdf:type owl:Class ;
                                                               rdfs:subClassOf <http://ontology.asam.net/ontologies/Domain#ChangeLane> ;
                                                               rdfs:comment "DEF: A ChangeLane activity where the vehicle drives in one lane at the beginning of the activity and drives in the lane right to the original lane at the end of the activity."^^xsd:string .


###  http://ontology.asam.net/ontologies/Domain#Clear
<http://ontology.asam.net/ontologies/Domain#Clear> rdf:type owl:Class ;
                                                   rdfs:subClassOf <http://ontology.asam.net/ontologies/Domain#CloudCondition> ;
                                                   rdfs:comment "DEF: Clear is a CloudCondition, is it described by the cloudinessLevel property using oktas unit, Clear is when the cloudinessLevel is 0-1 oktas."^^xsd:string .


###  http://ontology.asam.net/ontologies/Domain#CloseUp
<http://ontology.asam.net/ontologies/Domain#CloseUp> rdf:type owl:Class ;
                                                     rdfs:subClassOf <http://ontology.asam.net/ontologies/Domain#ActivityByTrafficParticipantType> ,
                                                                     <http://ontology.asam.net/ontologies/Domain#ManeuverLevelActivity> ,
                                                                     <http://ontology.asam.net/ontologies/Domain#MovingActivity> ,
                                                                     <http://ontology.asam.net/ontologies/Domain#MultiParticipantActivity> ;
                                                     rdfs:comment "DEF: A MovingActivity during which the subject traffic participant moves closer to the object traffic participant."^^xsd:string .


###  http://ontology.asam.net/ontologies/Domain#CloudCondition
<http://ontology.asam.net/ontologies/Domain#CloudCondition> rdf:type owl:Class ;
                                                            rdfs:subClassOf <http://ontology.asam.net/ontologies/Domain#WeatherCondition> ;
                                                            rdfs:comment "DEF: A WeatherCondition in which a specific amount of the sky is covered by clouds, which affects the illumination of things. This condition can occur during day and night. The amount of sky covered in clouds may be described with the cloudinessLevel property."^^xsd:string .


###  http://ontology.asam.net/ontologies/Domain#Cloudburst
<http://ontology.asam.net/ontologies/Domain#Cloudburst> rdf:type owl:Class ;
                                                        rdfs:subClassOf <http://ontology.asam.net/ontologies/Domain#RainfallCondition> ;
                                                        rdfs:comment "DEF: Cloudburst is a RainfallCondition, is it described by the precipitationIntensity property using mm/hr, Cloudburst is when the precipitationIntensity is > 100mm/hr."^^xsd:string .


###  http://ontology.asam.net/ontologies/Domain#CommunicationActivity
<http://ontology.asam.net/ontologies/Domain#CommunicationActivity> rdf:type owl:Class ;
                                                                   rdfs:subClassOf <http://ontology.asam.net/ontologies/Domain#ActivityByStateChange> ;
                                                                   rdfs:comment "DEF: A set of activites that are characterized by the subject traffic participant giving visual or acoustic signals in order to relay its intentions to other traffic participants."^^xsd:string .


###  http://ontology.asam.net/ontologies/Domain#CommunicationCondition
<http://ontology.asam.net/ontologies/Domain#CommunicationCondition> rdf:type owl:Class ;
                                                                    rdfs:subClassOf <http://ontology.asam.net/ontologies/Domain#ConnectivityCondition> ;
                                                                    rdfs:comment "DEF: A ConnectivityCondition that defines the type of communication method used for the communication between vehicle and other elements of the traffic domain, such as infrastructure (V2I) or other vehicles (V2V)."^^xsd:string .


###  http://ontology.asam.net/ontologies/Domain#ConnectivityCondition
<http://ontology.asam.net/ontologies/Domain#ConnectivityCondition> rdf:type owl:Class ;
                                                                   rdfs:subClassOf <http://ontology.asam.net/ontologies/Core#PhysicalProperty> ,
                                                                                   <http://ontology.asam.net/ontologies/Domain#EnvironmentalCondition> ;
                                                                   rdfs:comment "DEF: An EnvironmentalCondition that indicates a vehicle's ability to receive data from or transmit data to external systems. The purpose of the data transfer can be positioning of the vehicle or communication with other elements of the traffic domain."^^xsd:string .


###  http://ontology.asam.net/ontologies/Domain#ConstructionSign
<http://ontology.asam.net/ontologies/Domain#ConstructionSign> rdf:type owl:Class ;
                                                              rdfs:subClassOf <http://ontology.asam.net/ontologies/Domain#TemporaryRoadStructure> ;
                                                              rdfs:comment "DEF: A TemporaryRoadStructure that is a traffic sign indicating construction or landscaping work in a specific area."^^xsd:string .


###  http://ontology.asam.net/ontologies/Domain#ConstructionSiteDetour
<http://ontology.asam.net/ontologies/Domain#ConstructionSiteDetour> rdf:type owl:Class ;
                                                                    rdfs:subClassOf <http://ontology.asam.net/ontologies/Domain#TemporaryRoadStructure> ;
                                                                    rdfs:comment "DEF: A TemporaryRoadStructure that provides a detour or temporary route around an area that needs to be avoided, for example, due to construction work."^^xsd:string .


###  http://ontology.asam.net/ontologies/Domain#ConstructionVehicle
<http://ontology.asam.net/ontologies/Domain#ConstructionVehicle> rdf:type owl:Class ;
                                                                 rdfs:subClassOf <http://ontology.asam.net/ontologies/Domain#NonVRU> ,
                                                                                 <http://ontology.asam.net/ontologies/Domain#Vehicle> ;
                                                                 rdfs:comment "DEF: A vehicle that is specifically built for and used in construction work."^^xsd:string ,
                                                                              "EXAMPLES: crane, bulldozer"^^xsd:string .


###  http://ontology.asam.net/ontologies/Domain#Cracks
<http://ontology.asam.net/ontologies/Domain#Cracks> rdf:type owl:Class ;
                                                    rdfs:subClassOf <http://ontology.asam.net/ontologies/Domain#RoadSurfaceFeature> ;
                                                    rdfs:comment "DEF:Cracks is a  RoadSurfaceFeature  that are fractures or discontinuation of the road surface."^^xsd:string ;
                                                    rdfs:label "Cracks" .


###  http://ontology.asam.net/ontologies/Domain#Cross
<http://ontology.asam.net/ontologies/Domain#Cross> rdf:type owl:Class ;
                                                   rdfs:subClassOf <http://ontology.asam.net/ontologies/Domain#ActivityByTrafficParticipantType> ,
                                                                   <http://ontology.asam.net/ontologies/Domain#ManeuverLevelActivity> ,
                                                                   <http://ontology.asam.net/ontologies/Domain#MovingActivity> ,
                                                                   <http://ontology.asam.net/ontologies/Domain#MultiParticipantActivity> ;
                                                   rdfs:comment "DEF: A MovingActivity during which the path of the subject traffic participant crosses the path of the object traffic participant."^^xsd:string .


###  http://ontology.asam.net/ontologies/Domain#CrossRoad
<http://ontology.asam.net/ontologies/Domain#CrossRoad> rdf:type owl:Class ;
                                                       rdfs:subClassOf <http://ontology.asam.net/ontologies/Domain#IntersectionAtGrade> ;
                                                       rdfs:comment "DEF: An Intersection where exactly four roads meet."^^xsd:string .


###  http://ontology.asam.net/ontologies/Domain#Curb
<http://ontology.asam.net/ontologies/Domain#Curb> rdf:type owl:Class ;
                                                  rdfs:subClassOf <http://ontology.asam.net/ontologies/Domain#PhysicalDivider> ;
                                                  rdfs:comment "DEF: Curb is a  PhysicalDivider that is the edge where a raised sidewalk or road median/central reservation meets a street or other roadway."^^xsd:string .


###  http://ontology.asam.net/ontologies/Domain#CutIn
<http://ontology.asam.net/ontologies/Domain#CutIn> rdf:type owl:Class ;
                                                   rdfs:subClassOf <http://ontology.asam.net/ontologies/Domain#DrivingActivity> ,
                                                                   <http://ontology.asam.net/ontologies/Domain#ManeuverLevelActivity> ,
                                                                   <http://ontology.asam.net/ontologies/Domain#MovingActivity> ,
                                                                   <http://ontology.asam.net/ontologies/Domain#MultiParticipantActivity> ;
                                                   rdfs:comment "DEF: A MovingActivity in which the subject traffic participant ends up directly in front of the object traffic participant. A cutting-in activity can affect the behavior of the object."^^xsd:string .


###  http://ontology.asam.net/ontologies/Domain#CutOut
<http://ontology.asam.net/ontologies/Domain#CutOut> rdf:type owl:Class ;
                                                    rdfs:subClassOf <http://ontology.asam.net/ontologies/Domain#DrivingActivity> ,
                                                                    <http://ontology.asam.net/ontologies/Domain#ManeuverLevelActivity> ,
                                                                    <http://ontology.asam.net/ontologies/Domain#MovingActivity> ,
                                                                    <http://ontology.asam.net/ontologies/Domain#MultiParticipantActivity> ;
                                                    rdfs:comment "DEF: A MovingActivity where the subject and the object traffic participants start in the same lane. During the activity, the object traffic participant suddenly leaves the lane."^^xsd:string .


###  http://ontology.asam.net/ontologies/Domain#CycleLane
<http://ontology.asam.net/ontologies/Domain#CycleLane> rdf:type owl:Class ;
                                                       rdfs:subClassOf <http://ontology.asam.net/ontologies/Domain#LaneForSpecificParticipants> ;
                                                       rdfs:comment "DEF: CycleLane is a  LaneForSpecificParticipants that is paved  and intended for bicycle use only. Contains only regions or ground specifically designated for cyclists where pedestrians and cars should not enter."^^xsd:string .


###  http://ontology.asam.net/ontologies/Domain#DayLightingCondition
<http://ontology.asam.net/ontologies/Domain#DayLightingCondition> rdf:type owl:Class ;
                                                                  rdfs:subClassOf <http://ontology.asam.net/ontologies/Domain#IlluminationCondition> ;
                                                                  rdfs:comment "DEF: An IlluminationCondition where illuminance is greater than 2000 lux."^^xsd:string .


###  http://ontology.asam.net/ontologies/Domain#Debris
<http://ontology.asam.net/ontologies/Domain#Debris> rdf:type owl:Class ;
                                                    rdfs:subClassOf <http://ontology.asam.net/ontologies/Domain#TemporaryRoadStructure> ;
                                                    rdfs:comment "DEF: A TemporaryRoadStructure that consists of scattered pieces of rock, rubbish or other loose material on the road surface; placed not by intention, but by accident or construction work."^^xsd:string .


###  http://ontology.asam.net/ontologies/Domain#Decelerate
<http://ontology.asam.net/ontologies/Domain#Decelerate> rdf:type owl:Class ;
                                                        rdfs:subClassOf <http://ontology.asam.net/ontologies/Domain#MovingActivity> ,
                                                                        <http://ontology.asam.net/ontologies/Domain#PrimitiveLevelActivity> ,
                                                                        <http://ontology.asam.net/ontologies/Domain#SingleParticipantActivity> ;
                                                        rdfs:comment "DEF: A MovingActivity with one traffic participant during which the speed of the traffic participant decreases continuously."^^xsd:string .


###  http://ontology.asam.net/ontologies/Domain#DistributorRoad
<http://ontology.asam.net/ontologies/Domain#DistributorRoad> rdf:type owl:Class ;
                                                             rdfs:subClassOf <http://ontology.asam.net/ontologies/Domain#Road> ;
                                                             rdfs:comment "DEF: A Road with low to moderate capacity that connects local and minor roads to arterial roads."^^xsd:string .


###  http://ontology.asam.net/ontologies/Domain#DividedRoad
<http://ontology.asam.net/ontologies/Domain#DividedRoad> rdf:type owl:Class ;
                                                         rdfs:subClassOf <http://ontology.asam.net/ontologies/Domain#Road> ;
                                                         rdfs:comment "DEF: A type of road that has several carriageways for traffic travelling in opposite directions. The carriageways are separated by a central reservation."^^xsd:string .


###  http://ontology.asam.net/ontologies/Domain#DomainConcepts
<http://ontology.asam.net/ontologies/Domain#DomainConcepts> rdf:type owl:Class ;
                                                            rdfs:comment "DEF: Top-level container that separates domain concepts in the OpenXOntology. The DomainConcepts define central concepts of the road traffic domain, for example, lane, road, and vehicle. It contains only concepts that are shared by multiple ASAM OpenX standards using the ASAM OpenXOntology and that are not controlled by a single standard." .


###  http://ontology.asam.net/ontologies/Domain#DoubleSolidLine
<http://ontology.asam.net/ontologies/Domain#DoubleSolidLine> rdf:type owl:Class ;
                                                             rdfs:subClassOf <http://ontology.asam.net/ontologies/Domain#LaneMarking> ;
                                                             rdfs:comment "DEF: DoubleSolidLine is a LaneMarking that separates two lanes."^^xsd:string .


###  http://ontology.asam.net/ontologies/Domain#DrivableAreaElement
<http://ontology.asam.net/ontologies/Domain#DrivableAreaElement> rdf:type owl:Class ;
                                                                 rdfs:subClassOf <http://ontology.asam.net/ontologies/Core#WholeLifeFunctionalSystem> ,
                                                                                 <http://ontology.asam.net/ontologies/Core#WholeLifeFunctionalSystemComponent> ,
                                                                                 <http://ontology.asam.net/ontologies/Core#WholeLifeSystemComponent> ,
                                                                                 <http://ontology.asam.net/ontologies/Domain#RoadTopologyAndTrafficInfrastructure> ;
                                                                 rdfs:comment "DEF: Areas in the traffic infrastructure that vehicles are supposed and permitted to drive in."^^xsd:string ,
                                                                              "EXAMPLES: lanes, roads, and road edges"^^xsd:string .


###  http://ontology.asam.net/ontologies/Domain#Driver
<http://ontology.asam.net/ontologies/Domain#Driver> rdf:type owl:Class ;
                                                    rdfs:subClassOf <http://ontology.asam.net/ontologies/Domain#Human> ,
                                                                    <http://ontology.asam.net/ontologies/Domain#VRU> ;
                                                    rdfs:comment "DEF: A HumanParticipant who controls a vehicle."^^xsd:string .


###  http://ontology.asam.net/ontologies/Domain#DrivingActivity
<http://ontology.asam.net/ontologies/Domain#DrivingActivity> rdf:type owl:Class ;
                                                             rdfs:subClassOf <http://ontology.asam.net/ontologies/Domain#MovingActivity> ,
                                                                             <http://ontology.asam.net/ontologies/Domain#VehicleActivity> ;
                                                             rdfs:comment "DEF: A set of moving activites that are characterized by a continuous movement of the traffic participants during the complete activity."^^xsd:string .


###  http://ontology.asam.net/ontologies/Domain#DynamicTrafficSign
<http://ontology.asam.net/ontologies/Domain#DynamicTrafficSign> rdf:type owl:Class ;
                                                                rdfs:subClassOf <http://ontology.asam.net/ontologies/Domain#TrafficSignByState> ;
                                                                rdfs:comment "DEF: A traffic sign whose content can be changed."^^xsd:string ,
                                                                             "EXAMPLES: traffic lights, variable message signs"^^xsd:string .


###  http://ontology.asam.net/ontologies/Domain#EmergencyVehicle
<http://ontology.asam.net/ontologies/Domain#EmergencyVehicle> rdf:type owl:Class ;
                                                              rdfs:subClassOf <http://ontology.asam.net/ontologies/Domain#NonVRU> ,
                                                                              <http://ontology.asam.net/ontologies/Domain#OfficialVehicle> ;
                                                              rdfs:comment "DEF: A vehicle that is used by an emergency service to respond to incidents."^^xsd:string .


###  http://ontology.asam.net/ontologies/Domain#EnvironmentalCondition
<http://ontology.asam.net/ontologies/Domain#EnvironmentalCondition> rdf:type owl:Class ;
                                                                    rdfs:subClassOf <http://ontology.asam.net/ontologies/Domain#DomainConcepts> ;
                                                                    rdfs:comment "DEF: A set of environmental parameters that applies to a complete area, such as a town or a district. Conditions can have natural causes, for example rain or snowfall, or can be created artificially, for example by light sources or communication devices using specific methods like vehice-to-vehicle communication."^^xsd:string .


###  http://ontology.asam.net/ontologies/Domain#FewClouds
<http://ontology.asam.net/ontologies/Domain#FewClouds> rdf:type owl:Class ;
                                                       rdfs:subClassOf <http://ontology.asam.net/ontologies/Domain#CloudCondition> ;
                                                       rdfs:comment "DEF: FewClouds is a CloudCondition, is it described by the cloudinessLevel property using oktas unit, FewClouds is when the cloudinessLevel is 1-2 oktas."^^xsd:string .


###  http://ontology.asam.net/ontologies/Domain#FixedRoadStructure
<http://ontology.asam.net/ontologies/Domain#FixedRoadStructure> rdf:type owl:Class ;
                                                                rdfs:subClassOf <http://ontology.asam.net/ontologies/Core#WholeLifeFunctionalSystemComponent> ,
                                                                                <http://ontology.asam.net/ontologies/Core#WholeLifeSystemComponent> ,
                                                                                <http://ontology.asam.net/ontologies/Domain#RoadTopologyAndTrafficInfrastructure> ;
                                                                rdfs:comment "DEF: An element of the traffic infrastructure with a physical form that is either built or natural and is located near to or on a drivable area. Vehicles are not allowed to drive on a FixedRoadStructure."^^xsd:string ,
                                                                             "EXAMPLES: buildings and trees"^^xsd:string .


###  http://ontology.asam.net/ontologies/Domain#FlashHeadlights
<http://ontology.asam.net/ontologies/Domain#FlashHeadlights> rdf:type owl:Class ;
                                                             rdfs:subClassOf <http://ontology.asam.net/ontologies/Domain#VehicleCommunicationActivity> ;
                                                             rdfs:comment "DEF: A VehicleCommunicatingActivity in which the subject vehicle communicates a potential warning to the object vehicle by either briefly switching on the headlights or switching between low beams and high beams."^^xsd:string .


###  http://ontology.asam.net/ontologies/Domain#FoggyCondition
<http://ontology.asam.net/ontologies/Domain#FoggyCondition> rdf:type owl:Class ;
                                                            rdfs:subClassOf <http://ontology.asam.net/ontologies/Domain#ParticulatesCondition> ;
                                                            rdfs:comment "DEF: A ParticulateCondition where the particles are a mixture of non-precipitating water droplets or ice crystals."^^xsd:string .


###  http://ontology.asam.net/ontologies/Domain#FollowRoadUser
<http://ontology.asam.net/ontologies/Domain#FollowRoadUser> rdf:type owl:Class ;
                                                            rdfs:subClassOf <http://ontology.asam.net/ontologies/Domain#ManeuverLevelActivity> ,
                                                                            <http://ontology.asam.net/ontologies/Domain#MultiParticipantActivity> ;
                                                            rdfs:comment "DEF: An activity in which the subject traffic participant drives behind the object traffic participant at the same speed."^^xsd:string .


###  http://ontology.asam.net/ontologies/Domain#FollowTargetSpeed
<http://ontology.asam.net/ontologies/Domain#FollowTargetSpeed> rdf:type owl:Class ;
                                                               rdfs:subClassOf <http://ontology.asam.net/ontologies/Domain#ManeuverLevelActivity> ,
                                                                               <http://ontology.asam.net/ontologies/Domain#SingleParticipantActivity> ;
                                                               rdfs:comment "DEF: An activity in which the subject traffic participant drives at a fixed, configured speed."^^xsd:string .


###  http://ontology.asam.net/ontologies/Domain#FollowTrajectory
<http://ontology.asam.net/ontologies/Domain#FollowTrajectory> rdf:type owl:Class ;
                                                              rdfs:subClassOf <http://ontology.asam.net/ontologies/Domain#ManeuverLevelActivity> ,
                                                                              <http://ontology.asam.net/ontologies/Domain#SingleParticipantActivity> ;
                                                              rdfs:comment "DEF: An activity in which the subject traffic participant follows a defined driving path for a specific period of time."^^xsd:string .


###  http://ontology.asam.net/ontologies/Domain#FreshBreeze
<http://ontology.asam.net/ontologies/Domain#FreshBreeze> rdf:type owl:Class ;
                                                         rdfs:subClassOf <http://ontology.asam.net/ontologies/Domain#WindCondition> ;
                                                         rdfs:comment "DEF: FreshBreeze is a WindCondition, is it described by the WindSpeed property using m/s, FreshBreeze is when the WindSpeed is 8.0-10.7 m/s."^^xsd:string .


###  http://ontology.asam.net/ontologies/Domain#GLONASS
<http://ontology.asam.net/ontologies/Domain#GLONASS> rdf:type owl:Class ;
                                                     rdfs:subClassOf <http://ontology.asam.net/ontologies/Domain#PositioningCondition> ;
                                                     rdfs:comment "DEF: A PositioningCondition in which the vehicle's position is determined using the GLONASS global navigation satellite system."^^xsd:string .


###  http://ontology.asam.net/ontologies/Domain#GPS
<http://ontology.asam.net/ontologies/Domain#GPS> rdf:type owl:Class ;
                                                 rdfs:subClassOf <http://ontology.asam.net/ontologies/Domain#PositioningCondition> ;
                                                 rdfs:comment "DEF: A PositioningCondition in which the vehicle's position is determined using the Global Positioning System (GPS)."^^xsd:string .


###  http://ontology.asam.net/ontologies/Domain#Gale
<http://ontology.asam.net/ontologies/Domain#Gale> rdf:type owl:Class ;
                                                  rdfs:subClassOf <http://ontology.asam.net/ontologies/Domain#WindCondition> ;
                                                  rdfs:comment "DEF: Gale is a WindCondition, is it described by the WindSpeed property using m/s, Gale is when the WindSpeed is 17.2-20.7 m/s."^^xsd:string .


###  http://ontology.asam.net/ontologies/Domain#Galileo
<http://ontology.asam.net/ontologies/Domain#Galileo> rdf:type owl:Class ;
                                                     rdfs:subClassOf <http://ontology.asam.net/ontologies/Domain#PositioningCondition> ;
                                                     rdfs:comment "DEF: A PositioningCondition in which the vehicle's position is determined using the Galileo global navigation satellite system."^^xsd:string .


###  http://ontology.asam.net/ontologies/Domain#GentleBreeze
<http://ontology.asam.net/ontologies/Domain#GentleBreeze> rdf:type owl:Class ;
                                                          rdfs:subClassOf <http://ontology.asam.net/ontologies/Domain#WindCondition> ;
                                                          rdfs:comment "DEF: GentleBreeze is a WindCondition, is it described by the WindSpeed property using m/s, GentleBreeze is when the WindSpeed is 3.4-5.4 m/s."^^xsd:string .


###  http://ontology.asam.net/ontologies/Domain#GeofencedZone
<http://ontology.asam.net/ontologies/Domain#GeofencedZone> rdf:type owl:Class ;
                                                           rdfs:subClassOf <http://ontology.asam.net/ontologies/Domain#TrafficZone> ;
                                                           rdfs:comment "DEF: A geographic Zone with a virtual perimeter. Geofencing uses the GPS signal or other device services to track when a device crosses the virtual perimeter and enters the geo-fenced zone."^^xsd:string ,
                                                                        "EXAMPLES: Perimeters around school campuses or retirement communities. Geofencing triggers alerts to users or operators when registered devices leave the area."^^xsd:string .


###  http://ontology.asam.net/ontologies/Domain#GoodsVehicle
<http://ontology.asam.net/ontologies/Domain#GoodsVehicle> rdf:type owl:Class ;
                                                          rdfs:subClassOf <http://ontology.asam.net/ontologies/Domain#Vehicle> ;
                                                          rdfs:comment "DEF: Goods vehicles are vehicles with their designed purpose of transporting goods"^^xsd:string .


###  http://ontology.asam.net/ontologies/Domain#GradeSeparatedIntersection
<http://ontology.asam.net/ontologies/Domain#GradeSeparatedIntersection> rdf:type owl:Class ;
                                                                        rdfs:subClassOf <http://ontology.asam.net/ontologies/Domain#Junction> ;
                                                                        rdfs:comment "DEF: A Junction with two or more roads at different heights (grades). This layout ensures that the traffic flow on each axis is not disrupted by the crossing. The grade separation of the roads is achieved by means of overpasses, for example bridges, or underpasses, for example tunnels, or a combination of both."^^xsd:string .


###  http://ontology.asam.net/ontologies/Domain#GrassShoulder
<http://ontology.asam.net/ontologies/Domain#GrassShoulder> rdf:type owl:Class ;
                                                           rdfs:subClassOf <http://ontology.asam.net/ontologies/Domain#LaneWithConstructionProperties> ;
                                                           rdfs:comment "DEF: GrassShoulder is a  LanesWithConstructionProperties that is an emergency stopping lane by the verge of a road or motorway. Hence, a shoulder, where the surface of a lane consists out of grass is called grass shoulder"^^xsd:string .


###  http://ontology.asam.net/ontologies/Domain#GuardRail
<http://ontology.asam.net/ontologies/Domain#GuardRail> rdf:type owl:Class ;
                                                       rdfs:subClassOf <http://ontology.asam.net/ontologies/Domain#PhysicalDivider> ;
                                                       rdfs:comment "DEF: GuardRail is a  PhysicalDivider that is a strong fence at the side of a road or in the middle of an expressway, intended to reduce the risk of serious accidents; a crash barrier."^^xsd:string .


###  http://ontology.asam.net/ontologies/Domain#HeavyRain
<http://ontology.asam.net/ontologies/Domain#HeavyRain> rdf:type owl:Class ;
                                                       rdfs:subClassOf <http://ontology.asam.net/ontologies/Domain#RainfallCondition> ;
                                                       rdfs:comment "DEF: HeavyRain is a RainfallCondition, is it described by the precipitationIntensity property using mm/hr, HeavyRain is when the precipitationIntensity is 7.6 - 50 mm/hr."^^xsd:string .


###  http://ontology.asam.net/ontologies/Domain#HeavySnow
<http://ontology.asam.net/ontologies/Domain#HeavySnow> rdf:type owl:Class ;
                                                       rdfs:subClassOf <http://ontology.asam.net/ontologies/Domain#SnowfallCondition> ;
                                                       rdfs:comment "DEF: HeavySnow is a SnowfallCondition, is it described by the SnowfallIntensity property using visibility, HeavySnow is when the SnowfallIntensity is < 0.5 km."^^xsd:string .


###  http://ontology.asam.net/ontologies/Domain#HonkHorn
<http://ontology.asam.net/ontologies/Domain#HonkHorn> rdf:type owl:Class ;
                                                      rdfs:subClassOf <http://ontology.asam.net/ontologies/Domain#VehicleCommunicationActivity> ;
                                                      rdfs:comment "DEF: A VehicleCommunicatingActivity in which the subject vehicle sounds the car horn in order to warn other traffic participants."^^xsd:string .


###  http://ontology.asam.net/ontologies/Domain#Human
<http://ontology.asam.net/ontologies/Domain#Human> rdf:type owl:Class ;
                                                   rdfs:subClassOf <http://ontology.asam.net/ontologies/Domain#TrafficParticipantByParticipantType> ;
                                                   rdfs:comment "DEF: A human TrafficParticipant that is driving or moving in traffic, either within/on a vehicle or as pedestrian."^^xsd:string .


###  http://ontology.asam.net/ontologies/Domain#HumanActivity
<http://ontology.asam.net/ontologies/Domain#HumanActivity> rdf:type owl:Class ;
                                                           rdfs:subClassOf <http://ontology.asam.net/ontologies/Domain#ActivityByTrafficParticipantType> ;
                                                           rdfs:comment "DEF: A set of activities performed by humans, such as pedestrians."^^xsd:string .


###  http://ontology.asam.net/ontologies/Domain#Hurricane
<http://ontology.asam.net/ontologies/Domain#Hurricane> rdf:type owl:Class ;
                                                       rdfs:subClassOf <http://ontology.asam.net/ontologies/Domain#WindCondition> ;
                                                       rdfs:comment "DEF: Hurricane is a WindCondition, is it described by the WindSpeed property using m/s, Hurricane is when the WindSpeed is >= 32.7 m/s."^^xsd:string .


###  http://ontology.asam.net/ontologies/Domain#IlluminationCondition
<http://ontology.asam.net/ontologies/Domain#IlluminationCondition> rdf:type owl:Class ;
                                                                   rdfs:subClassOf <http://ontology.asam.net/ontologies/Core#PhysicalProperty> ,
                                                                                   <http://ontology.asam.net/ontologies/Domain#EnvironmentalCondition> ;
                                                                   rdfs:comment "DEF: An EnvironmentalCondition that is defined by the characteristics of light within a specific traffic situation. The objects that emit the light may be manufactured, such as lamps, or natural, like the sun. Illumination can improve the visibility of things or deteriorate it, for example by shadows or glare."^^xsd:string .


###  http://ontology.asam.net/ontologies/Domain#InformationSign
<http://ontology.asam.net/ontologies/Domain#InformationSign> rdf:type owl:Class ;
                                                             rdfs:subClassOf <http://ontology.asam.net/ontologies/Domain#TrafficSignByFunction> ;
                                                             rdfs:comment "DEF: A traffic sign that provides information to traffic participants regarding the route, traffic flow, or road condition, but does not enforce any traffic rule."^^xsd:string .


###  http://ontology.asam.net/ontologies/Domain#InterferenceZone
<http://ontology.asam.net/ontologies/Domain#InterferenceZone> rdf:type owl:Class ;
                                                              rdfs:subClassOf <http://ontology.asam.net/ontologies/Domain#TrafficZone> ;
                                                              rdfs:comment "DEF: A zone with limited positioning-signal reception caused by dense foliage on surfaces, tall buildings, tunnels, atmospheric interference, or similar."^^xsd:string .


###  http://ontology.asam.net/ontologies/Domain#IntersectionAtGrade
<http://ontology.asam.net/ontologies/Domain#IntersectionAtGrade> rdf:type owl:Class ;
                                                                 rdfs:subClassOf <http://ontology.asam.net/ontologies/Domain#Junction> ;
                                                                 rdfs:comment "DEF: A Junction where two or more roads meet at the same level."^^xsd:string .


###  http://ontology.asam.net/ontologies/Domain#Junction
<http://ontology.asam.net/ontologies/Domain#Junction> rdf:type owl:Class ;
                                                      rdfs:subClassOf <http://ontology.asam.net/ontologies/Core#WholeLifeFunctionalSystem> ,
                                                                      <http://ontology.asam.net/ontologies/Core#WholeLifeSystem> ,
                                                                      <http://ontology.asam.net/ontologies/Domain#RoadTopologyAndTrafficInfrastructure> ;
                                                      rdfs:comment "DEF: A RoadTopologyAndTrafficInfrastructure where two or more roads meet."^^xsd:string .


###  http://ontology.asam.net/ontologies/Domain#KeepLane
<http://ontology.asam.net/ontologies/Domain#KeepLane> rdf:type owl:Class ;
                                                      rdfs:subClassOf <http://ontology.asam.net/ontologies/Domain#DrivingActivity> ,
                                                                      <http://ontology.asam.net/ontologies/Domain#LongitudinalActivity> ,
                                                                      <http://ontology.asam.net/ontologies/Domain#ManeuverLevelActivity> ;
                                                      rdfs:comment "DEF: A MovingActivity in which the subject traffic participant keeps the same lane for the entire duration of the activity."^^xsd:string .


###  http://ontology.asam.net/ontologies/Domain#Lane
<http://ontology.asam.net/ontologies/Domain#Lane> rdf:type owl:Class ;
                                                  rdfs:subClassOf <http://ontology.asam.net/ontologies/Domain#LaneElement> ;
                                                  rdfs:comment "DEF: Lane is a  LaneElements that is a division of a road that is marked out by dividers, it is intended for use by traffic participants. The lane class contains the type of lanes that can be used to form part of the road"^^xsd:string .


###  http://ontology.asam.net/ontologies/Domain#LaneDivider
<http://ontology.asam.net/ontologies/Domain#LaneDivider> rdf:type owl:Class ;
                                                         rdfs:subClassOf <http://ontology.asam.net/ontologies/Domain#LaneElement> ;
                                                         rdfs:comment "DEF: LaneDivider is a LaneElement that is the extruded or painted component that separate one lane from the others. Typical lane dividers include lane markings and physical extrusion features such as guardrails or curbs."^^xsd:string .


###  http://ontology.asam.net/ontologies/Domain#LaneElement
<http://ontology.asam.net/ontologies/Domain#LaneElement> rdf:type owl:Class ;
                                                         rdfs:subClassOf <http://ontology.asam.net/ontologies/Domain#DrivableAreaElement> ;
                                                         rdfs:comment "DEF: A DriveableArea element that represents a part of a road, usually marked by lines, that is designed to be used by a single line of vehicles. Lanes may have different types, for example, dependent on the allowed vehicle types, and may have different characteristics, such as markings and curbs."^^xsd:string ,
                                                                      "EXAMPLES: bus lanes, HOV lanes, lanes with curbs, lanes with solid lines"^^xsd:string .


###  http://ontology.asam.net/ontologies/Domain#LaneForSpecificParticipants
<http://ontology.asam.net/ontologies/Domain#LaneForSpecificParticipants> rdf:type owl:Class ;
                                                                         rdfs:subClassOf <http://ontology.asam.net/ontologies/Domain#Lane> ;
                                                                         rdfs:comment "DEF: LaneForSpecificParticipants is a lane, which can be assoiated and categorized based on specific types of allowed traffic participants."^^xsd:string .


###  http://ontology.asam.net/ontologies/Domain#LaneMarking
<http://ontology.asam.net/ontologies/Domain#LaneMarking> rdf:type owl:Class ;
                                                         rdfs:subClassOf <http://ontology.asam.net/ontologies/Domain#LaneDivider> ,
                                                                         <http://ontology.asam.net/ontologies/Domain#RoadMarking> ;
                                                         rdfs:comment "DEF: LaneMarking is a type of LaneDivider, that is applied to individual indicating traffic rules such as lane change restriction."^^xsd:string .


###  http://ontology.asam.net/ontologies/Domain#LaneSection
<http://ontology.asam.net/ontologies/Domain#LaneSection> rdf:type owl:Class ;
                                                         rdfs:subClassOf <http://ontology.asam.net/ontologies/Domain#LaneElement> ;
                                                         rdfs:comment "DEF: LaneSection is a LaneElements. Lanes may be split into multiple lane sections. Each lane section contains a fixed number of lanes. Every time the number of lanes changes, a new lane section is required Lane sections are defined in ascending order along the road reference line."^^xsd:string .


###  http://ontology.asam.net/ontologies/Domain#LaneWithConstructionProperties
<http://ontology.asam.net/ontologies/Domain#LaneWithConstructionProperties> rdf:type owl:Class ;
                                                                            rdfs:subClassOf <http://ontology.asam.net/ontologies/Domain#Lane> ;
                                                                            rdfs:comment "DEF: LaneWithConstructionProperties is a lane, which can be assoiated and categorized based on surface material."^^xsd:string .


###  http://ontology.asam.net/ontologies/Domain#LaneWithSpecificRegulations
<http://ontology.asam.net/ontologies/Domain#LaneWithSpecificRegulations> rdf:type owl:Class ;
                                                                         rdfs:subClassOf <http://ontology.asam.net/ontologies/Domain#Lane> ;
                                                                         rdfs:comment "DEF: LaneWithSpecificRegulations is a lane, which can be assoiated and categorized based on allowed traffic function and rules."^^xsd:string .


###  http://ontology.asam.net/ontologies/Domain#LateralActivity
<http://ontology.asam.net/ontologies/Domain#LateralActivity> rdf:type owl:Class ;
                                                             rdfs:subClassOf <http://ontology.asam.net/ontologies/Domain#MovingActivity> ;
                                                             rdfs:comment "DEF: A MovingActivity which is characterized by sideways movement."^^xsd:string .


###  http://ontology.asam.net/ontologies/Domain#LightAir
<http://ontology.asam.net/ontologies/Domain#LightAir> rdf:type owl:Class ;
                                                      rdfs:subClassOf <http://ontology.asam.net/ontologies/Domain#WindCondition> ;
                                                      rdfs:comment "DEF: LightAir is a WindCondition, is it described by the WindSpeed property using m/s, LightAir is when the WindSpeed is 0.3-1.5 m/s."^^xsd:string .


###  http://ontology.asam.net/ontologies/Domain#LightBreeze
<http://ontology.asam.net/ontologies/Domain#LightBreeze> rdf:type owl:Class ;
                                                         rdfs:subClassOf <http://ontology.asam.net/ontologies/Domain#WindCondition> ;
                                                         rdfs:comment "DEF: LightBreeze is a WindCondition, is it described by the WindSpeed property using m/s, LightBreeze is when the WindSpeed is 1.6-3.3 m/s."^^xsd:string .


###  http://ontology.asam.net/ontologies/Domain#LightRain
<http://ontology.asam.net/ontologies/Domain#LightRain> rdf:type owl:Class ;
                                                       rdfs:subClassOf <http://ontology.asam.net/ontologies/Domain#RainfallCondition> ;
                                                       rdfs:comment "DEF: LightRain is a RainfallCondition, is it described by the precipitationIntensity property using mm/hr, LightRain is when the precipitationIntensity is < 2.5 mm/hr."^^xsd:string .


###  http://ontology.asam.net/ontologies/Domain#LightSnow
<http://ontology.asam.net/ontologies/Domain#LightSnow> rdf:type owl:Class ;
                                                       rdfs:subClassOf <http://ontology.asam.net/ontologies/Domain#SnowfallCondition> ;
                                                       rdfs:comment "DEF: LightSnow is a SnowfallCondition, is it described by the SnowfallIntensity property using visibility, LightSnowis is when the SnowfallIntensity is > 1.0 km."^^xsd:string .


###  http://ontology.asam.net/ontologies/Domain#LongitudinalActivity
<http://ontology.asam.net/ontologies/Domain#LongitudinalActivity> rdf:type owl:Class ;
                                                                  rdfs:subClassOf <http://ontology.asam.net/ontologies/Domain#MovingActivity> ;
                                                                  rdfs:comment "DEF: A MovingActivity which is characterized by lengthwise movement."^^xsd:string .


###  http://ontology.asam.net/ontologies/Domain#LooseSurface
<http://ontology.asam.net/ontologies/Domain#LooseSurface> rdf:type owl:Class ;
                                                          rdfs:subClassOf <http://ontology.asam.net/ontologies/Domain#RoadSurface> ;
                                                          rdfs:comment "DEF:LooseSurface is a  RoadSurface  that contains loose chippings such as loose gravel or stone fragments on a road surface"^^xsd:string ;
                                                          rdfs:label "LooseSurface" .


###  http://ontology.asam.net/ontologies/Domain#MakeALeftTurn
<http://ontology.asam.net/ontologies/Domain#MakeALeftTurn> rdf:type owl:Class ;
                                                           rdfs:subClassOf <http://ontology.asam.net/ontologies/Domain#MakeATurn> ;
                                                           rdfs:comment "DEF: A MakeATurn activity during which the subject traffic participant navigates through an intersection and exits the intersection on a road that is located to the left of the orginal road."^^xsd:string .


###  http://ontology.asam.net/ontologies/Domain#MakeARightTurn
<http://ontology.asam.net/ontologies/Domain#MakeARightTurn> rdf:type owl:Class ;
                                                            rdfs:subClassOf <http://ontology.asam.net/ontologies/Domain#MakeATurn> ;
                                                            rdfs:comment "DEF: A MakeATurn activity during which the subject traffic participant navigates through an intersection and exits the intersection on a road that is located to the right of the orginal road."^^xsd:string .


###  http://ontology.asam.net/ontologies/Domain#MakeATurn
<http://ontology.asam.net/ontologies/Domain#MakeATurn> rdf:type owl:Class ;
                                                       rdfs:subClassOf <http://ontology.asam.net/ontologies/Domain#DrivingActivity> ,
                                                                       <http://ontology.asam.net/ontologies/Domain#MissionLevelActivity> ,
                                                                       <http://ontology.asam.net/ontologies/Domain#SingleParticipantActivity> ;
                                                       rdfs:comment "DEF: A MovingActivity at mission level during which the subject traffic participant changes its direction in reference to a traffic infrastructure element, such as an intersection or a road, and has a different direction at the end of the activity."^^xsd:string .


###  http://ontology.asam.net/ontologies/Domain#ManeuverLevelActivity
<http://ontology.asam.net/ontologies/Domain#ManeuverLevelActivity> rdf:type owl:Class ;
                                                                   rdfs:subClassOf <http://ontology.asam.net/ontologies/Domain#ActivityByLevel> ;
                                                                   rdfs:comment "DEF: A set of activities with actions on maneuver level. This level contains abstract descriptions for the movements of a vehicle. It abstracts the physically continuous vehicle motion into a discrete logical state. This state is only partially observable from the outside. Every driving maneuver is linked to an intention."^^xsd:string .


###  http://ontology.asam.net/ontologies/Domain#Manhole
<http://ontology.asam.net/ontologies/Domain#Manhole> rdf:type owl:Class ;
                                                     rdfs:subClassOf <http://ontology.asam.net/ontologies/Domain#RoadSurfaceFeature> ;
                                                     rdfs:comment "DEF:Manhole is a  RoadSurfaceFeature  that is an opening in road to access canal system. Has to be big enough to fit a person and includes squared ones."^^xsd:string ;
                                                     rdfs:label "Manhole" .


###  http://ontology.asam.net/ontologies/Domain#MarineCondition
<http://ontology.asam.net/ontologies/Domain#MarineCondition> rdf:type owl:Class ;
                                                             rdfs:subClassOf <http://ontology.asam.net/ontologies/Domain#ParticulatesCondition> ;
                                                             rdfs:comment "DEF: A ParticulateCondition in an area near the sea where spray from the sea gets mixed into the atmosphere."^^xsd:string .


###  http://ontology.asam.net/ontologies/Domain#MinorRoad
<http://ontology.asam.net/ontologies/Domain#MinorRoad> rdf:type owl:Class ;
                                                       rdfs:subClassOf <http://ontology.asam.net/ontologies/Domain#Road> ;
                                                       rdfs:comment "DEF: MinorRoad is a  Road  that provides access to residential areas and other local developments."^^xsd:string .


###  http://ontology.asam.net/ontologies/Domain#MissionLevelActivity
<http://ontology.asam.net/ontologies/Domain#MissionLevelActivity> rdf:type owl:Class ;
                                                                  rdfs:subClassOf <http://ontology.asam.net/ontologies/Domain#ActivityByLevel> ;
                                                                  rdfs:comment "DEF: MissionLevelActivity is a ActivityByLevel, which structures the vehicle behavior at the level of mission or route planning and serves to achieve a higher-level goal. \"Mission elements are abstract task descriptions with no knowledge about how they will be executed by the system.\""^^xsd:string .


###  http://ontology.asam.net/ontologies/Domain#ModerateBreeze
<http://ontology.asam.net/ontologies/Domain#ModerateBreeze> rdf:type owl:Class ;
                                                            rdfs:subClassOf <http://ontology.asam.net/ontologies/Domain#WindCondition> ;
                                                            rdfs:comment "DEF: ModerateBreeze is a WindCondition, is it described by the WindSpeed property using m/s, ModerateBreeze is when the WindSpeed is 5.5-7.9 m/s."^^xsd:string .


###  http://ontology.asam.net/ontologies/Domain#ModerateRain
<http://ontology.asam.net/ontologies/Domain#ModerateRain> rdf:type owl:Class ;
                                                          rdfs:subClassOf <http://ontology.asam.net/ontologies/Domain#RainfallCondition> ;
                                                          rdfs:comment "DEF: ModerateRain is a RainfallCondition, is it described by the precipitationIntensity property using mm/hr, ModerateRain is when the precipitationIntensity is <2.5 - 7.6 mm/hr."^^xsd:string .


###  http://ontology.asam.net/ontologies/Domain#ModerateSnow
<http://ontology.asam.net/ontologies/Domain#ModerateSnow> rdf:type owl:Class ;
                                                          rdfs:subClassOf <http://ontology.asam.net/ontologies/Domain#SnowfallCondition> ;
                                                          rdfs:comment "DEF: ModerateSnow is a SnowfallCondition, is it described by the SnowfallIntensity property using visibility, ModerateSnow is when the SnowfallIntensity is 0.5 - 1.0 km."^^xsd:string .


###  http://ontology.asam.net/ontologies/Domain#Motorcycle
<http://ontology.asam.net/ontologies/Domain#Motorcycle> rdf:type owl:Class ;
                                                        rdfs:subClassOf <http://ontology.asam.net/ontologies/Domain#PrivateVehicle> ,
                                                                        <http://ontology.asam.net/ontologies/Domain#VRU> ;
                                                        rdfs:comment "DEF: A motor-powered Vehicle, also called motorbike or bike, that has two or three wheels and is used for transporting people."^^xsd:string .


###  http://ontology.asam.net/ontologies/Domain#Motorway
<http://ontology.asam.net/ontologies/Domain#Motorway> rdf:type owl:Class ;
                                                      rdfs:subClassOf <http://ontology.asam.net/ontologies/Domain#Road> ;
                                                      rdfs:comment "DEF: A Road that is designed for high speed and high traffic volume and has controlled entries and exits. Non-motorized vehicles and pedestrians are prohibited on motorways."^^xsd:string ,
                                                                   "EXAMPLES: UK: motorways, USA: highways, Germany: Autobahn"^^xsd:string .


###  http://ontology.asam.net/ontologies/Domain#MoveAway
<http://ontology.asam.net/ontologies/Domain#MoveAway> rdf:type owl:Class ;
                                                      rdfs:subClassOf <http://ontology.asam.net/ontologies/Domain#ActivityByTrafficParticipantType> ,
                                                                      <http://ontology.asam.net/ontologies/Domain#ManeuverLevelActivity> ,
                                                                      <http://ontology.asam.net/ontologies/Domain#MovingActivity> ,
                                                                      <http://ontology.asam.net/ontologies/Domain#MultiParticipantActivity> ;
                                                      rdfs:comment "DEF: A MovingActivity with moving traffic participants in which the subject traffic participant moves away from the object traffic participant."^^xsd:string .


###  http://ontology.asam.net/ontologies/Domain#MoveBackward
<http://ontology.asam.net/ontologies/Domain#MoveBackward> rdf:type owl:Class ;
                                                          rdfs:subClassOf <http://ontology.asam.net/ontologies/Domain#LongitudinalActivity> ,
                                                                          <http://ontology.asam.net/ontologies/Domain#PrimitiveLevelActivity> ,
                                                                          <http://ontology.asam.net/ontologies/Domain#SingleParticipantActivity> ;
                                                          rdfs:comment "DEF: An Activity with one traffic participant in which the traffic participant moves into the direction that is opposite to the original one without changing its orientation."^^xsd:string .


###  http://ontology.asam.net/ontologies/Domain#MovingActivity
<http://ontology.asam.net/ontologies/Domain#MovingActivity> rdf:type owl:Class ;
                                                            rdfs:subClassOf <http://ontology.asam.net/ontologies/Domain#ActivityByStateChange> ;
                                                            rdfs:comment "DEF: A set of activities which result in a changed location of the subject traffic participant."^^xsd:string .


###  http://ontology.asam.net/ontologies/Domain#MultiParticipantActivity
<http://ontology.asam.net/ontologies/Domain#MultiParticipantActivity> rdf:type owl:Class ;
                                                                      rdfs:subClassOf <http://ontology.asam.net/ontologies/Domain#ActivityByNumberOfParticipants> ;
                                                                      rdfs:comment "DEF: A set of activities which involve more than one traffic participant."^^xsd:string .


###  http://ontology.asam.net/ontologies/Domain#NearGale
<http://ontology.asam.net/ontologies/Domain#NearGale> rdf:type owl:Class ;
                                                      rdfs:subClassOf <http://ontology.asam.net/ontologies/Domain#WindCondition> ;
                                                      rdfs:comment "DEF: NearGale is a WindCondition, is it described by the WindSpeed property using m/s, NearGale is when the WindSpeed is 17.2-20.7 m/s."^^xsd:string .


###  http://ontology.asam.net/ontologies/Domain#NightLightingCondition
<http://ontology.asam.net/ontologies/Domain#NightLightingCondition> rdf:type owl:Class ;
                                                                    rdfs:subClassOf <http://ontology.asam.net/ontologies/Domain#IlluminationCondition> ;
                                                                    rdfs:comment "DEF: An IlluminationCondition where illuminance is below 1 lux."^^xsd:string .


###  http://ontology.asam.net/ontologies/Domain#NonVRU
<http://ontology.asam.net/ontologies/Domain#NonVRU> rdf:type owl:Class ;
                                                    rdfs:subClassOf <http://ontology.asam.net/ontologies/Domain#TrafficParticipantByVulnerability> ;
                                                    rdfs:comment "DEF: A set of non-vulnerable road users."^^xsd:string .


###  http://ontology.asam.net/ontologies/Domain#NotMove
<http://ontology.asam.net/ontologies/Domain#NotMove> rdf:type owl:Class ;
                                                     rdfs:subClassOf <http://ontology.asam.net/ontologies/Domain#MovingActivity> ,
                                                                     <http://ontology.asam.net/ontologies/Domain#PrimitiveLevelActivity> ,
                                                                     <http://ontology.asam.net/ontologies/Domain#SingleParticipantActivity> ;
                                                     rdfs:comment "DEF: An Activity during which the traffic participant has a speed of zero."^^xsd:string .


###  http://ontology.asam.net/ontologies/Domain#OfficialVehicle
<http://ontology.asam.net/ontologies/Domain#OfficialVehicle> rdf:type owl:Class ;
                                                             rdfs:subClassOf <http://ontology.asam.net/ontologies/Domain#Vehicle> ;
                                                             rdfs:comment "DEF: Official vehicles are vehicles with special access and operational authorities, such as ambulance, police vehicle"^^xsd:string .


###  http://ontology.asam.net/ontologies/Domain#Overcast
<http://ontology.asam.net/ontologies/Domain#Overcast> rdf:type owl:Class ;
                                                      rdfs:subClassOf <http://ontology.asam.net/ontologies/Domain#CloudCondition> ;
                                                      rdfs:comment "DEF: Overcast is a CloudCondition, is it described by the cloudinessLevel property using oktas unit, Overcast is when the cloudinessLevel is 8 oktas."^^xsd:string .


###  http://ontology.asam.net/ontologies/Domain#Overtake
<http://ontology.asam.net/ontologies/Domain#Overtake> rdf:type owl:Class ;
                                                      rdfs:subClassOf <http://ontology.asam.net/ontologies/Domain#DrivingActivity> ,
                                                                      <http://ontology.asam.net/ontologies/Domain#ManeuverLevelActivity> ,
                                                                      <http://ontology.asam.net/ontologies/Domain#MultiParticipantActivity> ;
                                                      rdfs:comment "DEF: An activity in which the subject traffic participant starts behind the object traffic participant and ends up in front of the object traffic participant. The subject changes lanes two time during the activity."^^xsd:string .


###  http://ontology.asam.net/ontologies/Domain#Parking
<http://ontology.asam.net/ontologies/Domain#Parking> rdf:type owl:Class ;
                                                     rdfs:subClassOf <http://ontology.asam.net/ontologies/Domain#Road> ;
                                                     rdfs:comment "DEF: A Road where vehicles are allowed to park."^^xsd:string .


###  http://ontology.asam.net/ontologies/Domain#ParticulatesCondition
<http://ontology.asam.net/ontologies/Domain#ParticulatesCondition> rdf:type owl:Class ;
                                                                   rdfs:subClassOf <http://ontology.asam.net/ontologies/Core#PhysicalProperty> ,
                                                                                   <http://ontology.asam.net/ontologies/Domain#EnvironmentalCondition> ;
                                                                   rdfs:comment "DEF: An EnvironmentalCondition where particles in the atmosphere lead to a limited visibility or obscuration of things. Particulates can be of different materials, for example water or sand."^^xsd:string .


###  http://ontology.asam.net/ontologies/Domain#Pass
<http://ontology.asam.net/ontologies/Domain#Pass> rdf:type owl:Class ;
                                                  rdfs:subClassOf <http://ontology.asam.net/ontologies/Domain#DrivingActivity> ,
                                                                  <http://ontology.asam.net/ontologies/Domain#ManeuverLevelActivity> ,
                                                                  <http://ontology.asam.net/ontologies/Domain#MultiParticipantActivity> ;
                                                  rdfs:comment "DEF: An activity in which the subject traffic participant is located in a lane adjacent to the lane in which the object traffic participant drives. The subject starts behind the object and is position ahead of the object at the end of the activity. The subject does not change lanes."^^xsd:string .


###  http://ontology.asam.net/ontologies/Domain#PavedShoulder
<http://ontology.asam.net/ontologies/Domain#PavedShoulder> rdf:type owl:Class ;
                                                           rdfs:subClassOf <http://ontology.asam.net/ontologies/Domain#LaneWithConstructionProperties> ;
                                                           rdfs:comment "DEF: PavedShoulder is a  LanesWithConstructionProperties that is an emergency stopping lane by the verge of a road or motorway. Hence, a shoulder, where the surface of a lane is paved is called paved shoulder"^^xsd:string .


###  http://ontology.asam.net/ontologies/Domain#Pedestrian
<http://ontology.asam.net/ontologies/Domain#Pedestrian> rdf:type owl:Class ;
                                                        rdfs:subClassOf <http://ontology.asam.net/ontologies/Domain#Human> ,
                                                                        <http://ontology.asam.net/ontologies/Domain#VRU> ;
                                                        rdfs:comment "DEF: A HumanParticipant who moves in traffic on foot."^^xsd:string .


###  http://ontology.asam.net/ontologies/Domain#PedestrianActivity
<http://ontology.asam.net/ontologies/Domain#PedestrianActivity> rdf:type owl:Class ;
                                                                rdfs:subClassOf <http://ontology.asam.net/ontologies/Domain#HumanActivity> ,
                                                                                <http://ontology.asam.net/ontologies/Domain#MovingActivity> ;
                                                                rdfs:comment "DEF: A set of activities performed by pedestrians."^^xsd:string .


###  http://ontology.asam.net/ontologies/Domain#PedestrianCrossing
<http://ontology.asam.net/ontologies/Domain#PedestrianCrossing> rdf:type owl:Class ;
                                                                rdfs:subClassOf <http://ontology.asam.net/ontologies/Domain#SpecialStructure> ;
                                                                rdfs:comment "DEF: A SpecialStructure that creates a place or area where pedestrians are able to cross a road or lane."^^xsd:string .


###  http://ontology.asam.net/ontologies/Domain#PedestrianZone
<http://ontology.asam.net/ontologies/Domain#PedestrianZone> rdf:type owl:Class ;
                                                            rdfs:subClassOf <http://ontology.asam.net/ontologies/Domain#TrafficZone> ;
                                                            rdfs:comment "DEF: A Zone where only pedestrians are allowed."^^xsd:string ,
                                                                         "EXAMPLES: city centers, parks, shopping areas"^^xsd:string .


###  http://ontology.asam.net/ontologies/Domain#PhysicalDivider
<http://ontology.asam.net/ontologies/Domain#PhysicalDivider> rdf:type owl:Class ;
                                                             rdfs:subClassOf <http://ontology.asam.net/ontologies/Domain#LaneElement> ;
                                                             rdfs:comment "DEF: PhysicalDivider is a LaneDivider that is a description of a way which has a physical or legal divider that divides opposing direction lanes and prevents crossing the way in a particular direction. In right side driving countries left turns and u-turns are not allowed, in left side driving countries right turns and u-turns are not allowed."^^xsd:string .


###  http://ontology.asam.net/ontologies/Domain#PositioningCondition
<http://ontology.asam.net/ontologies/Domain#PositioningCondition> rdf:type owl:Class ;
                                                                  rdfs:subClassOf <http://ontology.asam.net/ontologies/Domain#ConnectivityCondition> ;
                                                                  rdfs:comment "DEF: A ConnectivityCondition that specifies the system or mechanism used by a vehicle to determine its position. Examples: GPS and GLONASS."^^xsd:string .


###  http://ontology.asam.net/ontologies/Domain#Potholes
<http://ontology.asam.net/ontologies/Domain#Potholes> rdf:type owl:Class ;
                                                      rdfs:subClassOf <http://ontology.asam.net/ontologies/Domain#RoadSurfaceFeature> ;
                                                      rdfs:comment "DEF:Potholes is a  RoadSurfaceFeature  that is a depression in a road surface, usually asphalt pavement, where traffic has removed broken pieces of the pavement. It is usually the result of water in the underlying soil structure and traffic passing over the affected area"^^xsd:string ;
                                                      rdfs:label "Potholes" .


###  http://ontology.asam.net/ontologies/Domain#PrimitiveLevelActivity
<http://ontology.asam.net/ontologies/Domain#PrimitiveLevelActivity> rdf:type owl:Class ;
                                                                    rdfs:subClassOf <http://ontology.asam.net/ontologies/Domain#ActivityByLevel> ;
                                                                    rdfs:comment "DEF: A set of activities that describe the course of state variables through which a maneuver is to be implemented. While a maneuver is often defined relative to the traffic infrastructure, a motion primitive is defined in the vehicle coordinate system. A motion primitive can be a yaw rate, an acceleration or a deceleration."^^xsd:string .


###  http://ontology.asam.net/ontologies/Domain#PrivateVehicle
<http://ontology.asam.net/ontologies/Domain#PrivateVehicle> rdf:type owl:Class ;
                                                            rdfs:subClassOf <http://ontology.asam.net/ontologies/Domain#Vehicle> ;
                                                            rdfs:comment "DEF: Private vehicles are vehicles owned and used by private individuals."^^xsd:string .


###  http://ontology.asam.net/ontologies/Domain#PublicTransportationVehicle
<http://ontology.asam.net/ontologies/Domain#PublicTransportationVehicle> rdf:type owl:Class ;
                                                                         rdfs:subClassOf <http://ontology.asam.net/ontologies/Domain#Vehicle> ;
                                                                         rdfs:comment "DEF: Public transporation vehicles are vehicles operated to transport individuals from the public."^^xsd:string .


###  http://ontology.asam.net/ontologies/Domain#RadialRoad
<http://ontology.asam.net/ontologies/Domain#RadialRoad> rdf:type owl:Class ;
                                                        rdfs:subClassOf <http://ontology.asam.net/ontologies/Domain#Road> ;
                                                        rdfs:comment "DEF: A Road for high-density traffic that connects motorways to distributor roads or city centers."^^xsd:string .


###  http://ontology.asam.net/ontologies/Domain#RailCrossing
<http://ontology.asam.net/ontologies/Domain#RailCrossing> rdf:type owl:Class ;
                                                          rdfs:subClassOf <http://ontology.asam.net/ontologies/Domain#SpecialStructure> ;
                                                          rdfs:comment "DEF: A SpecialStructure that is an intersection between a road and a railway track."^^xsd:string .


###  http://ontology.asam.net/ontologies/Domain#RainfallCondition
<http://ontology.asam.net/ontologies/Domain#RainfallCondition> rdf:type owl:Class ;
                                                               rdfs:subClassOf <http://ontology.asam.net/ontologies/Domain#WeatherCondition> ;
                                                               rdfs:comment "DEF: A WeatherCondition where it is raining. The intensity of the rainfall may be described using the precipitationIntensity property."^^xsd:string .


###  http://ontology.asam.net/ontologies/Domain#RefuseCollection
<http://ontology.asam.net/ontologies/Domain#RefuseCollection> rdf:type owl:Class ;
                                                              rdfs:subClassOf <http://ontology.asam.net/ontologies/Domain#TemporaryRoadStructure> ;
                                                              rdfs:comment "DEF: A TemporaryRoadStructure that contains rubbish or waste that has not been disposed yet."^^xsd:string .


###  http://ontology.asam.net/ontologies/Domain#RegulatorySign
<http://ontology.asam.net/ontologies/Domain#RegulatorySign> rdf:type owl:Class ;
                                                            rdfs:subClassOf <http://ontology.asam.net/ontologies/Domain#TrafficSignByFunction> ;
                                                            rdfs:comment "DEF: A traffic sign that indicates rules, restrictions, and prohibitions for all or specific traffic participants."^^xsd:string ,
                                                                         "EXAMPLES: speed limit sign valid for trucks"^^xsd:string .


###  http://ontology.asam.net/ontologies/Domain#RestrictedLane
<http://ontology.asam.net/ontologies/Domain#RestrictedLane> rdf:type owl:Class ;
                                                            rdfs:subClassOf <http://ontology.asam.net/ontologies/Domain#LaneWithSpecificRegulations> ;
                                                            rdfs:comment "DEF: RestrictedLane is a  LaneWithSpecificRegulations that can have restrictions towards time, traffic participant type etc. For example, when two lanes split there is an area, where driving is forbidden."^^xsd:string .


###  http://ontology.asam.net/ontologies/Domain#Rider
<http://ontology.asam.net/ontologies/Domain#Rider> rdf:type owl:Class ;
                                                   rdfs:subClassOf <http://ontology.asam.net/ontologies/Domain#Human> ,
                                                                   <http://ontology.asam.net/ontologies/Domain#VRU> ;
                                                   rdfs:comment "DEF: A type of VRU which consists of a  human rider and the  transporting vehicle the rider is controlling, examples of such vehicles can be animal, bicycle, motorcycle, etc." .


###  http://ontology.asam.net/ontologies/Domain#RiderActivity
<http://ontology.asam.net/ontologies/Domain#RiderActivity> rdf:type owl:Class ;
                                                           rdfs:subClassOf <http://ontology.asam.net/ontologies/Domain#HumanActivity> ;
                                                           rdfs:comment "DEF: A BiologicalObjectActivity where the participant is a bicyclist or motorcyclist."^^xsd:string .


###  http://ontology.asam.net/ontologies/Domain#Road
<http://ontology.asam.net/ontologies/Domain#Road> rdf:type owl:Class ;
                                                  rdfs:subClassOf <http://ontology.asam.net/ontologies/Domain#DrivableAreaElement> ;
                                                  rdfs:comment "DEF: A DriveableArea that is a long stretch with a smooth or paved surface leading from one place to another. Made to be used by traffic participants."^^xsd:string .


###  http://ontology.asam.net/ontologies/Domain#RoadMarking
<http://ontology.asam.net/ontologies/Domain#RoadMarking> rdf:type owl:Class ;
                                                         rdfs:subClassOf <http://ontology.asam.net/ontologies/Domain#DrivableAreaElement> ;
                                                         rdfs:comment "DEF: A DriveableArea on a road surface that may consist of lines or other symbols and that conveys regulatory information about traffic rules."^^xsd:string ,
                                                                      "EXAMPLES: different types lane markings, such as solid or dashed lines"^^xsd:string .


###  http://ontology.asam.net/ontologies/Domain#RoadSignage
<http://ontology.asam.net/ontologies/Domain#RoadSignage> rdf:type owl:Class ;
                                                         rdfs:subClassOf <http://ontology.asam.net/ontologies/Domain#TemporaryRoadStructure> ;
                                                         rdfs:comment "DEF: A TemporaryRoadStructure that are signs or symbols on the road and that provide information about temporary changes to traffic routes, about road closures, construction works, detours, etc."^^xsd:string .


###  http://ontology.asam.net/ontologies/Domain#RoadStructureWithVegetation
<http://ontology.asam.net/ontologies/Domain#RoadStructureWithVegetation> rdf:type owl:Class ;
                                                                         rdfs:subClassOf <http://ontology.asam.net/ontologies/Domain#FixedRoadStructure> ;
                                                                         rdfs:comment "DEF: A FixedRoadStructure that consist of a several plants and the ground they cover."^^xsd:string .


###  http://ontology.asam.net/ontologies/Domain#RoadSurface
<http://ontology.asam.net/ontologies/Domain#RoadSurface> rdf:type owl:Class ;
                                                         rdfs:subClassOf <http://ontology.asam.net/ontologies/Domain#RoadSurfaceElement> ;
                                                         rdfs:comment "DEF:RoadSurface is a RoadSurfaceElement, which classify the road surface into different types based on characteristics of the surface material, for example segmented, uniform and loose."^^xsd:string ;
                                                         rdfs:label "RoadSurface" .


###  http://ontology.asam.net/ontologies/Domain#RoadSurfaceElement
<http://ontology.asam.net/ontologies/Domain#RoadSurfaceElement> rdf:type owl:Class ;
                                                                rdfs:subClassOf <http://ontology.asam.net/ontologies/Domain#DrivableAreaElement> ;
                                                                rdfs:comment "DEF: A DrivableArea on a road or sidewalk that is characterized by a specific surface, material, or coating."^^xsd:string ,
                                                                             "EXAMPLES: pavement, asphalt"^^xsd:string ,
                                                                             "RoadSurfaceElement is a DrivableAreaElement, which describes the surface material type and feature laid down on an area intended for traffic participants, such as a road or walkway." .


###  http://ontology.asam.net/ontologies/Domain#RoadSurfaceFeature
<http://ontology.asam.net/ontologies/Domain#RoadSurfaceFeature> rdf:type owl:Class ;
                                                                rdfs:subClassOf <http://ontology.asam.net/ontologies/Domain#RoadSurfaceElement> ;
                                                                rdfs:comment "DEF: RoadSurfaceFeature is a  RoadSurfaceElements. Drivable area surface features shall include damage caused by traffic and weather. Any road damage (and the resulting different surface features) shall be classified into cracks, potholes, ruts or swells."^^xsd:string ;
                                                                rdfs:label "RoadSurfaceFeature" .


###  http://ontology.asam.net/ontologies/Domain#RoadTopologyAndTrafficInfrastructure
<http://ontology.asam.net/ontologies/Domain#RoadTopologyAndTrafficInfrastructure> rdf:type owl:Class ;
                                                                                  rdfs:subClassOf <http://ontology.asam.net/ontologies/Domain#DomainConcepts> ;
                                                                                  rdfs:comment "DEF: A set of features for describing the logical road network, traffic infrastructure elements, and related conditions."^^xsd:string .


###  http://ontology.asam.net/ontologies/Domain#RoadWork
<http://ontology.asam.net/ontologies/Domain#RoadWork> rdf:type owl:Class ;
                                                      rdfs:subClassOf <http://ontology.asam.net/ontologies/Domain#TemporaryRoadStructure> ;
                                                      rdfs:comment "DEF: A TemporaryRoadStructure that is the part of a road under construction. As a result, the road layout may change."^^xsd:string .


###  http://ontology.asam.net/ontologies/Domain#Roadblocks
<http://ontology.asam.net/ontologies/Domain#Roadblocks> rdf:type owl:Class ;
                                                        rdfs:subClassOf <http://ontology.asam.net/ontologies/Domain#TemporaryRoadStructure> ;
                                                        rdfs:comment "DEF: A TemporaryRoadStructure that is set up to block or control traffic along a road."^^xsd:string ,
                                                                     "EXAMPLES: road block set up by law enforcement officers"^^xsd:string .


###  http://ontology.asam.net/ontologies/Domain#RoadwayEdgeElement
<http://ontology.asam.net/ontologies/Domain#RoadwayEdgeElement> rdf:type owl:Class ;
                                                                rdfs:subClassOf <http://ontology.asam.net/ontologies/Domain#FixedRoadStructure> ;
                                                                rdfs:comment "DEF: A FixedRoadStructure that forms the side boundary of a road."^^xsd:string ,
                                                                             "EXAMPLES: sound barriers, guard rails"^^xsd:string .


###  http://ontology.asam.net/ontologies/Domain#Roundabout
<http://ontology.asam.net/ontologies/Domain#Roundabout> rdf:type owl:Class ;
                                                        rdfs:subClassOf <http://ontology.asam.net/ontologies/Domain#Junction> ;
                                                        rdfs:comment "DEF: An Intersection where traffic moves into one direction in a circular shape around a central island to reach one of the roads leading into or out of the traffic circle. Roundabouts may have traffic signals."^^xsd:string .


###  http://ontology.asam.net/ontologies/Domain#Run
<http://ontology.asam.net/ontologies/Domain#Run> rdf:type owl:Class ;
                                                 rdfs:subClassOf <http://ontology.asam.net/ontologies/Domain#PedestrianActivity> ,
                                                                 <http://ontology.asam.net/ontologies/Domain#SingleParticipantActivity> ;
                                                 rdfs:comment "DEF: A PedestrianActivity where the biological object moves in such a way that at a specific point in time no foot touches the ground."^^xsd:string .


###  http://ontology.asam.net/ontologies/Domain#Ruts
<http://ontology.asam.net/ontologies/Domain#Ruts> rdf:type owl:Class ;
                                                  rdfs:subClassOf <http://ontology.asam.net/ontologies/Domain#RoadSurfaceFeature> ;
                                                  rdfs:comment "Ruts is a  RoadSurfaceFeature  that is a depression or groove worn into a road or path by the travel of wheels or skis. Ruts can be formed by wear, as from studded snow tires common in cold climate areas, or they can form through the deformation of the asphalt concrete, pavement or subbase material."^^xsd:string ;
                                                  rdfs:label "Ruts" .


###  http://ontology.asam.net/ontologies/Domain#SandCondition
<http://ontology.asam.net/ontologies/Domain#SandCondition> rdf:type owl:Class ;
                                                           rdfs:subClassOf <http://ontology.asam.net/ontologies/Domain#ParticulatesCondition> ;
                                                           rdfs:comment "DEF: A ParticulateCondition where the particles consist of sand or dust."^^xsd:string .


###  http://ontology.asam.net/ontologies/Domain#ScatteredClouds
<http://ontology.asam.net/ontologies/Domain#ScatteredClouds> rdf:type owl:Class ;
                                                             rdfs:subClassOf <http://ontology.asam.net/ontologies/Domain#CloudCondition> ;
                                                             rdfs:comment "DEF: ScatteredClouds is a CloudCondition, is it described by the cloudinessLevel property using oktas unit, ScatteredClouds is when the cloudinessLevel is 3-4 oktas."^^xsd:string .


###  http://ontology.asam.net/ontologies/Domain#SchoolZone
<http://ontology.asam.net/ontologies/Domain#SchoolZone> rdf:type owl:Class ;
                                                        rdfs:subClassOf <http://ontology.asam.net/ontologies/Domain#TrafficZone> ;
                                                        rdfs:comment "DEF: A Zone that is a road section near a school or near a crosswalk used by students. It is likely that younger pedestrians are present in this area."^^xsd:string .


###  http://ontology.asam.net/ontologies/Domain#SegmentedSurface
<http://ontology.asam.net/ontologies/Domain#SegmentedSurface> rdf:type owl:Class ;
                                                              rdfs:subClassOf <http://ontology.asam.net/ontologies/Domain#RoadSurface> ;
                                                              rdfs:comment "DEF:SegmentedSurface is a  RoadSurface  that consists of individual segments of certain type of surface material. An example of a segmented road surface could contain segments of concrete panels to form the surface."^^xsd:string ;
                                                              rdfs:label "SegmentedSurface" .


###  http://ontology.asam.net/ontologies/Domain#ServiceLane
<http://ontology.asam.net/ontologies/Domain#ServiceLane> rdf:type owl:Class ;
                                                         rdfs:subClassOf <http://ontology.asam.net/ontologies/Domain#LaneWithSpecificRegulations> ;
                                                         rdfs:comment "DEF: ServiceLane is a  LaneWithSpecificRegulations that which offer enough space for a car to drive and stop in emergency cases - typically on highways. Usually on the right side of drivable lanes, but can also be on the left side."^^xsd:string .


###  http://ontology.asam.net/ontologies/Domain#SharedSpace
<http://ontology.asam.net/ontologies/Domain#SharedSpace> rdf:type owl:Class ;
                                                         rdfs:subClassOf <http://ontology.asam.net/ontologies/Domain#Road> ;
                                                         rdfs:comment "DEF: A Road that may be used equally by vehicles and pedestrians. Shared spaces are designed to minimize the segregation between traffic participants.This is done by reducing traffic management features that tend to encourge users of vehicles to assume priority, such as curbs and lane markings."^^xsd:string .


###  http://ontology.asam.net/ontologies/Domain#Sidewalk
<http://ontology.asam.net/ontologies/Domain#Sidewalk> rdf:type owl:Class ;
                                                      rdfs:subClassOf <http://ontology.asam.net/ontologies/Domain#LaneForSpecificParticipants> ;
                                                      rdfs:comment "DEF: Sidewalk is a  LaneForSpecificParticipants that is designated for pedestrians or cyclist. Delimited from the road by some obstacles or poles, but not only by marking. Often elevated compared to the road and often located at the side of a road. Also includes walkable parts of traffic islands, but not pedestrian areas."^^xsd:string .


###  http://ontology.asam.net/ontologies/Domain#SingleParticipantActivity
<http://ontology.asam.net/ontologies/Domain#SingleParticipantActivity> rdf:type owl:Class ;
                                                                       rdfs:subClassOf <http://ontology.asam.net/ontologies/Domain#ActivityByNumberOfParticipants> ;
                                                                       rdfs:comment "DEF: A set of activities which involve exactly one traffic participant."^^xsd:string .


###  http://ontology.asam.net/ontologies/Domain#Slide
<http://ontology.asam.net/ontologies/Domain#Slide> rdf:type owl:Class ;
                                                   rdfs:subClassOf <http://ontology.asam.net/ontologies/Domain#PedestrianActivity> ,
                                                                   <http://ontology.asam.net/ontologies/Domain#SingleParticipantActivity> ;
                                                   rdfs:comment "DEF: A PedestrianActivity where the biological object moves in such a way that the feet always touch the ground."^^xsd:string .


###  http://ontology.asam.net/ontologies/Domain#SmokeAndDustCondition
<http://ontology.asam.net/ontologies/Domain#SmokeAndDustCondition> rdf:type owl:Class ;
                                                                   rdfs:subClassOf <http://ontology.asam.net/ontologies/Domain#ParticulatesCondition> ;
                                                                   rdfs:comment "DEF: A ParticulateCondition where the particles consist of smoke or pollution."^^xsd:string .


###  http://ontology.asam.net/ontologies/Domain#SnowfallCondition
<http://ontology.asam.net/ontologies/Domain#SnowfallCondition> rdf:type owl:Class ;
                                                               rdfs:subClassOf <http://ontology.asam.net/ontologies/Domain#WeatherCondition> ;
                                                               rdfs:comment "DEF: A WeatherCondition where it snows. The intensity of the snowfall may be described by the SnowfallIntensity property."^^xsd:string .


###  http://ontology.asam.net/ontologies/Domain#SolidLine
<http://ontology.asam.net/ontologies/Domain#SolidLine> rdf:type owl:Class ;
                                                       rdfs:subClassOf <http://ontology.asam.net/ontologies/Domain#LaneMarking> ;
                                                       rdfs:comment "DEF: SolidLine is a  LaneMarking that is  drawn on a two-way road and it indicates that traffic participants cannot overtake the vehicle ahead, or are not allowed to change the lanes."^^xsd:string .


###  http://ontology.asam.net/ontologies/Domain#SoundBarrier
<http://ontology.asam.net/ontologies/Domain#SoundBarrier> rdf:type owl:Class ;
                                                          rdfs:subClassOf <http://ontology.asam.net/ontologies/Domain#RoadwayEdgeElement> ;
                                                          rdfs:comment "DEF: A RoadwayEdgeElement that is an built structure designed to protect people in residential areas from noise pollution. Sound barriers are usually high walls next to roads."^^xsd:string .


###  http://ontology.asam.net/ontologies/Domain#SoundSiren
<http://ontology.asam.net/ontologies/Domain#SoundSiren> rdf:type owl:Class ;
                                                        rdfs:subClassOf <http://ontology.asam.net/ontologies/Domain#VehicleCommunicationActivity> ;
                                                        rdfs:comment "DEF: A VehicleCommunicatingActivity of an emergency vehicle that uses its siren to alert other traffic participants."^^xsd:string .


###  http://ontology.asam.net/ontologies/Domain#SpecialStructure
<http://ontology.asam.net/ontologies/Domain#SpecialStructure> rdf:type owl:Class ;
                                                              rdfs:subClassOf <http://ontology.asam.net/ontologies/Core#WholeLifeFunctionalSystem> ,
                                                                              <http://ontology.asam.net/ontologies/Core#WholeLifeFunctionalSystemComponent> ,
                                                                              <http://ontology.asam.net/ontologies/Core#WholeLifeSystemComponent> ,
                                                                              <http://ontology.asam.net/ontologies/Domain#RoadTopologyAndTrafficInfrastructure> ;
                                                              rdfs:comment "DEF: A set of traffic infrastructure types that are installed on road or junctions and on/through which cars can travel."^^xsd:string .


###  http://ontology.asam.net/ontologies/Domain#StaggeredIntersection
<http://ontology.asam.net/ontologies/Domain#StaggeredIntersection> rdf:type owl:Class ;
                                                                   rdfs:subClassOf <http://ontology.asam.net/ontologies/Domain#IntersectionAtGrade> ;
                                                                   rdfs:comment "DEF: An Intersection that consists of two T-junctions that directly follow each other. One intersection is vertically rotated by 180° in relation to the other intersection."^^xsd:string .


###  http://ontology.asam.net/ontologies/Domain#Stand
<http://ontology.asam.net/ontologies/Domain#Stand> rdf:type owl:Class ;
                                                   rdfs:subClassOf <http://ontology.asam.net/ontologies/Domain#PedestrianActivity> ,
                                                                   <http://ontology.asam.net/ontologies/Domain#SingleParticipantActivity> ;
                                                   rdfs:comment "DEF: A PedestrianActivity in which the biological object remains with both legs on the ground without moving in any direction."^^xsd:string .


###  http://ontology.asam.net/ontologies/Domain#Start
<http://ontology.asam.net/ontologies/Domain#Start> rdf:type owl:Class ;
                                                   rdfs:subClassOf <http://ontology.asam.net/ontologies/Domain#MovingActivity> ,
                                                                   <http://ontology.asam.net/ontologies/Domain#PrimitiveLevelActivity> ,
                                                                   <http://ontology.asam.net/ontologies/Domain#SingleParticipantActivity> ;
                                                   rdfs:comment "DEF: An Activity that starts with a speed of 0 for the subject traffic participant and ends with the traffic participant driving at a non-zero speed."^^xsd:string .


###  http://ontology.asam.net/ontologies/Domain#StaticTrafficSign
<http://ontology.asam.net/ontologies/Domain#StaticTrafficSign> rdf:type owl:Class ;
                                                               rdfs:subClassOf <http://ontology.asam.net/ontologies/Domain#TrafficSignByState> ;
                                                               rdfs:comment "DEF: A traffic sign whose content is static, meaning it does not change over time."^^xsd:string ,
                                                                            "EXAMPLES: fixed road signs like stop signs and speed limit signs"^^xsd:string .


###  http://ontology.asam.net/ontologies/Domain#Stop
<http://ontology.asam.net/ontologies/Domain#Stop> rdf:type owl:Class ;
                                                  rdfs:subClassOf <http://ontology.asam.net/ontologies/Domain#MovingActivity> ,
                                                                  <http://ontology.asam.net/ontologies/Domain#PrimitiveLevelActivity> ,
                                                                  <http://ontology.asam.net/ontologies/Domain#SingleParticipantActivity> ;
                                                  rdfs:comment "DEF: An Activity that starts with the subject traffic participant driving at a non-zero speed and ends with a speed of 0 for the subject."^^xsd:string .


###  http://ontology.asam.net/ontologies/Domain#StopLane
<http://ontology.asam.net/ontologies/Domain#StopLane> rdf:type owl:Class ;
                                                      rdfs:subClassOf <http://ontology.asam.net/ontologies/Domain#LaneWithSpecificRegulations> ;
                                                      rdfs:comment "DEF: StopLane is a  LaneWithSpecificRegulations that is on the side of a highway (typically paved). This lane is only allowed for emergency stopping."^^xsd:string .


###  http://ontology.asam.net/ontologies/Domain#Storm
<http://ontology.asam.net/ontologies/Domain#Storm> rdf:type owl:Class ;
                                                   rdfs:subClassOf <http://ontology.asam.net/ontologies/Domain#WindCondition> ;
                                                   rdfs:comment "DEF: Storm is a WindCondition, is it described by the WindSpeed property using m/s, Storm is when the WindSpeed is 24.5-28.4 m/s."^^xsd:string .


###  http://ontology.asam.net/ontologies/Domain#StreetFurniture
<http://ontology.asam.net/ontologies/Domain#StreetFurniture> rdf:type owl:Class ;
                                                             rdfs:subClassOf <http://ontology.asam.net/ontologies/Domain#FixedRoadStructure> ;
                                                             rdfs:comment "DEF: A FixedRoadStructure installed at or along a road. Street furniture may have different purposes, such as providing resting places, creating obstacles for traffic, or decorating."^^xsd:string ,
                                                                          "EXAMPLES: post boxes, benches, bollards, sculptures"^^xsd:string .


###  http://ontology.asam.net/ontologies/Domain#StreetLight
<http://ontology.asam.net/ontologies/Domain#StreetLight> rdf:type owl:Class ;
                                                         rdfs:subClassOf <http://ontology.asam.net/ontologies/Domain#FixedRoadStructure> ;
                                                         rdfs:comment "DEF: A FixedRoadStructure that is a manufactured source of light on the edge of the road."^^xsd:string ,
                                                                      "EXAMPLES: street lamps, light poles, lamp posts"^^xsd:string .


###  http://ontology.asam.net/ontologies/Domain#StreetLighting
<http://ontology.asam.net/ontologies/Domain#StreetLighting> rdf:type owl:Class ;
                                                            rdfs:subClassOf <http://ontology.asam.net/ontologies/Domain#ArtificialLightingCondition> ;
                                                            rdfs:comment "DEF: An ArtificialLightingCondition where the area in question is illuminated by lighting equipment installed along the road, typically mounted on tall posts."^^xsd:string .


###  http://ontology.asam.net/ontologies/Domain#StrongBreeze
<http://ontology.asam.net/ontologies/Domain#StrongBreeze> rdf:type owl:Class ;
                                                          rdfs:subClassOf <http://ontology.asam.net/ontologies/Domain#WindCondition> ;
                                                          rdfs:comment "DEF: StrongBreeze is a WindCondition, is it described by the WindSpeed property using m/s, StrongBreeze is when the WindSpeed is 10.8-13.8 m/s."^^xsd:string .


###  http://ontology.asam.net/ontologies/Domain#StrongGale
<http://ontology.asam.net/ontologies/Domain#StrongGale> rdf:type owl:Class ;
                                                        rdfs:subClassOf <http://ontology.asam.net/ontologies/Domain#WindCondition> ;
                                                        rdfs:comment "DEF: StrongGale is a WindCondition, is it described by the WindSpeed property using m/s, StrongGale is when the WindSpeed is 20.8-24.4 m/s."^^xsd:string .


###  http://ontology.asam.net/ontologies/Domain#Swells
<http://ontology.asam.net/ontologies/Domain#Swells> rdf:type owl:Class ;
                                                    rdfs:subClassOf <http://ontology.asam.net/ontologies/Domain#RoadSurfaceFeature> ;
                                                    rdfs:comment "DEF:Swells is a  RoadSurfaceFeature  that indicates a raised or elevated surface that was not part of the original road designs and can often be caused by the environmental conditions."^^xsd:string ;
                                                    rdfs:label "Swells" .


###  http://ontology.asam.net/ontologies/Domain#TIntersection
<http://ontology.asam.net/ontologies/Domain#TIntersection> rdf:type owl:Class ;
                                                           rdfs:subClassOf <http://ontology.asam.net/ontologies/Domain#IntersectionAtGrade> ;
                                                           rdfs:comment "DEF: An Intersection that consists of three roads. Two of the roads form a straight line, the third road meets the others at 90°. The resulting shape is similar to the capital letter T."^^xsd:string .


###  http://ontology.asam.net/ontologies/Domain#TemporaryRoadStructure
<http://ontology.asam.net/ontologies/Domain#TemporaryRoadStructure> rdf:type owl:Class ;
                                                                    rdfs:subClassOf <http://ontology.asam.net/ontologies/Core#WholeLifeFunctionalSystem> ,
                                                                                    <http://ontology.asam.net/ontologies/Core#WholeLifeFunctionalSystemComponent> ,
                                                                                    <http://ontology.asam.net/ontologies/Core#WholeLifeSystemComponent> ,
                                                                                    <http://ontology.asam.net/ontologies/Domain#RoadTopologyAndTrafficInfrastructure> ;
                                                                    rdfs:comment "DEF: A traffic infrastructure that is located on a road for limited period of time and because of specific situations, such as accidents, traffic guidance, or construction works"^^xsd:string ,
                                                                                 "EXAMPLES: temporary signs, traffic cones, construction site fencing"^^xsd:string .


###  http://ontology.asam.net/ontologies/Domain#TimeCondition
<http://ontology.asam.net/ontologies/Domain#TimeCondition> rdf:type owl:Class ;
                                                           rdfs:subClassOf <http://ontology.asam.net/ontologies/Core#PhysicalProperty> ,
                                                                           <http://ontology.asam.net/ontologies/Domain#EnvironmentalCondition> ;
                                                           rdfs:comment "DEF: An EnvironmentalCondition that gives information about the time when a specific traffic situation occurs. Time may be give as time of day, day of week, or date of year."^^xsd:string .


###  http://ontology.asam.net/ontologies/Domain#TollPlaza
<http://ontology.asam.net/ontologies/Domain#TollPlaza> rdf:type owl:Class ;
                                                       rdfs:subClassOf <http://ontology.asam.net/ontologies/Domain#SpecialStructure> ;
                                                       rdfs:comment "DEF: A SpecialStructure that contains toll roads, toll boths, and other structures for toll collection."^^xsd:string .


###  http://ontology.asam.net/ontologies/Domain#TrafficActivity
<http://ontology.asam.net/ontologies/Domain#TrafficActivity> rdf:type owl:Class ;
                                                             rdfs:subClassOf <http://ontology.asam.net/ontologies/Core#ActivityState> ,
                                                                             <http://ontology.asam.net/ontologies/Domain#TrafficParticipantAndBehavior> ;
                                                             rdfs:comment "DEF: An activity implies actions performed by traffic participants during a traffic situation, typically to achieve a specific goal, like changing a lane."^^xsd:string .


###  http://ontology.asam.net/ontologies/Domain#TrafficCone
<http://ontology.asam.net/ontologies/Domain#TrafficCone> rdf:type owl:Class ;
                                                         rdfs:subClassOf <http://ontology.asam.net/ontologies/Domain#TemporaryRoadStructure> ;
                                                         rdfs:comment "DEF: A TemporaryRoadStructure that is a solid or hollow cone-shaped marker that is place on roads or sidewalks to temporarily redirect the traffic."^^xsd:string ,
                                                                      "EXAMPLES: cones around a construction site"^^xsd:string .


###  http://ontology.asam.net/ontologies/Domain#TrafficIsland
<http://ontology.asam.net/ontologies/Domain#TrafficIsland> rdf:type owl:Class ;
                                                           rdfs:subClassOf <http://ontology.asam.net/ontologies/Domain#FixedRoadStructure> ;
                                                           rdfs:comment "DEF: A FixedRoadStructure that is located on the surface of a road and that serves to guide the traffic flow or protect pedestrians at crosswalks."^^xsd:string .


###  http://ontology.asam.net/ontologies/Domain#TrafficLane
<http://ontology.asam.net/ontologies/Domain#TrafficLane> rdf:type owl:Class ;
                                                         rdfs:subClassOf <http://ontology.asam.net/ontologies/Domain#LaneWithSpecificRegulations> ;
                                                         rdfs:comment "DEF: TrafficLane is a type of LaneWithSpecificRegulations. It is intended for motorist to use and not suitable for pedestrians, traffic stream is marked off on a road."^^xsd:string .


###  http://ontology.asam.net/ontologies/Domain#TrafficManagementZone
<http://ontology.asam.net/ontologies/Domain#TrafficManagementZone> rdf:type owl:Class ;
                                                                   rdfs:subClassOf <http://ontology.asam.net/ontologies/Domain#TrafficZone> ;
                                                                   rdfs:comment "DEF: A Zone that features infrastructure elements and measures to avoid peaks in the traffic density and create a smooth traffic flow on busy major traffic routes."^^xsd:string ,
                                                                                "EXAMPLES: Measures may include temporary lane closures, variable speed limits, and traffic redirections. Infrastructure elements may include dynamic traffic signs, temporary or non-existing lane markings, loading zones, and more."^^xsd:string .


###  http://ontology.asam.net/ontologies/Domain#TrafficParticipant
<http://ontology.asam.net/ontologies/Domain#TrafficParticipant> rdf:type owl:Class ;
                                                                rdfs:subClassOf <http://ontology.asam.net/ontologies/Core#Participant> ,
                                                                                <http://ontology.asam.net/ontologies/Core#WholeLifeSystemComponent> ,
                                                                                <http://ontology.asam.net/ontologies/Domain#TrafficParticipantAndBehavior> ;
                                                                rdfs:comment "DEF: Traffic participant is A state of a physical object that is participating actively in some traffic activity"^^xsd:string .


###  http://ontology.asam.net/ontologies/Domain#TrafficParticipantAndBehavior
<http://ontology.asam.net/ontologies/Domain#TrafficParticipantAndBehavior> rdf:type owl:Class ;
                                                                           rdfs:subClassOf <http://ontology.asam.net/ontologies/Domain#DomainConcepts> ;
                                                                           rdfs:comment "DEF: A set of activities, physical objects, and functional objects that describe traffic participants and their dynamic behavior."^^xsd:string .


###  http://ontology.asam.net/ontologies/Domain#TrafficParticipantByParticipantType
<http://ontology.asam.net/ontologies/Domain#TrafficParticipantByParticipantType> rdf:type owl:Class ;
                                                                                 rdfs:subClassOf <http://ontology.asam.net/ontologies/Domain#TrafficParticipant> ;
                                                                                 rdfs:comment "DEF: A set of traffic participants which are categorized by the individuals that participate in road traffic, such as vehicles or pedestrians."^^xsd:string .


###  http://ontology.asam.net/ontologies/Domain#TrafficParticipantByVulnerability
<http://ontology.asam.net/ontologies/Domain#TrafficParticipantByVulnerability> rdf:type owl:Class ;
                                                                               rdfs:subClassOf <http://ontology.asam.net/ontologies/Domain#TrafficParticipant> ;
                                                                               rdfs:comment "DEF: A set of traffic participants categorized by the probability and severity of injuries to people involved in a particular traffic situation."^^xsd:string .


###  http://ontology.asam.net/ontologies/Domain#TrafficSign
<http://ontology.asam.net/ontologies/Domain#TrafficSign> rdf:type owl:Class ;
                                                         rdfs:subClassOf <http://ontology.asam.net/ontologies/Core#WholeLifeSystemComponent> ,
                                                                         <http://ontology.asam.net/ontologies/Domain#RoadTopologyAndTrafficInfrastructure> ;
                                                         rdfs:comment "DEF: A traffic infrastructure element that is a sign located at the side or above a road to provide information or instructions to traffic participants."^^xsd:string ,
                                                                      "EXAMPLES: speed limit signs, warning signs"^^xsd:string .


###  http://ontology.asam.net/ontologies/Domain#TrafficSignByFunction
<http://ontology.asam.net/ontologies/Domain#TrafficSignByFunction> rdf:type owl:Class ;
                                                                   rdfs:subClassOf <http://ontology.asam.net/ontologies/Domain#TrafficSign> ;
                                                                   rdfs:comment "DEF: A set of traffic signs that groups signs according to type of content that they contain or which purpose they fulfil."^^xsd:string ,
                                                                                "EXAMPLE: possible types of content: warning, information message, speed limits"^^xsd:string .


###  http://ontology.asam.net/ontologies/Domain#TrafficSignByState
<http://ontology.asam.net/ontologies/Domain#TrafficSignByState> rdf:type owl:Class ;
                                                                rdfs:subClassOf <http://ontology.asam.net/ontologies/Domain#TrafficSign> ;
                                                                rdfs:comment "DEF: A set of traffic signs that groups signs depending on whether their content can be changed dynamically or is static."^^xsd:string .


###  http://ontology.asam.net/ontologies/Domain#TrafficZone
<http://ontology.asam.net/ontologies/Domain#TrafficZone> rdf:type owl:Class ;
                                                         rdfs:subClassOf <http://ontology.asam.net/ontologies/Core#SpatialLocation> ,
                                                                         <http://ontology.asam.net/ontologies/Core#WholeLifeSystemComponent> ,
                                                                         <http://ontology.asam.net/ontologies/Domain#RoadTopologyAndTrafficInfrastructure> ;
                                                         rdfs:comment "DEF: A geographic area with special road configurations, driving regulations, or environmental conditions. The boundaries of a zone may be fixed or dynamic. The conditions that define a zone may be based on complexity, operating procedures, or other factors."^^xsd:string ,
                                                                      "EXAMPLES: zones where autonomous cars can operate safely"^^xsd:string .


###  http://ontology.asam.net/ontologies/Domain#Trailer
<http://ontology.asam.net/ontologies/Domain#Trailer> rdf:type owl:Class ;
                                                     rdfs:subClassOf <http://ontology.asam.net/ontologies/Domain#NonVRU> ,
                                                                     <http://ontology.asam.net/ontologies/Domain#PrivateVehicle> ;
                                                     rdfs:comment "DEF: An unpowered Vehicle that is designed for being towed by another Vehicle."^^xsd:string .


###  http://ontology.asam.net/ontologies/Domain#Truck
<http://ontology.asam.net/ontologies/Domain#Truck> rdf:type owl:Class ;
                                                   rdfs:subClassOf <http://ontology.asam.net/ontologies/Domain#GoodsVehicle> ,
                                                                   <http://ontology.asam.net/ontologies/Domain#NonVRU> ;
                                                   rdfs:comment "DEF: A large and heavy road Vehicle designed and used for carrying goods and materials."^^xsd:string .


###  http://ontology.asam.net/ontologies/Domain#Tunnel
<http://ontology.asam.net/ontologies/Domain#Tunnel> rdf:type owl:Class ;
                                                    rdfs:subClassOf <http://ontology.asam.net/ontologies/Domain#SpecialStructure> ;
                                                    rdfs:comment "DEF: A SpecialStructure that is a built underground passage through or below a natural or built structure."^^xsd:string .


###  http://ontology.asam.net/ontologies/Domain#Turn
<http://ontology.asam.net/ontologies/Domain#Turn> rdf:type owl:Class ;
                                                  rdfs:subClassOf <http://ontology.asam.net/ontologies/Domain#MovingActivity> ,
                                                                  <http://ontology.asam.net/ontologies/Domain#PrimitiveLevelActivity> ,
                                                                  <http://ontology.asam.net/ontologies/Domain#SingleParticipantActivity> ;
                                                  rdfs:comment "DEF: An Activity during which the subject traffic participant changes its orientation."^^xsd:string .


###  http://ontology.asam.net/ontologies/Domain#UndividedRoad
<http://ontology.asam.net/ontologies/Domain#UndividedRoad> rdf:type owl:Class ;
                                                           rdfs:subClassOf <http://ontology.asam.net/ontologies/Domain#Road> ;
                                                           rdfs:comment "DEF: A type of road where traffic travels in both directions; the directions are not separated by a central reservation."^^xsd:string .


###  http://ontology.asam.net/ontologies/Domain#UniformSurface
<http://ontology.asam.net/ontologies/Domain#UniformSurface> rdf:type owl:Class ;
                                                            rdfs:subClassOf <http://ontology.asam.net/ontologies/Domain#RoadSurface> ;
                                                            rdfs:comment "DEF:UniformSurface is a  RoadSurface  where the surface material is distributed evenly."^^xsd:string ;
                                                            rdfs:label "UniformSurface" .


###  http://ontology.asam.net/ontologies/Domain#UseHazardLight
<http://ontology.asam.net/ontologies/Domain#UseHazardLight> rdf:type owl:Class ;
                                                            rdfs:subClassOf <http://ontology.asam.net/ontologies/Domain#VehicleCommunicationActivity> ;
                                                            rdfs:comment "DEF: A VehicleCommunicatingActivity where a vehicle uses its hazard warning lights to warn other traffic participants of a dangerous situation or malfunction of the vehicle."^^xsd:string .


###  http://ontology.asam.net/ontologies/Domain#UseTurnIndicator
<http://ontology.asam.net/ontologies/Domain#UseTurnIndicator> rdf:type owl:Class ;
                                                              rdfs:subClassOf <http://ontology.asam.net/ontologies/Domain#VehicleCommunicationActivity> ;
                                                              rdfs:comment "DEF: A VehicleCommunicatingActivity in which the subject vehicle uses its direction indicator light to indicate its intention of turning, changing lane, or similar."^^xsd:string .


###  http://ontology.asam.net/ontologies/Domain#V2I
<http://ontology.asam.net/ontologies/Domain#V2I> rdf:type owl:Class ;
                                                 rdfs:subClassOf <http://ontology.asam.net/ontologies/Domain#CommunicationCondition> ;
                                                 rdfs:comment "DEF: A CommunicationCondition that enables communication between a vehicle and the surrounding infrastructure."^^xsd:string .


###  http://ontology.asam.net/ontologies/Domain#V2V
<http://ontology.asam.net/ontologies/Domain#V2V> rdf:type owl:Class ;
                                                 rdfs:subClassOf <http://ontology.asam.net/ontologies/Domain#CommunicationCondition> ;
                                                 rdfs:comment "DEF: A CommunicationCondition that enables communication between a vehicle and other vehicles in a traffic situation."^^xsd:string .


###  http://ontology.asam.net/ontologies/Domain#VRU
<http://ontology.asam.net/ontologies/Domain#VRU> rdf:type owl:Class ;
                                                 rdfs:subClassOf <http://ontology.asam.net/ontologies/Domain#TrafficParticipantByVulnerability> ;
                                                 rdfs:comment "DEF: Set of vulnerable road users (VRU) which are non-motorized traffic participants with reduce mobilities and orientation. A VRU includes both the mobility device (if applicable) and the human that controls it."^^xsd:string ,
                                                              "EXAMPLES: pedestriants, cyclists, motorcyclist, people with disabilities"^^xsd:string .


###  http://ontology.asam.net/ontologies/Domain#Van
<http://ontology.asam.net/ontologies/Domain#Van> rdf:type owl:Class ;
                                                 rdfs:subClassOf <http://ontology.asam.net/ontologies/Domain#GoodsVehicle> ,
                                                                 <http://ontology.asam.net/ontologies/Domain#NonVRU> ;
                                                 rdfs:comment "DEF: A medium sized, motor-powered Vehicle, usually without rear side windows, that is used for transporting goods."^^xsd:string .


###  http://ontology.asam.net/ontologies/Domain#Vehicle
<http://ontology.asam.net/ontologies/Domain#Vehicle> rdf:type owl:Class ;
                                                     rdfs:subClassOf <http://ontology.asam.net/ontologies/Domain#TrafficParticipantByParticipantType> ;
                                                     rdfs:comment "DEF: A machine that is a TrafficFunctionalObject which has the intended role of transporting things like goods, humans, or animals. Vehicles are participants in traffic-related activities."^^xsd:string .


###  http://ontology.asam.net/ontologies/Domain#VehicleActivity
<http://ontology.asam.net/ontologies/Domain#VehicleActivity> rdf:type owl:Class ;
                                                             rdfs:subClassOf <http://ontology.asam.net/ontologies/Domain#ActivityByTrafficParticipantType> ;
                                                             rdfs:comment "DEF: A set of activities performed by vehicles."^^xsd:string .


###  http://ontology.asam.net/ontologies/Domain#VehicleCommunicationActivity
<http://ontology.asam.net/ontologies/Domain#VehicleCommunicationActivity> rdf:type owl:Class ;
                                                                          rdfs:subClassOf <http://ontology.asam.net/ontologies/Domain#CommunicationActivity> ,
                                                                                          <http://ontology.asam.net/ontologies/Domain#VehicleActivity> ;
                                                                          rdfs:comment "DEF: A CommunicatingActivity where the subject is a vehicle."^^xsd:string .


###  http://ontology.asam.net/ontologies/Domain#VehicleLighting
<http://ontology.asam.net/ontologies/Domain#VehicleLighting> rdf:type owl:Class ;
                                                             rdfs:subClassOf <http://ontology.asam.net/ontologies/Domain#ArtificialLightingCondition> ;
                                                             rdfs:comment "DEF: An ArtificialLightingCondition where the area in question is illuminated by lighting or signaling equipment installed on vehicles, for example, headlights."^^xsd:string .


###  http://ontology.asam.net/ontologies/Domain#VehicleRestrictionArea
<http://ontology.asam.net/ontologies/Domain#VehicleRestrictionArea> rdf:type owl:Class ;
                                                                    rdfs:subClassOf <http://ontology.asam.net/ontologies/Domain#TrafficZone> ;
                                                                    rdfs:comment "DEF: A Zone where specific types of traffic participants are not allowed to travel."^^xsd:string ,
                                                                                 "EXAMPLES: zone forbidden for cars or motorcycles"^^xsd:string .


###  http://ontology.asam.net/ontologies/Domain#ViolentRain
<http://ontology.asam.net/ontologies/Domain#ViolentRain> rdf:type owl:Class ;
                                                         rdfs:subClassOf <http://ontology.asam.net/ontologies/Domain#RainfallCondition> ;
                                                         rdfs:comment "DEF: ViolentRain is a RainfallCondition, is it described by the precipitationIntensity property using mm/hr, ViolentRain is when the precipitationIntensity is < 50 -100 mm/hr."^^xsd:string .


###  http://ontology.asam.net/ontologies/Domain#ViolentStorm
<http://ontology.asam.net/ontologies/Domain#ViolentStorm> rdf:type owl:Class ;
                                                          rdfs:subClassOf <http://ontology.asam.net/ontologies/Domain#WindCondition> ;
                                                          rdfs:comment "DEF: ViolentStorm is a WindCondition, is it described by the WindSpeed property using m/s, ViolentStorm is when the WindSpeed is 28.5-32.6 m/s."^^xsd:string .


###  http://ontology.asam.net/ontologies/Domain#Walk
<http://ontology.asam.net/ontologies/Domain#Walk> rdf:type owl:Class ;
                                                  rdfs:subClassOf <http://ontology.asam.net/ontologies/Domain#PedestrianActivity> ,
                                                                  <http://ontology.asam.net/ontologies/Domain#SingleParticipantActivity> ;
                                                  rdfs:comment "DEF: A PedestrianActivity where the biological object moves in such a way that at least one foot is always on the ground."^^xsd:string .


###  http://ontology.asam.net/ontologies/Domain#WallOnRoadEdge
<http://ontology.asam.net/ontologies/Domain#WallOnRoadEdge> rdf:type owl:Class ;
                                                            rdfs:subClassOf <http://ontology.asam.net/ontologies/Domain#RoadwayEdgeElement> ;
                                                            rdfs:comment "DEF: A RoadwayEdgeElement that is a vertical structure built from brick or stone and that separates the road from the surrounding area of land."^^xsd:string .


###  http://ontology.asam.net/ontologies/Domain#WarningSign
<http://ontology.asam.net/ontologies/Domain#WarningSign> rdf:type owl:Class ;
                                                         rdfs:subClassOf <http://ontology.asam.net/ontologies/Domain#TrafficSignByFunction> ;
                                                         rdfs:comment "DEF: A traffic sign that warns traffic participants of potential dangers ahead so that these can react accordingly, for example, reduce speed."^^xsd:string .


###  http://ontology.asam.net/ontologies/Domain#Wave
<http://ontology.asam.net/ontologies/Domain#Wave> rdf:type owl:Class ;
                                                  rdfs:subClassOf :HumanCommunicationActivity ;
                                                  rdfs:comment "DEF: An Activity of a human traffic participant which waves a hand to indicate their intention."^^xsd:string .


###  http://ontology.asam.net/ontologies/Domain#WeatherCondition
<http://ontology.asam.net/ontologies/Domain#WeatherCondition> rdf:type owl:Class ;
                                                              rdfs:subClassOf <http://ontology.asam.net/ontologies/Core#PhysicalProperty> ,
                                                                              <http://ontology.asam.net/ontologies/Domain#EnvironmentalCondition> ;
                                                              rdfs:comment "DEF: An EnvironmentalCondition that comprises the characteristics of the atmosphere in terms of wind, rain, fog, snowfall and other natural phenomena."^^xsd:string .


###  http://ontology.asam.net/ontologies/Domain#Wheelchair
<http://ontology.asam.net/ontologies/Domain#Wheelchair> rdf:type owl:Class ;
                                                        rdfs:subClassOf <http://ontology.asam.net/ontologies/Domain#PrivateVehicle> ,
                                                                        <http://ontology.asam.net/ontologies/Domain#VRU> ;
                                                        rdfs:comment "DEF: A traffic participant which consists of a (handicapped) person sitting in a chair that is equipped with wheels. The person uses the chair as means of transport."^^xsd:string .


###  http://ontology.asam.net/ontologies/Domain#WindCondition
<http://ontology.asam.net/ontologies/Domain#WindCondition> rdf:type owl:Class ;
                                                           rdfs:subClassOf <http://ontology.asam.net/ontologies/Domain#WeatherCondition> ;
                                                           rdfs:comment "DEF: A WeatherCondition that defines the wind properties within a traffic situation. Properties can include speed, direction, and other characteristics."^^xsd:string .


###  http://ontology.asam.net/ontologies/Domain#YIntersection
<http://ontology.asam.net/ontologies/Domain#YIntersection> rdf:type owl:Class ;
                                                           rdfs:subClassOf <http://ontology.asam.net/ontologies/Domain#IntersectionAtGrade> ;
                                                           rdfs:comment "DEF: An Intersection with three roads that has the shape of the capital letter Y."^^xsd:string .


###  http://ontology.asam.net/ontologies/Domain#arc
<http://ontology.asam.net/ontologies/Domain#arc> rdf:type owl:Class ;
                                                 rdfs:subClassOf <http://ontology.asam.net/ontologies/Domain#curve> ;
                                                 rdfs:comment "DEF: A Curve with a constant curvature."^^xsd:string .


###  http://ontology.asam.net/ontologies/Domain#atmosphericPressure
<http://ontology.asam.net/ontologies/Domain#atmosphericPressure> rdf:type owl:Class ;
                                                                 rdfs:subClassOf <http://ontology.asam.net/ontologies/Domain#environmentalConditionProperty> ;
                                                                 rdfs:comment "DEF: An environmentalConditionProperty that specifies the force per given area unit exerted by the atmosphere. Pascal is used as unit of measurement; values may range from 0 to infinity."^^xsd:string .


###  http://ontology.asam.net/ontologies/Domain#cloudinessLevel
<http://ontology.asam.net/ontologies/Domain#cloudinessLevel> rdf:type owl:Class ;
                                                             rdfs:subClassOf <http://ontology.asam.net/ontologies/Domain#environmentalConditionProperty> ;
                                                             rdfs:comment "DEF: An environmentalConditionProperty that determines the amount of sky covered in clouds. Okta is used as unit of measurement."^^xsd:string .


###  http://ontology.asam.net/ontologies/Domain#contaminatingRoadCondition
<http://ontology.asam.net/ontologies/Domain#contaminatingRoadCondition> rdf:type owl:Class ;
                                                                        rdfs:subClassOf <http://ontology.asam.net/ontologies/Domain#inducedRoadSurfaceCondition> ;
                                                                        rdfs:comment "DEF: An InducedRoadSurfaceCondition where the road surface is covered with substances or a mix of substances and other materials."^^xsd:string ,
                                                                                     "EXAMPLES: Substances may include chemicals and oil; materials may include leaves, mud, or rocks."^^xsd:string .


###  http://ontology.asam.net/ontologies/Domain#curve
<http://ontology.asam.net/ontologies/Domain#curve> rdf:type owl:Class ;
                                                   rdfs:subClassOf <http://ontology.asam.net/ontologies/Domain#horizontalGeometry> ;
                                                   rdfs:comment "DEF: A HorizontalGeometry that is not straight."^^xsd:string .


###  http://ontology.asam.net/ontologies/Domain#downSlope
<http://ontology.asam.net/ontologies/Domain#downSlope> rdf:type owl:Class ;
                                                       rdfs:subClassOf <http://ontology.asam.net/ontologies/Domain#verticalGeometry> ;
                                                       rdfs:comment "DEF: A VerticalGeometry that is a plane with negative gradient. It represents a descending elevation of the road in driving direction."^^xsd:string .


###  http://ontology.asam.net/ontologies/Domain#drivableAreaGeometry
<http://ontology.asam.net/ontologies/Domain#drivableAreaGeometry> rdf:type owl:Class ;
                                                                  rdfs:subClassOf <http://ontology.asam.net/ontologies/Domain#roadTopologyAndTrafficInfrastructureProperty> ;
                                                                  rdfs:comment "DEF: Shape of a drivable area described as geometry."^^xsd:string .


###  http://ontology.asam.net/ontologies/Domain#drivingDirection
<http://ontology.asam.net/ontologies/Domain#drivingDirection> rdf:type owl:Class ;
                                                              rdfs:subClassOf <http://ontology.asam.net/ontologies/Domain#roadTopologyAndTrafficInfrastructureProperty> ;
                                                              rdfs:comment "DEF: A traffic infrastructure property that indicates whether traffic participants keep on the left or right side of the road in birectional travel."^^xsd:string .


###  http://ontology.asam.net/ontologies/Domain#environmentalConditionProperty
<http://ontology.asam.net/ontologies/Domain#environmentalConditionProperty> rdf:type owl:Class ;
                                                                            rdfs:subClassOf <http://ontology.asam.net/ontologies/Core#PhysicalProperty> ,
                                                                                            <http://ontology.asam.net/ontologies/Domain#EnvironmentalCondition> .


###  http://ontology.asam.net/ontologies/Domain#floodedRoadCondition
<http://ontology.asam.net/ontologies/Domain#floodedRoadCondition> rdf:type owl:Class ;
                                                                  rdfs:subClassOf <http://ontology.asam.net/ontologies/Domain#inducedRoadSurfaceCondition> ;
                                                                  rdfs:comment "DEF: An InducedRoadSurfaceCondition where the road is covered with flowing water, especially from rain."^^xsd:string ,
                                                                               "EXAMPLES: Flooded roads occur when more water rains down on the road than the sewage system can drain away."^^xsd:string .


###  http://ontology.asam.net/ontologies/Domain#horizontalGeometry
<http://ontology.asam.net/ontologies/Domain#horizontalGeometry> rdf:type owl:Class ;
                                                                rdfs:subClassOf <http://ontology.asam.net/ontologies/Domain#drivableAreaGeometry> ;
                                                                rdfs:comment "DEF: A DrivableAreaGeometry in the horizontal plane"^^xsd:string .


###  http://ontology.asam.net/ontologies/Domain#icyRoadCondition
<http://ontology.asam.net/ontologies/Domain#icyRoadCondition> rdf:type owl:Class ;
                                                              rdfs:subClassOf <http://ontology.asam.net/ontologies/Domain#inducedRoadSurfaceCondition> ;
                                                              rdfs:comment "DEF: An InducedRoadSurfaceCondition where the road is completely or partially covered with ice."^^xsd:string .


###  http://ontology.asam.net/ontologies/Domain#inducedRoadSurfaceCondition
<http://ontology.asam.net/ontologies/Domain#inducedRoadSurfaceCondition> rdf:type owl:Class ;
                                                                         rdfs:subClassOf <http://ontology.asam.net/ontologies/Domain#roadTopologyAndTrafficInfrastructureProperty> ;
                                                                         rdfs:comment "DEF: A traffic infrastructure property that describes the conditions on the road surface caused by environmental influences, such as rain or snow."^^xsd:string .


###  http://ontology.asam.net/ontologies/Domain#laneDimension
<http://ontology.asam.net/ontologies/Domain#laneDimension> rdf:type owl:Class ;
                                                           rdfs:subClassOf <http://ontology.asam.net/ontologies/Domain#laneProperty> ;
                                                           rdfs:comment "DEF: A LaneProperty that is the width of the lane."^^xsd:string .


###  http://ontology.asam.net/ontologies/Domain#laneMarkingColor
<http://ontology.asam.net/ontologies/Domain#laneMarkingColor> rdf:type owl:Class ;
                                                              rdfs:subClassOf <http://ontology.asam.net/ontologies/Domain#laneProperty> ;
                                                              rdfs:comment "DEF: A LaneProperty that is the colour of the lane marking."^^xsd:string .


###  http://ontology.asam.net/ontologies/Domain#laneMarkingWidth
<http://ontology.asam.net/ontologies/Domain#laneMarkingWidth> rdf:type owl:Class ;
                                                              rdfs:subClassOf <http://ontology.asam.net/ontologies/Domain#laneProperty> ;
                                                              rdfs:comment "DEF: A LaneProperty that is the width of the lane marking."^^xsd:string .


###  http://ontology.asam.net/ontologies/Domain#laneProperty
<http://ontology.asam.net/ontologies/Domain#laneProperty> rdf:type owl:Class ;
                                                          rdfs:subClassOf <http://ontology.asam.net/ontologies/Domain#roadTopologyAndTrafficInfrastructureProperty> ;
                                                          rdfs:comment "DEF: A traffic infrastructure property that describes the characteristics of a lane."^^xsd:string .


###  http://ontology.asam.net/ontologies/Domain#lateralProfile
<http://ontology.asam.net/ontologies/Domain#lateralProfile> rdf:type owl:Class ;
                                                            rdfs:subClassOf <http://ontology.asam.net/ontologies/Domain#transverseGeometry> ;
                                                            rdfs:comment "DEF: A TransverseGeometry that specifies the elevation of a road orthogonally to a reference line."^^xsd:string .


###  http://ontology.asam.net/ontologies/Domain#levelPlane
<http://ontology.asam.net/ontologies/Domain#levelPlane> rdf:type owl:Class ;
                                                        rdfs:subClassOf <http://ontology.asam.net/ontologies/Domain#verticalGeometry> ;
                                                        rdfs:comment "DEF: A VerticalGeometry that is a plane with a gradient of 0. All points of the plane are on the same vertical level."^^xsd:string .


###  http://ontology.asam.net/ontologies/Domain#lightingIntensity
<http://ontology.asam.net/ontologies/Domain#lightingIntensity> rdf:type owl:Class ;
                                                               rdfs:subClassOf <http://ontology.asam.net/ontologies/Domain#environmentalConditionProperty> ;
                                                               rdfs:comment "DEF: An environmentalConditionProperty that describes the intensity of illumination by a lighting source. Lux is used as unit of measurement."^^xsd:string .


###  http://ontology.asam.net/ontologies/Domain#mirageRoadCondition
<http://ontology.asam.net/ontologies/Domain#mirageRoadCondition> rdf:type owl:Class ;
                                                                 rdfs:subClassOf <http://ontology.asam.net/ontologies/Domain#inducedRoadSurfaceCondition> ;
                                                                 rdfs:comment "DEF: An InducedRoadSurfaceCondition where displaced images of distant objects or the sky appear. A mirage is a natural optical phenomenon caused by the bending of light rays via refraction."^^xsd:string .


###  http://ontology.asam.net/ontologies/Domain#numberOfLanes
<http://ontology.asam.net/ontologies/Domain#numberOfLanes> rdf:type owl:Class ;
                                                           rdfs:subClassOf <http://ontology.asam.net/ontologies/Domain#roadTopologyAndTrafficInfrastructureProperty> ;
                                                           rdfs:comment "DEF: A traffic infrastructure property that indicates how many lanes a road has."^^xsd:string .


###  http://ontology.asam.net/ontologies/Domain#precipitationIntensity
<http://ontology.asam.net/ontologies/Domain#precipitationIntensity> rdf:type owl:Class ;
                                                                    rdfs:subClassOf <http://ontology.asam.net/ontologies/Domain#environmentalConditionProperty> ;
                                                                    rdfs:comment "DEF: An environmentalConditionProperty that measures the level of rainfall. mm/hr is used as unit of measurement. It gives the amount or volume of water per fixed amount of time (hour)."^^xsd:string .


###  http://ontology.asam.net/ontologies/Domain#roadFrictionScaleFactor
<http://ontology.asam.net/ontologies/Domain#roadFrictionScaleFactor> rdf:type owl:Class ;
                                                                     rdfs:subClassOf <http://ontology.asam.net/ontologies/Domain#roadTopologyAndTrafficInfrastructureProperty> ;
                                                                     rdfs:comment "DEF: RoadFrictionScaleFactor is a  RoadTopologyAndTrafficInfrastructureProperty  that describes the Friction scale factor"^^xsd:string .


###  http://ontology.asam.net/ontologies/Domain#roadTopologyAndTrafficInfrastructureProperty
<http://ontology.asam.net/ontologies/Domain#roadTopologyAndTrafficInfrastructureProperty> rdf:type owl:Class ;
                                                                                          rdfs:subClassOf <http://ontology.asam.net/ontologies/Core#PhysicalProperty> ,
                                                                                                          <http://ontology.asam.net/ontologies/Domain#RoadTopologyAndTrafficInfrastructure> .


###  http://ontology.asam.net/ontologies/Domain#snowfallIntensity
<http://ontology.asam.net/ontologies/Domain#snowfallIntensity> rdf:type owl:Class ;
                                                               rdfs:subClassOf <http://ontology.asam.net/ontologies/Domain#environmentalConditionProperty> ;
                                                               rdfs:comment "DEF: An environmentalConditionProperty that quantifies the amount of snow that falls within an area. mm/hr is used as unit of measurement.  It gives the amount or volume of water per fixed amount of time (hour)."^^xsd:string .


###  http://ontology.asam.net/ontologies/Domain#snowyRoadCondition
<http://ontology.asam.net/ontologies/Domain#snowyRoadCondition> rdf:type owl:Class ;
                                                                rdfs:subClassOf <http://ontology.asam.net/ontologies/Domain#inducedRoadSurfaceCondition> ;
                                                                rdfs:comment "DEF: An InducedRoadSurfaceCondition where snow covers the surface of the road. Snow on the surface lowers the friction coefficent and can obscure lane markings."^^xsd:string .


###  http://ontology.asam.net/ontologies/Domain#speedLimitForLane
<http://ontology.asam.net/ontologies/Domain#speedLimitForLane> rdf:type owl:Class ;
                                                               rdfs:subClassOf <http://ontology.asam.net/ontologies/Domain#roadTopologyAndTrafficInfrastructureProperty> ;
                                                               rdfs:comment "A traffic infrastructure property that represents the maximum speed allowed on a lane. Lane speed limits override road speed limits."^^xsd:string .


###  http://ontology.asam.net/ontologies/Domain#spiral
<http://ontology.asam.net/ontologies/Domain#spiral> rdf:type owl:Class ;
                                                    rdfs:subClassOf <http://ontology.asam.net/ontologies/Domain#curve> ;
                                                    rdfs:comment "DEF: A Curve with a changing curvature that is described as a clothoid. Spirals may be used to describe the transitions between geometric shapes and help avoiding leaps and gaps in the curvature."^^xsd:string .


###  http://ontology.asam.net/ontologies/Domain#standingWaterCondition
<http://ontology.asam.net/ontologies/Domain#standingWaterCondition> rdf:type owl:Class ;
                                                                    rdfs:subClassOf <http://ontology.asam.net/ontologies/Domain#inducedRoadSurfaceCondition> ;
                                                                    rdfs:comment "DEF: An InducedRoadSurfaceCondition where the road is covered with non-flowing (standing) water. Standing water often occurs in road sinks."^^xsd:string .


###  http://ontology.asam.net/ontologies/Domain#straightLine
<http://ontology.asam.net/ontologies/Domain#straightLine> rdf:type owl:Class ;
                                                          rdfs:subClassOf <http://ontology.asam.net/ontologies/Domain#horizontalGeometry> ;
                                                          rdfs:comment "DEF: A HorizontalGeometry that runs as a straight line in the associated coordinate system."^^xsd:string .


###  http://ontology.asam.net/ontologies/Domain#sunAzimuth
<http://ontology.asam.net/ontologies/Domain#sunAzimuth> rdf:type owl:Class ;
                                                        rdfs:subClassOf <http://ontology.asam.net/ontologies/Domain#sunProperty> ;
                                                        rdfs:comment "DEF: A sunProperty that is the azimuth angle of the sun's position. It is defined as the angle between a line due south and the shadow cast by a vertical rod on Earth."^^xsd:string .


###  http://ontology.asam.net/ontologies/Domain#sunElevation
<http://ontology.asam.net/ontologies/Domain#sunElevation> rdf:type owl:Class ;
                                                          rdfs:subClassOf <http://ontology.asam.net/ontologies/Domain#sunProperty> ;
                                                          rdfs:comment "DEF: A sunProperty that is the solar zenith angle, which is defined as the angle between the sun's rays and the vertical direction. It is complementary to the solar altitude angle, which is the angle between the sun’s rays and a horizontal plane."^^xsd:string .


###  http://ontology.asam.net/ontologies/Domain#sunProperty
<http://ontology.asam.net/ontologies/Domain#sunProperty> rdf:type owl:Class ;
                                                         rdfs:subClassOf <http://ontology.asam.net/ontologies/Domain#environmentalConditionProperty> ;
                                                         rdfs:comment "DEF: An environmentalConditionProperty that defines characteristics of the sun, for example, azimuth and elevation."^^xsd:string .


###  http://ontology.asam.net/ontologies/Domain#superElevation
<http://ontology.asam.net/ontologies/Domain#superElevation> rdf:type owl:Class ;
                                                            rdfs:subClassOf <http://ontology.asam.net/ontologies/Domain#transverseGeometry> ;
                                                            rdfs:comment "DEF: A TransverseGeometry the specifies the cross slope of a road, meaning the roll angle of the road cross section around a reference line."^^xsd:string .


###  http://ontology.asam.net/ontologies/Domain#temperature
<http://ontology.asam.net/ontologies/Domain#temperature> rdf:type owl:Class ;
                                                         rdfs:subClassOf <http://ontology.asam.net/ontologies/Domain#environmentalConditionProperty> ;
                                                         rdfs:comment "DEF: An environmentalConditionProperty that describes how warm or cold it is. Temperature is given in one of the following units: Kelvin [K], Celsius[℃] or Fahrenheit [℉]."^^xsd:string .


###  http://ontology.asam.net/ontologies/Domain#trafficParticipantsAndBehavioursProperty
<http://ontology.asam.net/ontologies/Domain#trafficParticipantsAndBehavioursProperty> rdf:type owl:Class ;
                                                                                      rdfs:subClassOf <http://ontology.asam.net/ontologies/Core#PhysicalProperty> ,
                                                                                                      <http://ontology.asam.net/ontologies/Domain#TrafficParticipantAndBehavior> .


###  http://ontology.asam.net/ontologies/Domain#transverseGeometry
<http://ontology.asam.net/ontologies/Domain#transverseGeometry> rdf:type owl:Class ;
                                                                rdfs:subClassOf <http://ontology.asam.net/ontologies/Domain#drivableAreaGeometry> ;
                                                                rdfs:comment "DEF: A DrivableAreaGeometry in the cross-section plane; the transverse profile"^^xsd:string .


###  http://ontology.asam.net/ontologies/Domain#upSlope
<http://ontology.asam.net/ontologies/Domain#upSlope> rdf:type owl:Class ;
                                                     rdfs:subClassOf <http://ontology.asam.net/ontologies/Domain#verticalGeometry> ;
                                                     rdfs:comment "DEF: A VerticalGeometry that is a plane with positive gradient. It represents an ascending elevation of the road in driving direction."^^xsd:string .


###  http://ontology.asam.net/ontologies/Domain#verticalGeometry
<http://ontology.asam.net/ontologies/Domain#verticalGeometry> rdf:type owl:Class ;
                                                              rdfs:subClassOf <http://ontology.asam.net/ontologies/Domain#drivableAreaGeometry> ;
                                                              rdfs:comment "DEF: A DrivableAreaGeometry in the vertical (longitudinal) plane"^^xsd:string .


###  http://ontology.asam.net/ontologies/Domain#visibility
<http://ontology.asam.net/ontologies/Domain#visibility> rdf:type owl:Class ;
                                                        rdfs:subClassOf <http://ontology.asam.net/ontologies/Domain#environmentalConditionProperty> ;
                                                        rdfs:comment "DEF: An environmentalConditionProperty type that specifies the distance at which a thing can be clearly discerned. The distance may be specified in meters, kilometers, or miles."^^xsd:string .


###  http://ontology.asam.net/ontologies/Domain#wetRoadCondition
<http://ontology.asam.net/ontologies/Domain#wetRoadCondition> rdf:type owl:Class ;
                                                              rdfs:subClassOf <http://ontology.asam.net/ontologies/Domain#inducedRoadSurfaceCondition> ;
                                                              rdfs:comment "DEF: An InducedRoadSurfaceCondition where the road is covered with a thin layer of water. This can lower the friction coefficent."^^xsd:string .


###  http://ontology.asam.net/ontologies/Domain#windDirection
<http://ontology.asam.net/ontologies/Domain#windDirection> rdf:type owl:Class ;
                                                           rdfs:subClassOf <http://ontology.asam.net/ontologies/Domain#environmentalConditionProperty> ;
                                                           rdfs:comment "DEF: An environmentalConditionProperty that characterizes the direction from which the wind is coming. The direction may be specified as cardinal direction or in degrees. Example: Wind coming from the North is defined as a wind direction of 0° or 360°."^^xsd:string .


###  http://ontology.asam.net/ontologies/Domain#windSpeed
<http://ontology.asam.net/ontologies/Domain#windSpeed> rdf:type owl:Class ;
                                                       rdfs:subClassOf <http://ontology.asam.net/ontologies/Domain#environmentalConditionProperty> ;
                                                       rdfs:comment "DEF: An environmentalConditionProperty that defines how strong the wind is blowing. Wind speed is given in m/s."^^xsd:string .


###  http://ontology.asam.net/ontologies/OpenXOntology.owl#HumanCommunicationActivity
:HumanCommunicationActivity rdf:type owl:Class ;
                            rdfs:subClassOf <http://ontology.asam.net/ontologies/Domain#CommunicationActivity> ,
                                            <http://ontology.asam.net/ontologies/Domain#HumanActivity> ;
                            rdfs:comment "DEF: A CommunicatingActivity where the subject is a vehicle." .


#################################################################
#    General axioms
#################################################################

[ rdf:type owl:AllDisjointClasses ;
  owl:members ( <http://ontology.asam.net/ontologies/Core#AngleQuantity>
                <http://ontology.asam.net/ontologies/Core#DirectionQuantity>
                <http://ontology.asam.net/ontologies/Core#LengthQuantity>
                <http://ontology.asam.net/ontologies/Core#SpeedQuantity>
              )
] .


#################################################################
#    Rules
#################################################################

<http://www.semanticweb.org/stevek/ontologies/2021/6/objectPropertiesV1#p1> rdf:type <http://www.w3.org/2003/11/swrl#Variable> .

<http://www.semanticweb.org/stevek/ontologies/2021/6/objectPropertiesV1#p2> rdf:type <http://www.w3.org/2003/11/swrl#Variable> .

<http://www.semanticweb.org/stevek/ontologies/2021/6/objectPropertiesV1#p1h> rdf:type <http://www.w3.org/2003/11/swrl#Variable> .

<http://www.semanticweb.org/stevek/ontologies/2021/6/objectPropertiesV1#r> rdf:type <http://www.w3.org/2003/11/swrl#Variable> .

<http://www.semanticweb.org/stevek/ontologies/2021/6/objectPropertiesV1#rdir1> rdf:type <http://www.w3.org/2003/11/swrl#Variable> .

<http://www.semanticweb.org/stevek/ontologies/2021/6/objectPropertiesV1#rdir2> rdf:type <http://www.w3.org/2003/11/swrl#Variable> .

<http://www.semanticweb.org/stevek/ontologies/2021/6/objectPropertiesV1#p1hvalue> rdf:type <http://www.w3.org/2003/11/swrl#Variable> .

<http://www.semanticweb.org/stevek/ontologies/2021/6/objectPropertiesV1#rdir1value> rdf:type <http://www.w3.org/2003/11/swrl#Variable> .

<http://www.semanticweb.org/stevek/ontologies/2021/6/objectPropertiesV1#dirDiff> rdf:type <http://www.w3.org/2003/11/swrl#Variable> .

<http://ontology.asam.net/ontologies/Core#q1> rdf:type <http://www.w3.org/2003/11/swrl#Variable> .

<http://ontology.asam.net/ontologies/Core#q2> rdf:type <http://www.w3.org/2003/11/swrl#Variable> .

<http://ontology.asam.net/ontologies/Core#q1val> rdf:type <http://www.w3.org/2003/11/swrl#Variable> .

<http://ontology.asam.net/ontologies/Core#q2val> rdf:type <http://www.w3.org/2003/11/swrl#Variable> .

<http://www.semanticweb.org/stevek/ontologies/2021/6/objectPropertiesV1#q1> rdf:type <http://www.w3.org/2003/11/swrl#Variable> .

<http://www.semanticweb.org/stevek/ontologies/2021/6/objectPropertiesV1#q2> rdf:type <http://www.w3.org/2003/11/swrl#Variable> .

<http://www.semanticweb.org/stevek/ontologies/2021/6/objectPropertiesV1#q1val> rdf:type <http://www.w3.org/2003/11/swrl#Variable> .

<http://www.semanticweb.org/stevek/ontologies/2021/6/objectPropertiesV1#q2val> rdf:type <http://www.w3.org/2003/11/swrl#Variable> .

<http://www.semanticweb.org/stevek/ontologies/2021/6/objectPropertiesV1#qdiff> rdf:type <http://www.w3.org/2003/11/swrl#Variable> .

<http://www.semanticweb.org/stevek/ontologies/2021/6/objectPropertiesV1#qmax> rdf:type <http://www.w3.org/2003/11/swrl#Variable> .

<http://www.semanticweb.org/stevek/ontologies/2021/6/objectPropertiesV1#qmin> rdf:type <http://www.w3.org/2003/11/swrl#Variable> .

<http://www.semanticweb.org/stevek/ontologies/2021/6/objectPropertiesV1#x> rdf:type <http://www.w3.org/2003/11/swrl#Variable> .

<http://www.semanticweb.org/stevek/ontologies/2021/6/objectPropertiesV1#y> rdf:type <http://www.w3.org/2003/11/swrl#Variable> .

<http://www.semanticweb.org/stevek/ontologies/2021/6/objectPropertiesV1#z> rdf:type <http://www.w3.org/2003/11/swrl#Variable> .

[ <http://swrl.stanford.edu/ontologies/3.3/swrla.owl#isRuleEnabled> "true"^^xsd:boolean ;
   rdfs:comment ""^^xsd:string ;
   rdfs:label "new behind"^^xsd:string ;
   rdf:type <http://www.w3.org/2003/11/swrl#Imp> ;
   <http://www.w3.org/2003/11/swrl#body> [ rdf:type <http://www.w3.org/2003/11/swrl#AtomList> ;
                                           rdf:first [ rdf:type <http://www.w3.org/2003/11/swrl#ClassAtom> ;
                                                       <http://www.w3.org/2003/11/swrl#classPredicate> <http://ontology.asam.net/ontologies/Core#PhysicalObjectState> ;
                                                       <http://www.w3.org/2003/11/swrl#argument1> <http://www.semanticweb.org/stevek/ontologies/2021/6/objectPropertiesV1#p1>
                                                     ] ;
                                           rdf:rest [ rdf:type <http://www.w3.org/2003/11/swrl#AtomList> ;
                                                      rdf:first [ rdf:type <http://www.w3.org/2003/11/swrl#ClassAtom> ;
                                                                  <http://www.w3.org/2003/11/swrl#classPredicate> <http://ontology.asam.net/ontologies/Core#PhysicalObjectState> ;
                                                                  <http://www.w3.org/2003/11/swrl#argument1> <http://www.semanticweb.org/stevek/ontologies/2021/6/objectPropertiesV1#p2>
                                                                ] ;
                                                      rdf:rest [ rdf:type <http://www.w3.org/2003/11/swrl#AtomList> ;
                                                                 rdf:first [ rdf:type <http://www.w3.org/2003/11/swrl#ClassAtom> ;
                                                                             <http://www.w3.org/2003/11/swrl#classPredicate> <http://ontology.asam.net/ontologies/Core#DirectionQuantity> ;
                                                                             <http://www.w3.org/2003/11/swrl#argument1> <http://www.semanticweb.org/stevek/ontologies/2021/6/objectPropertiesV1#p1h>
                                                                           ] ;
                                                                 rdf:rest [ rdf:type <http://www.w3.org/2003/11/swrl#AtomList> ;
                                                                            rdf:first [ rdf:type <http://www.w3.org/2003/11/swrl#IndividualPropertyAtom> ;
                                                                                        <http://www.w3.org/2003/11/swrl#propertyPredicate> <http://ontology.asam.net/ontologies/Core#hasHeading> ;
                                                                                        <http://www.w3.org/2003/11/swrl#argument1> <http://www.semanticweb.org/stevek/ontologies/2021/6/objectPropertiesV1#p1> ;
                                                                                        <http://www.w3.org/2003/11/swrl#argument2> <http://www.semanticweb.org/stevek/ontologies/2021/6/objectPropertiesV1#p1h>
                                                                                      ] ;
                                                                            rdf:rest [ rdf:type <http://www.w3.org/2003/11/swrl#AtomList> ;
                                                                                       rdf:first [ rdf:type <http://www.w3.org/2003/11/swrl#ClassAtom> ;
                                                                                                   <http://www.w3.org/2003/11/swrl#classPredicate> <http://ontology.asam.net/ontologies/Core#SpatialRelation> ;
                                                                                                   <http://www.w3.org/2003/11/swrl#argument1> <http://www.semanticweb.org/stevek/ontologies/2021/6/objectPropertiesV1#r>
                                                                                                 ] ;
                                                                                       rdf:rest [ rdf:type <http://www.w3.org/2003/11/swrl#AtomList> ;
                                                                                                  rdf:first [ rdf:type <http://www.w3.org/2003/11/swrl#IndividualPropertyAtom> ;
                                                                                                              <http://www.w3.org/2003/11/swrl#propertyPredicate> <http://ontology.asam.net/ontologies/Core#hasSpatialSubject> ;
                                                                                                              <http://www.w3.org/2003/11/swrl#argument1> <http://www.semanticweb.org/stevek/ontologies/2021/6/objectPropertiesV1#r> ;
                                                                                                              <http://www.w3.org/2003/11/swrl#argument2> <http://www.semanticweb.org/stevek/ontologies/2021/6/objectPropertiesV1#p1>
                                                                                                            ] ;
                                                                                                  rdf:rest [ rdf:type <http://www.w3.org/2003/11/swrl#AtomList> ;
                                                                                                             rdf:first [ rdf:type <http://www.w3.org/2003/11/swrl#IndividualPropertyAtom> ;
                                                                                                                         <http://www.w3.org/2003/11/swrl#propertyPredicate> <http://ontology.asam.net/ontologies/Core#hasSpatialObject> ;
                                                                                                                         <http://www.w3.org/2003/11/swrl#argument1> <http://www.semanticweb.org/stevek/ontologies/2021/6/objectPropertiesV1#r> ;
                                                                                                                         <http://www.w3.org/2003/11/swrl#argument2> <http://www.semanticweb.org/stevek/ontologies/2021/6/objectPropertiesV1#p2>
                                                                                                                       ] ;
                                                                                                             rdf:rest [ rdf:type <http://www.w3.org/2003/11/swrl#AtomList> ;
                                                                                                                        rdf:first [ rdf:type <http://www.w3.org/2003/11/swrl#ClassAtom> ;
                                                                                                                                    <http://www.w3.org/2003/11/swrl#classPredicate> <http://ontology.asam.net/ontologies/Core#DirectionQuantity> ;
                                                                                                                                    <http://www.w3.org/2003/11/swrl#argument1> <http://www.semanticweb.org/stevek/ontologies/2021/6/objectPropertiesV1#rdir1>
                                                                                                                                  ] ;
                                                                                                                        rdf:rest [ rdf:type <http://www.w3.org/2003/11/swrl#AtomList> ;
                                                                                                                                   rdf:first [ rdf:type <http://www.w3.org/2003/11/swrl#ClassAtom> ;
                                                                                                                                               <http://www.w3.org/2003/11/swrl#classPredicate> <http://ontology.asam.net/ontologies/Core#DirectionQuantity> ;
                                                                                                                                               <http://www.w3.org/2003/11/swrl#argument1> <http://www.semanticweb.org/stevek/ontologies/2021/6/objectPropertiesV1#rdir2>
                                                                                                                                             ] ;
                                                                                                                                   rdf:rest [ rdf:type <http://www.w3.org/2003/11/swrl#AtomList> ;
                                                                                                                                              rdf:first [ rdf:type <http://www.w3.org/2003/11/swrl#IndividualPropertyAtom> ;
                                                                                                                                                          <http://www.w3.org/2003/11/swrl#propertyPredicate> <http://ontology.asam.net/ontologies/Core#hasRelationDirection> ;
                                                                                                                                                          <http://www.w3.org/2003/11/swrl#argument1> <http://www.semanticweb.org/stevek/ontologies/2021/6/objectPropertiesV1#r> ;
                                                                                                                                                          <http://www.w3.org/2003/11/swrl#argument2> <http://www.semanticweb.org/stevek/ontologies/2021/6/objectPropertiesV1#rdir1>
                                                                                                                                                        ] ;
                                                                                                                                              rdf:rest [ rdf:type <http://www.w3.org/2003/11/swrl#AtomList> ;
                                                                                                                                                         rdf:first [ rdf:type <http://www.w3.org/2003/11/swrl#DatavaluedPropertyAtom> ;
                                                                                                                                                                     <http://www.w3.org/2003/11/swrl#propertyPredicate> <http://ontology.asam.net/ontologies/Core#hasValue> ;
                                                                                                                                                                     <http://www.w3.org/2003/11/swrl#argument1> <http://www.semanticweb.org/stevek/ontologies/2021/6/objectPropertiesV1#p1h> ;
                                                                                                                                                                     <http://www.w3.org/2003/11/swrl#argument2> <http://www.semanticweb.org/stevek/ontologies/2021/6/objectPropertiesV1#p1hvalue>
                                                                                                                                                                   ] ;
                                                                                                                                                         rdf:rest [ rdf:type <http://www.w3.org/2003/11/swrl#AtomList> ;
                                                                                                                                                                    rdf:first [ rdf:type <http://www.w3.org/2003/11/swrl#DatavaluedPropertyAtom> ;
                                                                                                                                                                                <http://www.w3.org/2003/11/swrl#propertyPredicate> <http://ontology.asam.net/ontologies/Core#hasValue> ;
                                                                                                                                                                                <http://www.w3.org/2003/11/swrl#argument1> <http://www.semanticweb.org/stevek/ontologies/2021/6/objectPropertiesV1#rdir1> ;
                                                                                                                                                                                <http://www.w3.org/2003/11/swrl#argument2> <http://www.semanticweb.org/stevek/ontologies/2021/6/objectPropertiesV1#rdir1value>
                                                                                                                                                                              ] ;
                                                                                                                                                                    rdf:rest [ rdf:type <http://www.w3.org/2003/11/swrl#AtomList> ;
                                                                                                                                                                               rdf:first [ rdf:type <http://www.w3.org/2003/11/swrl#BuiltinAtom> ;
                                                                                                                                                                                           <http://www.w3.org/2003/11/swrl#builtin> <http://www.w3.org/2003/11/swrlb#subtract> ;
                                                                                                                                                                                           <http://www.w3.org/2003/11/swrl#arguments> ( <http://www.semanticweb.org/stevek/ontologies/2021/6/objectPropertiesV1#dirDiff>
                                                                                                                                                                                                                                        <http://www.semanticweb.org/stevek/ontologies/2021/6/objectPropertiesV1#rdir1value>
                                                                                                                                                                                                                                        <http://www.semanticweb.org/stevek/ontologies/2021/6/objectPropertiesV1#p1hvalue>
                                                                                                                                                                                                                                      )
                                                                                                                                                                                         ] ;
                                                                                                                                                                               rdf:rest [ rdf:type <http://www.w3.org/2003/11/swrl#AtomList> ;
                                                                                                                                                                                          rdf:first [ rdf:type <http://www.w3.org/2003/11/swrl#BuiltinAtom> ;
                                                                                                                                                                                                      <http://www.w3.org/2003/11/swrl#builtin> <http://www.w3.org/2003/11/swrlb#lessThan> ;
                                                                                                                                                                                                      <http://www.w3.org/2003/11/swrl#arguments> [ rdf:type rdf:List ;
                                                                                                                                                                                                                                                   rdf:first <http://www.semanticweb.org/stevek/ontologies/2021/6/objectPropertiesV1#dirDiff> ;
                                                                                                                                                                                                                                                   rdf:rest [ rdf:type rdf:List ;
                                                                                                                                                                                                                                                              rdf:first 195 ;
                                                                                                                                                                                                                                                              rdf:rest rdf:nil
                                                                                                                                                                                                                                                            ]
                                                                                                                                                                                                                                                 ]
                                                                                                                                                                                                    ] ;
                                                                                                                                                                                          rdf:rest [ rdf:type <http://www.w3.org/2003/11/swrl#AtomList> ;
                                                                                                                                                                                                     rdf:first [ rdf:type <http://www.w3.org/2003/11/swrl#BuiltinAtom> ;
                                                                                                                                                                                                                 <http://www.w3.org/2003/11/swrl#builtin> <http://www.w3.org/2003/11/swrlb#greaterThan> ;
                                                                                                                                                                                                                 <http://www.w3.org/2003/11/swrl#arguments> [ rdf:type rdf:List ;
                                                                                                                                                                                                                                                              rdf:first <http://www.semanticweb.org/stevek/ontologies/2021/6/objectPropertiesV1#dirDiff> ;
                                                                                                                                                                                                                                                              rdf:rest [ rdf:type rdf:List ;
                                                                                                                                                                                                                                                                         rdf:first 165 ;
                                                                                                                                                                                                                                                                         rdf:rest rdf:nil
                                                                                                                                                                                                                                                                       ]
                                                                                                                                                                                                                                                            ]
                                                                                                                                                                                                               ] ;
                                                                                                                                                                                                     rdf:rest rdf:nil
                                                                                                                                                                                                   ]
                                                                                                                                                                                        ]
                                                                                                                                                                             ]
                                                                                                                                                                  ]
                                                                                                                                                       ]
                                                                                                                                            ]
                                                                                                                                 ]
                                                                                                                      ]
                                                                                                           ]
                                                                                                ]
                                                                                     ]
                                                                          ]
                                                               ]
                                                    ]
                                         ] ;
   <http://www.w3.org/2003/11/swrl#head> [ rdf:type <http://www.w3.org/2003/11/swrl#AtomList> ;
                                           rdf:first [ rdf:type <http://www.w3.org/2003/11/swrl#IndividualPropertyAtom> ;
                                                       <http://www.w3.org/2003/11/swrl#propertyPredicate> <http://ontology.asam.net/ontologies/Core#behind> ;
                                                       <http://www.w3.org/2003/11/swrl#argument1> <http://www.semanticweb.org/stevek/ontologies/2021/6/objectPropertiesV1#p2> ;
                                                       <http://www.w3.org/2003/11/swrl#argument2> <http://www.semanticweb.org/stevek/ontologies/2021/6/objectPropertiesV1#p1>
                                                     ] ;
                                           rdf:rest rdf:nil
                                         ]
 ] .

[ <http://swrl.stanford.edu/ontologies/3.3/swrla.owl#isRuleEnabled> "true"^^xsd:boolean ;
   rdfs:comment ""^^xsd:string ;
   rdfs:label "new right of"^^xsd:string ;
   rdf:type <http://www.w3.org/2003/11/swrl#Imp> ;
   <http://www.w3.org/2003/11/swrl#body> [ rdf:type <http://www.w3.org/2003/11/swrl#AtomList> ;
                                           rdf:first [ rdf:type <http://www.w3.org/2003/11/swrl#ClassAtom> ;
                                                       <http://www.w3.org/2003/11/swrl#classPredicate> <http://ontology.asam.net/ontologies/Core#PhysicalObjectState> ;
                                                       <http://www.w3.org/2003/11/swrl#argument1> <http://www.semanticweb.org/stevek/ontologies/2021/6/objectPropertiesV1#p1>
                                                     ] ;
                                           rdf:rest [ rdf:type <http://www.w3.org/2003/11/swrl#AtomList> ;
                                                      rdf:first [ rdf:type <http://www.w3.org/2003/11/swrl#ClassAtom> ;
                                                                  <http://www.w3.org/2003/11/swrl#classPredicate> <http://ontology.asam.net/ontologies/Core#PhysicalObjectState> ;
                                                                  <http://www.w3.org/2003/11/swrl#argument1> <http://www.semanticweb.org/stevek/ontologies/2021/6/objectPropertiesV1#p2>
                                                                ] ;
                                                      rdf:rest [ rdf:type <http://www.w3.org/2003/11/swrl#AtomList> ;
                                                                 rdf:first [ rdf:type <http://www.w3.org/2003/11/swrl#ClassAtom> ;
                                                                             <http://www.w3.org/2003/11/swrl#classPredicate> <http://ontology.asam.net/ontologies/Core#DirectionQuantity> ;
                                                                             <http://www.w3.org/2003/11/swrl#argument1> <http://www.semanticweb.org/stevek/ontologies/2021/6/objectPropertiesV1#p1h>
                                                                           ] ;
                                                                 rdf:rest [ rdf:type <http://www.w3.org/2003/11/swrl#AtomList> ;
                                                                            rdf:first [ rdf:type <http://www.w3.org/2003/11/swrl#IndividualPropertyAtom> ;
                                                                                        <http://www.w3.org/2003/11/swrl#propertyPredicate> <http://ontology.asam.net/ontologies/Core#hasHeading> ;
                                                                                        <http://www.w3.org/2003/11/swrl#argument1> <http://www.semanticweb.org/stevek/ontologies/2021/6/objectPropertiesV1#p1> ;
                                                                                        <http://www.w3.org/2003/11/swrl#argument2> <http://www.semanticweb.org/stevek/ontologies/2021/6/objectPropertiesV1#p1h>
                                                                                      ] ;
                                                                            rdf:rest [ rdf:type <http://www.w3.org/2003/11/swrl#AtomList> ;
                                                                                       rdf:first [ rdf:type <http://www.w3.org/2003/11/swrl#ClassAtom> ;
                                                                                                   <http://www.w3.org/2003/11/swrl#classPredicate> <http://ontology.asam.net/ontologies/Core#SpatialRelation> ;
                                                                                                   <http://www.w3.org/2003/11/swrl#argument1> <http://www.semanticweb.org/stevek/ontologies/2021/6/objectPropertiesV1#r>
                                                                                                 ] ;
                                                                                       rdf:rest [ rdf:type <http://www.w3.org/2003/11/swrl#AtomList> ;
                                                                                                  rdf:first [ rdf:type <http://www.w3.org/2003/11/swrl#IndividualPropertyAtom> ;
                                                                                                              <http://www.w3.org/2003/11/swrl#propertyPredicate> <http://ontology.asam.net/ontologies/Core#hasSpatialSubject> ;
                                                                                                              <http://www.w3.org/2003/11/swrl#argument1> <http://www.semanticweb.org/stevek/ontologies/2021/6/objectPropertiesV1#r> ;
                                                                                                              <http://www.w3.org/2003/11/swrl#argument2> <http://www.semanticweb.org/stevek/ontologies/2021/6/objectPropertiesV1#p1>
                                                                                                            ] ;
                                                                                                  rdf:rest [ rdf:type <http://www.w3.org/2003/11/swrl#AtomList> ;
                                                                                                             rdf:first [ rdf:type <http://www.w3.org/2003/11/swrl#IndividualPropertyAtom> ;
                                                                                                                         <http://www.w3.org/2003/11/swrl#propertyPredicate> <http://ontology.asam.net/ontologies/Core#hasSpatialObject> ;
                                                                                                                         <http://www.w3.org/2003/11/swrl#argument1> <http://www.semanticweb.org/stevek/ontologies/2021/6/objectPropertiesV1#r> ;
                                                                                                                         <http://www.w3.org/2003/11/swrl#argument2> <http://www.semanticweb.org/stevek/ontologies/2021/6/objectPropertiesV1#p2>
                                                                                                                       ] ;
                                                                                                             rdf:rest [ rdf:type <http://www.w3.org/2003/11/swrl#AtomList> ;
                                                                                                                        rdf:first [ rdf:type <http://www.w3.org/2003/11/swrl#ClassAtom> ;
                                                                                                                                    <http://www.w3.org/2003/11/swrl#classPredicate> <http://ontology.asam.net/ontologies/Core#DirectionQuantity> ;
                                                                                                                                    <http://www.w3.org/2003/11/swrl#argument1> <http://www.semanticweb.org/stevek/ontologies/2021/6/objectPropertiesV1#rdir1>
                                                                                                                                  ] ;
                                                                                                                        rdf:rest [ rdf:type <http://www.w3.org/2003/11/swrl#AtomList> ;
                                                                                                                                   rdf:first [ rdf:type <http://www.w3.org/2003/11/swrl#ClassAtom> ;
                                                                                                                                               <http://www.w3.org/2003/11/swrl#classPredicate> <http://ontology.asam.net/ontologies/Core#DirectionQuantity> ;
                                                                                                                                               <http://www.w3.org/2003/11/swrl#argument1> <http://www.semanticweb.org/stevek/ontologies/2021/6/objectPropertiesV1#rdir2>
                                                                                                                                             ] ;
                                                                                                                                   rdf:rest [ rdf:type <http://www.w3.org/2003/11/swrl#AtomList> ;
                                                                                                                                              rdf:first [ rdf:type <http://www.w3.org/2003/11/swrl#IndividualPropertyAtom> ;
                                                                                                                                                          <http://www.w3.org/2003/11/swrl#propertyPredicate> <http://ontology.asam.net/ontologies/Core#hasRelationDirection> ;
                                                                                                                                                          <http://www.w3.org/2003/11/swrl#argument1> <http://www.semanticweb.org/stevek/ontologies/2021/6/objectPropertiesV1#r> ;
                                                                                                                                                          <http://www.w3.org/2003/11/swrl#argument2> <http://www.semanticweb.org/stevek/ontologies/2021/6/objectPropertiesV1#rdir1>
                                                                                                                                                        ] ;
                                                                                                                                              rdf:rest [ rdf:type <http://www.w3.org/2003/11/swrl#AtomList> ;
                                                                                                                                                         rdf:first [ rdf:type <http://www.w3.org/2003/11/swrl#DatavaluedPropertyAtom> ;
                                                                                                                                                                     <http://www.w3.org/2003/11/swrl#propertyPredicate> <http://ontology.asam.net/ontologies/Core#hasValue> ;
                                                                                                                                                                     <http://www.w3.org/2003/11/swrl#argument1> <http://www.semanticweb.org/stevek/ontologies/2021/6/objectPropertiesV1#p1h> ;
                                                                                                                                                                     <http://www.w3.org/2003/11/swrl#argument2> <http://www.semanticweb.org/stevek/ontologies/2021/6/objectPropertiesV1#p1hvalue>
                                                                                                                                                                   ] ;
                                                                                                                                                         rdf:rest [ rdf:type <http://www.w3.org/2003/11/swrl#AtomList> ;
                                                                                                                                                                    rdf:first [ rdf:type <http://www.w3.org/2003/11/swrl#DatavaluedPropertyAtom> ;
                                                                                                                                                                                <http://www.w3.org/2003/11/swrl#propertyPredicate> <http://ontology.asam.net/ontologies/Core#hasValue> ;
                                                                                                                                                                                <http://www.w3.org/2003/11/swrl#argument1> <http://www.semanticweb.org/stevek/ontologies/2021/6/objectPropertiesV1#rdir1> ;
                                                                                                                                                                                <http://www.w3.org/2003/11/swrl#argument2> <http://www.semanticweb.org/stevek/ontologies/2021/6/objectPropertiesV1#rdir1value>
                                                                                                                                                                              ] ;
                                                                                                                                                                    rdf:rest [ rdf:type <http://www.w3.org/2003/11/swrl#AtomList> ;
                                                                                                                                                                               rdf:first [ rdf:type <http://www.w3.org/2003/11/swrl#BuiltinAtom> ;
                                                                                                                                                                                           <http://www.w3.org/2003/11/swrl#builtin> <http://www.w3.org/2003/11/swrlb#subtract> ;
                                                                                                                                                                                           <http://www.w3.org/2003/11/swrl#arguments> ( <http://www.semanticweb.org/stevek/ontologies/2021/6/objectPropertiesV1#dirDiff>
                                                                                                                                                                                                                                        <http://www.semanticweb.org/stevek/ontologies/2021/6/objectPropertiesV1#rdir1value>
                                                                                                                                                                                                                                        <http://www.semanticweb.org/stevek/ontologies/2021/6/objectPropertiesV1#p1hvalue>
                                                                                                                                                                                                                                      )
                                                                                                                                                                                         ] ;
                                                                                                                                                                               rdf:rest [ rdf:type <http://www.w3.org/2003/11/swrl#AtomList> ;
                                                                                                                                                                                          rdf:first [ rdf:type <http://www.w3.org/2003/11/swrl#BuiltinAtom> ;
                                                                                                                                                                                                      <http://www.w3.org/2003/11/swrl#builtin> <http://www.w3.org/2003/11/swrlb#lessThan> ;
                                                                                                                                                                                                      <http://www.w3.org/2003/11/swrl#arguments> [ rdf:type rdf:List ;
                                                                                                                                                                                                                                                   rdf:first <http://www.semanticweb.org/stevek/ontologies/2021/6/objectPropertiesV1#dirDiff> ;
                                                                                                                                                                                                                                                   rdf:rest [ rdf:type rdf:List ;
                                                                                                                                                                                                                                                              rdf:first 105 ;
                                                                                                                                                                                                                                                              rdf:rest rdf:nil
                                                                                                                                                                                                                                                            ]
                                                                                                                                                                                                                                                 ]
                                                                                                                                                                                                    ] ;
                                                                                                                                                                                          rdf:rest [ rdf:type <http://www.w3.org/2003/11/swrl#AtomList> ;
                                                                                                                                                                                                     rdf:first [ rdf:type <http://www.w3.org/2003/11/swrl#BuiltinAtom> ;
                                                                                                                                                                                                                 <http://www.w3.org/2003/11/swrl#builtin> <http://www.w3.org/2003/11/swrlb#greaterThan> ;
                                                                                                                                                                                                                 <http://www.w3.org/2003/11/swrl#arguments> [ rdf:type rdf:List ;
                                                                                                                                                                                                                                                              rdf:first <http://www.semanticweb.org/stevek/ontologies/2021/6/objectPropertiesV1#dirDiff> ;
                                                                                                                                                                                                                                                              rdf:rest [ rdf:type rdf:List ;
                                                                                                                                                                                                                                                                         rdf:first 75 ;
                                                                                                                                                                                                                                                                         rdf:rest rdf:nil
                                                                                                                                                                                                                                                                       ]
                                                                                                                                                                                                                                                            ]
                                                                                                                                                                                                               ] ;
                                                                                                                                                                                                     rdf:rest rdf:nil
                                                                                                                                                                                                   ]
                                                                                                                                                                                        ]
                                                                                                                                                                             ]
                                                                                                                                                                  ]
                                                                                                                                                       ]
                                                                                                                                            ]
                                                                                                                                 ]
                                                                                                                      ]
                                                                                                           ]
                                                                                                ]
                                                                                     ]
                                                                          ]
                                                               ]
                                                    ]
                                         ] ;
   <http://www.w3.org/2003/11/swrl#head> [ rdf:type <http://www.w3.org/2003/11/swrl#AtomList> ;
                                           rdf:first [ rdf:type <http://www.w3.org/2003/11/swrl#IndividualPropertyAtom> ;
                                                       <http://www.w3.org/2003/11/swrl#propertyPredicate> <http://ontology.asam.net/ontologies/Core#rightOf> ;
                                                       <http://www.w3.org/2003/11/swrl#argument1> <http://www.semanticweb.org/stevek/ontologies/2021/6/objectPropertiesV1#p2> ;
                                                       <http://www.w3.org/2003/11/swrl#argument2> <http://www.semanticweb.org/stevek/ontologies/2021/6/objectPropertiesV1#p1>
                                                     ] ;
                                           rdf:rest rdf:nil
                                         ]
 ] .

[ <http://swrl.stanford.edu/ontologies/3.3/swrla.owl#isRuleEnabled> "true"^^xsd:boolean ;
   rdfs:comment ""^^xsd:string ;
   rdfs:label "quantity greater than"^^xsd:string ;
   rdf:type <http://www.w3.org/2003/11/swrl#Imp> ;
   <http://www.w3.org/2003/11/swrl#body> [ rdf:type <http://www.w3.org/2003/11/swrl#AtomList> ;
                                           rdf:first [ rdf:type <http://www.w3.org/2003/11/swrl#ClassAtom> ;
                                                       <http://www.w3.org/2003/11/swrl#classPredicate> <http://ontology.asam.net/ontologies/Core#PhysicalQuantity> ;
                                                       <http://www.w3.org/2003/11/swrl#argument1> <http://ontology.asam.net/ontologies/Core#q1>
                                                     ] ;
                                           rdf:rest [ rdf:type <http://www.w3.org/2003/11/swrl#AtomList> ;
                                                      rdf:first [ rdf:type <http://www.w3.org/2003/11/swrl#ClassAtom> ;
                                                                  <http://www.w3.org/2003/11/swrl#classPredicate> <http://ontology.asam.net/ontologies/Core#PhysicalQuantity> ;
                                                                  <http://www.w3.org/2003/11/swrl#argument1> <http://ontology.asam.net/ontologies/Core#q2>
                                                                ] ;
                                                      rdf:rest [ rdf:type <http://www.w3.org/2003/11/swrl#AtomList> ;
                                                                 rdf:first [ rdf:type <http://www.w3.org/2003/11/swrl#DatavaluedPropertyAtom> ;
                                                                             <http://www.w3.org/2003/11/swrl#propertyPredicate> <http://ontology.asam.net/ontologies/Core#hasValue> ;
                                                                             <http://www.w3.org/2003/11/swrl#argument1> <http://ontology.asam.net/ontologies/Core#q1> ;
                                                                             <http://www.w3.org/2003/11/swrl#argument2> <http://ontology.asam.net/ontologies/Core#q1val>
                                                                           ] ;
                                                                 rdf:rest [ rdf:type <http://www.w3.org/2003/11/swrl#AtomList> ;
                                                                            rdf:first [ rdf:type <http://www.w3.org/2003/11/swrl#DatavaluedPropertyAtom> ;
                                                                                        <http://www.w3.org/2003/11/swrl#propertyPredicate> <http://ontology.asam.net/ontologies/Core#hasValue> ;
                                                                                        <http://www.w3.org/2003/11/swrl#argument1> <http://ontology.asam.net/ontologies/Core#q2> ;
                                                                                        <http://www.w3.org/2003/11/swrl#argument2> <http://ontology.asam.net/ontologies/Core#q2val>
                                                                                      ] ;
                                                                            rdf:rest [ rdf:type <http://www.w3.org/2003/11/swrl#AtomList> ;
                                                                                       rdf:first [ rdf:type <http://www.w3.org/2003/11/swrl#BuiltinAtom> ;
                                                                                                   <http://www.w3.org/2003/11/swrl#builtin> <http://www.w3.org/2003/11/swrlb#greaterThan> ;
                                                                                                   <http://www.w3.org/2003/11/swrl#arguments> ( <http://ontology.asam.net/ontologies/Core#q1val>
                                                                                                                                                <http://ontology.asam.net/ontologies/Core#q2val>
                                                                                                                                              )
                                                                                                 ] ;
                                                                                       rdf:rest rdf:nil
                                                                                     ]
                                                                          ]
                                                               ]
                                                    ]
                                         ] ;
   <http://www.w3.org/2003/11/swrl#head> [ rdf:type <http://www.w3.org/2003/11/swrl#AtomList> ;
                                           rdf:first [ rdf:type <http://www.w3.org/2003/11/swrl#IndividualPropertyAtom> ;
                                                       <http://www.w3.org/2003/11/swrl#propertyPredicate> <http://ontology.asam.net/ontologies/Core#quantityGreaterThan> ;
                                                       <http://www.w3.org/2003/11/swrl#argument1> <http://ontology.asam.net/ontologies/Core#q2> ;
                                                       <http://www.w3.org/2003/11/swrl#argument2> <http://ontology.asam.net/ontologies/Core#q1>
                                                     ] ;
                                           rdf:rest rdf:nil
                                         ]
 ] .

[ <http://swrl.stanford.edu/ontologies/3.3/swrla.owl#isRuleEnabled> "true"^^xsd:boolean ;
   rdfs:comment ""^^xsd:string ;
   rdfs:label "greater than or equal to"^^xsd:string ;
   rdf:type <http://www.w3.org/2003/11/swrl#Imp> ;
   <http://www.w3.org/2003/11/swrl#body> [ rdf:type <http://www.w3.org/2003/11/swrl#AtomList> ;
                                           rdf:first [ rdf:type <http://www.w3.org/2003/11/swrl#ClassAtom> ;
                                                       <http://www.w3.org/2003/11/swrl#classPredicate> <http://ontology.asam.net/ontologies/Core#PhysicalQuantity> ;
                                                       <http://www.w3.org/2003/11/swrl#argument1> <http://ontology.asam.net/ontologies/Core#q1>
                                                     ] ;
                                           rdf:rest [ rdf:type <http://www.w3.org/2003/11/swrl#AtomList> ;
                                                      rdf:first [ rdf:type <http://www.w3.org/2003/11/swrl#ClassAtom> ;
                                                                  <http://www.w3.org/2003/11/swrl#classPredicate> <http://ontology.asam.net/ontologies/Core#PhysicalQuantity> ;
                                                                  <http://www.w3.org/2003/11/swrl#argument1> <http://ontology.asam.net/ontologies/Core#q2>
                                                                ] ;
                                                      rdf:rest [ rdf:type <http://www.w3.org/2003/11/swrl#AtomList> ;
                                                                 rdf:first [ rdf:type <http://www.w3.org/2003/11/swrl#DatavaluedPropertyAtom> ;
                                                                             <http://www.w3.org/2003/11/swrl#propertyPredicate> <http://ontology.asam.net/ontologies/Core#hasValue> ;
                                                                             <http://www.w3.org/2003/11/swrl#argument1> <http://ontology.asam.net/ontologies/Core#q1> ;
                                                                             <http://www.w3.org/2003/11/swrl#argument2> <http://ontology.asam.net/ontologies/Core#q1val>
                                                                           ] ;
                                                                 rdf:rest [ rdf:type <http://www.w3.org/2003/11/swrl#AtomList> ;
                                                                            rdf:first [ rdf:type <http://www.w3.org/2003/11/swrl#DatavaluedPropertyAtom> ;
                                                                                        <http://www.w3.org/2003/11/swrl#propertyPredicate> <http://ontology.asam.net/ontologies/Core#hasValue> ;
                                                                                        <http://www.w3.org/2003/11/swrl#argument1> <http://ontology.asam.net/ontologies/Core#q2> ;
                                                                                        <http://www.w3.org/2003/11/swrl#argument2> <http://ontology.asam.net/ontologies/Core#q2val>
                                                                                      ] ;
                                                                            rdf:rest [ rdf:type <http://www.w3.org/2003/11/swrl#AtomList> ;
                                                                                       rdf:first [ rdf:type <http://www.w3.org/2003/11/swrl#BuiltinAtom> ;
                                                                                                   <http://www.w3.org/2003/11/swrl#builtin> <http://www.w3.org/2003/11/swrlb#greaterThanOrEqual> ;
                                                                                                   <http://www.w3.org/2003/11/swrl#arguments> ( <http://ontology.asam.net/ontologies/Core#q1val>
                                                                                                                                                <http://ontology.asam.net/ontologies/Core#q2val>
                                                                                                                                              )
                                                                                                 ] ;
                                                                                       rdf:rest rdf:nil
                                                                                     ]
                                                                          ]
                                                               ]
                                                    ]
                                         ] ;
   <http://www.w3.org/2003/11/swrl#head> [ rdf:type <http://www.w3.org/2003/11/swrl#AtomList> ;
                                           rdf:first [ rdf:type <http://www.w3.org/2003/11/swrl#IndividualPropertyAtom> ;
                                                       <http://www.w3.org/2003/11/swrl#propertyPredicate> <http://ontology.asam.net/ontologies/Core#quantityGreaterThanOrEqualTo> ;
                                                       <http://www.w3.org/2003/11/swrl#argument1> <http://ontology.asam.net/ontologies/Core#q2> ;
                                                       <http://www.w3.org/2003/11/swrl#argument2> <http://ontology.asam.net/ontologies/Core#q1>
                                                     ] ;
                                           rdf:rest rdf:nil
                                         ]
 ] .

[ <http://swrl.stanford.edu/ontologies/3.3/swrla.owl#isRuleEnabled> "true"^^xsd:boolean ;
   rdfs:comment ""^^xsd:string ;
   rdfs:label "quantity less than"^^xsd:string ;
   rdf:type <http://www.w3.org/2003/11/swrl#Imp> ;
   <http://www.w3.org/2003/11/swrl#body> [ rdf:type <http://www.w3.org/2003/11/swrl#AtomList> ;
                                           rdf:first [ rdf:type <http://www.w3.org/2003/11/swrl#ClassAtom> ;
                                                       <http://www.w3.org/2003/11/swrl#classPredicate> <http://ontology.asam.net/ontologies/Core#PhysicalQuantity> ;
                                                       <http://www.w3.org/2003/11/swrl#argument1> <http://ontology.asam.net/ontologies/Core#q1>
                                                     ] ;
                                           rdf:rest [ rdf:type <http://www.w3.org/2003/11/swrl#AtomList> ;
                                                      rdf:first [ rdf:type <http://www.w3.org/2003/11/swrl#ClassAtom> ;
                                                                  <http://www.w3.org/2003/11/swrl#classPredicate> <http://ontology.asam.net/ontologies/Core#PhysicalQuantity> ;
                                                                  <http://www.w3.org/2003/11/swrl#argument1> <http://ontology.asam.net/ontologies/Core#q2>
                                                                ] ;
                                                      rdf:rest [ rdf:type <http://www.w3.org/2003/11/swrl#AtomList> ;
                                                                 rdf:first [ rdf:type <http://www.w3.org/2003/11/swrl#DatavaluedPropertyAtom> ;
                                                                             <http://www.w3.org/2003/11/swrl#propertyPredicate> <http://ontology.asam.net/ontologies/Core#hasValue> ;
                                                                             <http://www.w3.org/2003/11/swrl#argument1> <http://ontology.asam.net/ontologies/Core#q1> ;
                                                                             <http://www.w3.org/2003/11/swrl#argument2> <http://ontology.asam.net/ontologies/Core#q1val>
                                                                           ] ;
                                                                 rdf:rest [ rdf:type <http://www.w3.org/2003/11/swrl#AtomList> ;
                                                                            rdf:first [ rdf:type <http://www.w3.org/2003/11/swrl#DatavaluedPropertyAtom> ;
                                                                                        <http://www.w3.org/2003/11/swrl#propertyPredicate> <http://ontology.asam.net/ontologies/Core#hasValue> ;
                                                                                        <http://www.w3.org/2003/11/swrl#argument1> <http://ontology.asam.net/ontologies/Core#q2> ;
                                                                                        <http://www.w3.org/2003/11/swrl#argument2> <http://ontology.asam.net/ontologies/Core#q2val>
                                                                                      ] ;
                                                                            rdf:rest [ rdf:type <http://www.w3.org/2003/11/swrl#AtomList> ;
                                                                                       rdf:first [ rdf:type <http://www.w3.org/2003/11/swrl#BuiltinAtom> ;
                                                                                                   <http://www.w3.org/2003/11/swrl#builtin> <http://www.w3.org/2003/11/swrlb#lessThan> ;
                                                                                                   <http://www.w3.org/2003/11/swrl#arguments> ( <http://ontology.asam.net/ontologies/Core#q1val>
                                                                                                                                                <http://ontology.asam.net/ontologies/Core#q2val>
                                                                                                                                              )
                                                                                                 ] ;
                                                                                       rdf:rest rdf:nil
                                                                                     ]
                                                                          ]
                                                               ]
                                                    ]
                                         ] ;
   <http://www.w3.org/2003/11/swrl#head> [ rdf:type <http://www.w3.org/2003/11/swrl#AtomList> ;
                                           rdf:first [ rdf:type <http://www.w3.org/2003/11/swrl#IndividualPropertyAtom> ;
                                                       <http://www.w3.org/2003/11/swrl#propertyPredicate> <http://ontology.asam.net/ontologies/Core#quantityLessThan> ;
                                                       <http://www.w3.org/2003/11/swrl#argument1> <http://ontology.asam.net/ontologies/Core#q2> ;
                                                       <http://www.w3.org/2003/11/swrl#argument2> <http://ontology.asam.net/ontologies/Core#q1>
                                                     ] ;
                                           rdf:rest rdf:nil
                                         ]
 ] .

[ <http://swrl.stanford.edu/ontologies/3.3/swrla.owl#isRuleEnabled> "true"^^xsd:boolean ;
   rdfs:comment ""^^xsd:string ;
   rdfs:label "quantity less than or equal to"^^xsd:string ;
   rdf:type <http://www.w3.org/2003/11/swrl#Imp> ;
   <http://www.w3.org/2003/11/swrl#body> [ rdf:type <http://www.w3.org/2003/11/swrl#AtomList> ;
                                           rdf:first [ rdf:type <http://www.w3.org/2003/11/swrl#ClassAtom> ;
                                                       <http://www.w3.org/2003/11/swrl#classPredicate> <http://ontology.asam.net/ontologies/Core#PhysicalQuantity> ;
                                                       <http://www.w3.org/2003/11/swrl#argument1> <http://ontology.asam.net/ontologies/Core#q1>
                                                     ] ;
                                           rdf:rest [ rdf:type <http://www.w3.org/2003/11/swrl#AtomList> ;
                                                      rdf:first [ rdf:type <http://www.w3.org/2003/11/swrl#ClassAtom> ;
                                                                  <http://www.w3.org/2003/11/swrl#classPredicate> <http://ontology.asam.net/ontologies/Core#PhysicalQuantity> ;
                                                                  <http://www.w3.org/2003/11/swrl#argument1> <http://ontology.asam.net/ontologies/Core#q2>
                                                                ] ;
                                                      rdf:rest [ rdf:type <http://www.w3.org/2003/11/swrl#AtomList> ;
                                                                 rdf:first [ rdf:type <http://www.w3.org/2003/11/swrl#DatavaluedPropertyAtom> ;
                                                                             <http://www.w3.org/2003/11/swrl#propertyPredicate> <http://ontology.asam.net/ontologies/Core#hasValue> ;
                                                                             <http://www.w3.org/2003/11/swrl#argument1> <http://ontology.asam.net/ontologies/Core#q1> ;
                                                                             <http://www.w3.org/2003/11/swrl#argument2> <http://ontology.asam.net/ontologies/Core#q1val>
                                                                           ] ;
                                                                 rdf:rest [ rdf:type <http://www.w3.org/2003/11/swrl#AtomList> ;
                                                                            rdf:first [ rdf:type <http://www.w3.org/2003/11/swrl#DatavaluedPropertyAtom> ;
                                                                                        <http://www.w3.org/2003/11/swrl#propertyPredicate> <http://ontology.asam.net/ontologies/Core#hasValue> ;
                                                                                        <http://www.w3.org/2003/11/swrl#argument1> <http://ontology.asam.net/ontologies/Core#q2> ;
                                                                                        <http://www.w3.org/2003/11/swrl#argument2> <http://ontology.asam.net/ontologies/Core#q2val>
                                                                                      ] ;
                                                                            rdf:rest [ rdf:type <http://www.w3.org/2003/11/swrl#AtomList> ;
                                                                                       rdf:first [ rdf:type <http://www.w3.org/2003/11/swrl#BuiltinAtom> ;
                                                                                                   <http://www.w3.org/2003/11/swrl#builtin> <http://www.w3.org/2003/11/swrlb#lessThanOrEqual> ;
                                                                                                   <http://www.w3.org/2003/11/swrl#arguments> ( <http://ontology.asam.net/ontologies/Core#q1val>
                                                                                                                                                <http://ontology.asam.net/ontologies/Core#q2val>
                                                                                                                                              )
                                                                                                 ] ;
                                                                                       rdf:rest rdf:nil
                                                                                     ]
                                                                          ]
                                                               ]
                                                    ]
                                         ] ;
   <http://www.w3.org/2003/11/swrl#head> [ rdf:type <http://www.w3.org/2003/11/swrl#AtomList> ;
                                           rdf:first [ rdf:type <http://www.w3.org/2003/11/swrl#IndividualPropertyAtom> ;
                                                       <http://www.w3.org/2003/11/swrl#propertyPredicate> <http://ontology.asam.net/ontologies/Core#quantityLessThanOrEqualTo> ;
                                                       <http://www.w3.org/2003/11/swrl#argument1> <http://ontology.asam.net/ontologies/Core#q2> ;
                                                       <http://www.w3.org/2003/11/swrl#argument2> <http://ontology.asam.net/ontologies/Core#q1>
                                                     ] ;
                                           rdf:rest rdf:nil
                                         ]
 ] .

[ <http://swrl.stanford.edu/ontologies/3.3/swrla.owl#isRuleEnabled> "true"^^xsd:boolean ;
   rdfs:comment ""^^xsd:string ;
   rdfs:label "quantity not equal to"^^xsd:string ;
   rdf:type <http://www.w3.org/2003/11/swrl#Imp> ;
   <http://www.w3.org/2003/11/swrl#body> [ rdf:type <http://www.w3.org/2003/11/swrl#AtomList> ;
                                           rdf:first [ rdf:type <http://www.w3.org/2003/11/swrl#ClassAtom> ;
                                                       <http://www.w3.org/2003/11/swrl#classPredicate> <http://ontology.asam.net/ontologies/Core#PhysicalQuantity> ;
                                                       <http://www.w3.org/2003/11/swrl#argument1> <http://ontology.asam.net/ontologies/Core#q1>
                                                     ] ;
                                           rdf:rest [ rdf:type <http://www.w3.org/2003/11/swrl#AtomList> ;
                                                      rdf:first [ rdf:type <http://www.w3.org/2003/11/swrl#ClassAtom> ;
                                                                  <http://www.w3.org/2003/11/swrl#classPredicate> <http://ontology.asam.net/ontologies/Core#PhysicalQuantity> ;
                                                                  <http://www.w3.org/2003/11/swrl#argument1> <http://ontology.asam.net/ontologies/Core#q2>
                                                                ] ;
                                                      rdf:rest [ rdf:type <http://www.w3.org/2003/11/swrl#AtomList> ;
                                                                 rdf:first [ rdf:type <http://www.w3.org/2003/11/swrl#DatavaluedPropertyAtom> ;
                                                                             <http://www.w3.org/2003/11/swrl#propertyPredicate> <http://ontology.asam.net/ontologies/Core#hasValue> ;
                                                                             <http://www.w3.org/2003/11/swrl#argument1> <http://ontology.asam.net/ontologies/Core#q1> ;
                                                                             <http://www.w3.org/2003/11/swrl#argument2> <http://ontology.asam.net/ontologies/Core#q1val>
                                                                           ] ;
                                                                 rdf:rest [ rdf:type <http://www.w3.org/2003/11/swrl#AtomList> ;
                                                                            rdf:first [ rdf:type <http://www.w3.org/2003/11/swrl#DatavaluedPropertyAtom> ;
                                                                                        <http://www.w3.org/2003/11/swrl#propertyPredicate> <http://ontology.asam.net/ontologies/Core#hasValue> ;
                                                                                        <http://www.w3.org/2003/11/swrl#argument1> <http://ontology.asam.net/ontologies/Core#q2> ;
                                                                                        <http://www.w3.org/2003/11/swrl#argument2> <http://ontology.asam.net/ontologies/Core#q2val>
                                                                                      ] ;
                                                                            rdf:rest [ rdf:type <http://www.w3.org/2003/11/swrl#AtomList> ;
                                                                                       rdf:first [ rdf:type <http://www.w3.org/2003/11/swrl#BuiltinAtom> ;
                                                                                                   <http://www.w3.org/2003/11/swrl#builtin> <http://www.w3.org/2003/11/swrlb#notEqual> ;
                                                                                                   <http://www.w3.org/2003/11/swrl#arguments> ( <http://ontology.asam.net/ontologies/Core#q1val>
                                                                                                                                                <http://ontology.asam.net/ontologies/Core#q2val>
                                                                                                                                              )
                                                                                                 ] ;
                                                                                       rdf:rest rdf:nil
                                                                                     ]
                                                                          ]
                                                               ]
                                                    ]
                                         ] ;
   <http://www.w3.org/2003/11/swrl#head> [ rdf:type <http://www.w3.org/2003/11/swrl#AtomList> ;
                                           rdf:first [ rdf:type <http://www.w3.org/2003/11/swrl#IndividualPropertyAtom> ;
                                                       <http://www.w3.org/2003/11/swrl#propertyPredicate> <http://ontology.asam.net/ontologies/Core#quantityNotEqualTo> ;
                                                       <http://www.w3.org/2003/11/swrl#argument1> <http://ontology.asam.net/ontologies/Core#q2> ;
                                                       <http://www.w3.org/2003/11/swrl#argument2> <http://ontology.asam.net/ontologies/Core#q1>
                                                     ] ;
                                           rdf:rest rdf:nil
                                         ]
 ] .

[ <http://swrl.stanford.edu/ontologies/3.3/swrla.owl#isRuleEnabled> "true"^^xsd:boolean ;
   rdfs:comment ""^^xsd:string ;
   rdfs:label "quantity equal to"^^xsd:string ;
   rdf:type <http://www.w3.org/2003/11/swrl#Imp> ;
   <http://www.w3.org/2003/11/swrl#body> [ rdf:type <http://www.w3.org/2003/11/swrl#AtomList> ;
                                           rdf:first [ rdf:type <http://www.w3.org/2003/11/swrl#ClassAtom> ;
                                                       <http://www.w3.org/2003/11/swrl#classPredicate> <http://ontology.asam.net/ontologies/Core#PhysicalQuantity> ;
                                                       <http://www.w3.org/2003/11/swrl#argument1> <http://www.semanticweb.org/stevek/ontologies/2021/6/objectPropertiesV1#q1>
                                                     ] ;
                                           rdf:rest [ rdf:type <http://www.w3.org/2003/11/swrl#AtomList> ;
                                                      rdf:first [ rdf:type <http://www.w3.org/2003/11/swrl#ClassAtom> ;
                                                                  <http://www.w3.org/2003/11/swrl#classPredicate> <http://ontology.asam.net/ontologies/Core#PhysicalQuantity> ;
                                                                  <http://www.w3.org/2003/11/swrl#argument1> <http://www.semanticweb.org/stevek/ontologies/2021/6/objectPropertiesV1#q2>
                                                                ] ;
                                                      rdf:rest [ rdf:type <http://www.w3.org/2003/11/swrl#AtomList> ;
                                                                 rdf:first [ rdf:type <http://www.w3.org/2003/11/swrl#DatavaluedPropertyAtom> ;
                                                                             <http://www.w3.org/2003/11/swrl#propertyPredicate> <http://ontology.asam.net/ontologies/Core#hasValue> ;
                                                                             <http://www.w3.org/2003/11/swrl#argument1> <http://www.semanticweb.org/stevek/ontologies/2021/6/objectPropertiesV1#q1> ;
                                                                             <http://www.w3.org/2003/11/swrl#argument2> <http://www.semanticweb.org/stevek/ontologies/2021/6/objectPropertiesV1#q1val>
                                                                           ] ;
                                                                 rdf:rest [ rdf:type <http://www.w3.org/2003/11/swrl#AtomList> ;
                                                                            rdf:first [ rdf:type <http://www.w3.org/2003/11/swrl#DatavaluedPropertyAtom> ;
                                                                                        <http://www.w3.org/2003/11/swrl#propertyPredicate> <http://ontology.asam.net/ontologies/Core#hasValue> ;
                                                                                        <http://www.w3.org/2003/11/swrl#argument1> <http://www.semanticweb.org/stevek/ontologies/2021/6/objectPropertiesV1#q2> ;
                                                                                        <http://www.w3.org/2003/11/swrl#argument2> <http://www.semanticweb.org/stevek/ontologies/2021/6/objectPropertiesV1#q2val>
                                                                                      ] ;
                                                                            rdf:rest [ rdf:type <http://www.w3.org/2003/11/swrl#AtomList> ;
                                                                                       rdf:first [ rdf:type <http://www.w3.org/2003/11/swrl#BuiltinAtom> ;
                                                                                                   <http://www.w3.org/2003/11/swrl#builtin> <http://www.w3.org/2003/11/swrlb#add> ;
                                                                                                   <http://www.w3.org/2003/11/swrl#arguments> [ rdf:type rdf:List ;
                                                                                                                                                rdf:first <http://www.semanticweb.org/stevek/ontologies/2021/6/objectPropertiesV1#q2val> ;
                                                                                                                                                rdf:rest [ rdf:type rdf:List ;
                                                                                                                                                           rdf:first <http://www.semanticweb.org/stevek/ontologies/2021/6/objectPropertiesV1#q1val> ;
                                                                                                                                                           rdf:rest [ rdf:type rdf:List ;
                                                                                                                                                                      rdf:first 0.0 ;
                                                                                                                                                                      rdf:rest rdf:nil
                                                                                                                                                                    ]
                                                                                                                                                         ]
                                                                                                                                              ]
                                                                                                 ] ;
                                                                                       rdf:rest rdf:nil
                                                                                     ]
                                                                          ]
                                                               ]
                                                    ]
                                         ] ;
   <http://www.w3.org/2003/11/swrl#head> [ rdf:type <http://www.w3.org/2003/11/swrl#AtomList> ;
                                           rdf:first [ rdf:type <http://www.w3.org/2003/11/swrl#IndividualPropertyAtom> ;
                                                       <http://www.w3.org/2003/11/swrl#propertyPredicate> <http://ontology.asam.net/ontologies/Core#quantityEqualTo> ;
                                                       <http://www.w3.org/2003/11/swrl#argument1> <http://www.semanticweb.org/stevek/ontologies/2021/6/objectPropertiesV1#q2> ;
                                                       <http://www.w3.org/2003/11/swrl#argument2> <http://www.semanticweb.org/stevek/ontologies/2021/6/objectPropertiesV1#q1>
                                                     ] ;
                                           rdf:rest rdf:nil
                                         ]
 ] .

[ <http://swrl.stanford.edu/ontologies/3.3/swrla.owl#isRuleEnabled> "true"^^xsd:boolean ;
   rdfs:comment ""^^xsd:string ;
   rdfs:label "quantity approximately equal to"^^xsd:string ;
   rdf:type <http://www.w3.org/2003/11/swrl#Imp> ;
   <http://www.w3.org/2003/11/swrl#body> [ rdf:type <http://www.w3.org/2003/11/swrl#AtomList> ;
                                           rdf:first [ rdf:type <http://www.w3.org/2003/11/swrl#ClassAtom> ;
                                                       <http://www.w3.org/2003/11/swrl#classPredicate> <http://ontology.asam.net/ontologies/Core#PhysicalQuantity> ;
                                                       <http://www.w3.org/2003/11/swrl#argument1> <http://www.semanticweb.org/stevek/ontologies/2021/6/objectPropertiesV1#q1>
                                                     ] ;
                                           rdf:rest [ rdf:type <http://www.w3.org/2003/11/swrl#AtomList> ;
                                                      rdf:first [ rdf:type <http://www.w3.org/2003/11/swrl#ClassAtom> ;
                                                                  <http://www.w3.org/2003/11/swrl#classPredicate> <http://ontology.asam.net/ontologies/Core#PhysicalQuantity> ;
                                                                  <http://www.w3.org/2003/11/swrl#argument1> <http://www.semanticweb.org/stevek/ontologies/2021/6/objectPropertiesV1#q2>
                                                                ] ;
                                                      rdf:rest [ rdf:type <http://www.w3.org/2003/11/swrl#AtomList> ;
                                                                 rdf:first [ rdf:type <http://www.w3.org/2003/11/swrl#DatavaluedPropertyAtom> ;
                                                                             <http://www.w3.org/2003/11/swrl#propertyPredicate> <http://ontology.asam.net/ontologies/Core#hasValue> ;
                                                                             <http://www.w3.org/2003/11/swrl#argument1> <http://www.semanticweb.org/stevek/ontologies/2021/6/objectPropertiesV1#q1> ;
                                                                             <http://www.w3.org/2003/11/swrl#argument2> <http://www.semanticweb.org/stevek/ontologies/2021/6/objectPropertiesV1#q1val>
                                                                           ] ;
                                                                 rdf:rest [ rdf:type <http://www.w3.org/2003/11/swrl#AtomList> ;
                                                                            rdf:first [ rdf:type <http://www.w3.org/2003/11/swrl#DatavaluedPropertyAtom> ;
                                                                                        <http://www.w3.org/2003/11/swrl#propertyPredicate> <http://ontology.asam.net/ontologies/Core#hasValue> ;
                                                                                        <http://www.w3.org/2003/11/swrl#argument1> <http://www.semanticweb.org/stevek/ontologies/2021/6/objectPropertiesV1#q2> ;
                                                                                        <http://www.w3.org/2003/11/swrl#argument2> <http://www.semanticweb.org/stevek/ontologies/2021/6/objectPropertiesV1#q2val>
                                                                                      ] ;
                                                                            rdf:rest [ rdf:type <http://www.w3.org/2003/11/swrl#AtomList> ;
                                                                                       rdf:first [ rdf:type <http://www.w3.org/2003/11/swrl#BuiltinAtom> ;
                                                                                                   <http://www.w3.org/2003/11/swrl#builtin> <http://www.w3.org/2003/11/swrlb#subtract> ;
                                                                                                   <http://www.w3.org/2003/11/swrl#arguments> ( <http://www.semanticweb.org/stevek/ontologies/2021/6/objectPropertiesV1#qdiff>
                                                                                                                                                <http://www.semanticweb.org/stevek/ontologies/2021/6/objectPropertiesV1#q2val>
                                                                                                                                                <http://www.semanticweb.org/stevek/ontologies/2021/6/objectPropertiesV1#q1val>
                                                                                                                                              )
                                                                                                 ] ;
                                                                                       rdf:rest [ rdf:type <http://www.w3.org/2003/11/swrl#AtomList> ;
                                                                                                  rdf:first [ rdf:type <http://www.w3.org/2003/11/swrl#BuiltinAtom> ;
                                                                                                              <http://www.w3.org/2003/11/swrl#builtin> <http://www.w3.org/2003/11/swrlb#multiply> ;
                                                                                                              <http://www.w3.org/2003/11/swrl#arguments> [ rdf:type rdf:List ;
                                                                                                                                                           rdf:first <http://www.semanticweb.org/stevek/ontologies/2021/6/objectPropertiesV1#qmax> ;
                                                                                                                                                           rdf:rest [ rdf:type rdf:List ;
                                                                                                                                                                      rdf:first <http://www.semanticweb.org/stevek/ontologies/2021/6/objectPropertiesV1#q2val> ;
                                                                                                                                                                      rdf:rest [ rdf:type rdf:List ;
                                                                                                                                                                                 rdf:first 0.1 ;
                                                                                                                                                                                 rdf:rest rdf:nil
                                                                                                                                                                               ]
                                                                                                                                                                    ]
                                                                                                                                                         ]
                                                                                                            ] ;
                                                                                                  rdf:rest [ rdf:type <http://www.w3.org/2003/11/swrl#AtomList> ;
                                                                                                             rdf:first [ rdf:type <http://www.w3.org/2003/11/swrl#BuiltinAtom> ;
                                                                                                                         <http://www.w3.org/2003/11/swrl#builtin> <http://www.w3.org/2003/11/swrlb#multiply> ;
                                                                                                                         <http://www.w3.org/2003/11/swrl#arguments> [ rdf:type rdf:List ;
                                                                                                                                                                      rdf:first <http://www.semanticweb.org/stevek/ontologies/2021/6/objectPropertiesV1#qmin> ;
                                                                                                                                                                      rdf:rest [ rdf:type rdf:List ;
                                                                                                                                                                                 rdf:first <http://www.semanticweb.org/stevek/ontologies/2021/6/objectPropertiesV1#q2val> ;
                                                                                                                                                                                 rdf:rest [ rdf:type rdf:List ;
                                                                                                                                                                                            rdf:first -0.1 ;
                                                                                                                                                                                            rdf:rest rdf:nil
                                                                                                                                                                                          ]
                                                                                                                                                                               ]
                                                                                                                                                                    ]
                                                                                                                       ] ;
                                                                                                             rdf:rest [ rdf:type <http://www.w3.org/2003/11/swrl#AtomList> ;
                                                                                                                        rdf:first [ rdf:type <http://www.w3.org/2003/11/swrl#BuiltinAtom> ;
                                                                                                                                    <http://www.w3.org/2003/11/swrl#builtin> <http://www.w3.org/2003/11/swrlb#lessThan> ;
                                                                                                                                    <http://www.w3.org/2003/11/swrl#arguments> ( <http://www.semanticweb.org/stevek/ontologies/2021/6/objectPropertiesV1#qdiff>
                                                                                                                                                                                 <http://www.semanticweb.org/stevek/ontologies/2021/6/objectPropertiesV1#qmax>
                                                                                                                                                                               )
                                                                                                                                  ] ;
                                                                                                                        rdf:rest [ rdf:type <http://www.w3.org/2003/11/swrl#AtomList> ;
                                                                                                                                   rdf:first [ rdf:type <http://www.w3.org/2003/11/swrl#BuiltinAtom> ;
                                                                                                                                               <http://www.w3.org/2003/11/swrl#builtin> <http://www.w3.org/2003/11/swrlb#greaterThan> ;
                                                                                                                                               <http://www.w3.org/2003/11/swrl#arguments> ( <http://www.semanticweb.org/stevek/ontologies/2021/6/objectPropertiesV1#qdiff>
                                                                                                                                                                                            <http://www.semanticweb.org/stevek/ontologies/2021/6/objectPropertiesV1#qmin>
                                                                                                                                                                                          )
                                                                                                                                             ] ;
                                                                                                                                   rdf:rest rdf:nil
                                                                                                                                 ]
                                                                                                                      ]
                                                                                                           ]
                                                                                                ]
                                                                                     ]
                                                                          ]
                                                               ]
                                                    ]
                                         ] ;
   <http://www.w3.org/2003/11/swrl#head> [ rdf:type <http://www.w3.org/2003/11/swrl#AtomList> ;
                                           rdf:first [ rdf:type <http://www.w3.org/2003/11/swrl#IndividualPropertyAtom> ;
                                                       <http://www.w3.org/2003/11/swrl#propertyPredicate> <http://ontology.asam.net/ontologies/Core#approximatelyEqualTo> ;
                                                       <http://www.w3.org/2003/11/swrl#argument1> <http://www.semanticweb.org/stevek/ontologies/2021/6/objectPropertiesV1#q2> ;
                                                       <http://www.w3.org/2003/11/swrl#argument2> <http://www.semanticweb.org/stevek/ontologies/2021/6/objectPropertiesV1#q1>
                                                     ] ;
                                           rdf:rest rdf:nil
                                         ]
 ] .

[ <http://swrl.stanford.edu/ontologies/3.3/swrla.owl#isRuleEnabled> "true"^^xsd:boolean ;
   rdfs:comment ""^^xsd:string ;
   rdfs:label "new left of"^^xsd:string ;
   rdf:type <http://www.w3.org/2003/11/swrl#Imp> ;
   <http://www.w3.org/2003/11/swrl#body> [ rdf:type <http://www.w3.org/2003/11/swrl#AtomList> ;
                                           rdf:first [ rdf:type <http://www.w3.org/2003/11/swrl#ClassAtom> ;
                                                       <http://www.w3.org/2003/11/swrl#classPredicate> <http://ontology.asam.net/ontologies/Core#PhysicalObjectState> ;
                                                       <http://www.w3.org/2003/11/swrl#argument1> <http://www.semanticweb.org/stevek/ontologies/2021/6/objectPropertiesV1#p1>
                                                     ] ;
                                           rdf:rest [ rdf:type <http://www.w3.org/2003/11/swrl#AtomList> ;
                                                      rdf:first [ rdf:type <http://www.w3.org/2003/11/swrl#ClassAtom> ;
                                                                  <http://www.w3.org/2003/11/swrl#classPredicate> <http://ontology.asam.net/ontologies/Core#PhysicalObjectState> ;
                                                                  <http://www.w3.org/2003/11/swrl#argument1> <http://www.semanticweb.org/stevek/ontologies/2021/6/objectPropertiesV1#p2>
                                                                ] ;
                                                      rdf:rest [ rdf:type <http://www.w3.org/2003/11/swrl#AtomList> ;
                                                                 rdf:first [ rdf:type <http://www.w3.org/2003/11/swrl#ClassAtom> ;
                                                                             <http://www.w3.org/2003/11/swrl#classPredicate> <http://ontology.asam.net/ontologies/Core#DirectionQuantity> ;
                                                                             <http://www.w3.org/2003/11/swrl#argument1> <http://www.semanticweb.org/stevek/ontologies/2021/6/objectPropertiesV1#p1h>
                                                                           ] ;
                                                                 rdf:rest [ rdf:type <http://www.w3.org/2003/11/swrl#AtomList> ;
                                                                            rdf:first [ rdf:type <http://www.w3.org/2003/11/swrl#IndividualPropertyAtom> ;
                                                                                        <http://www.w3.org/2003/11/swrl#propertyPredicate> <http://ontology.asam.net/ontologies/Core#hasHeading> ;
                                                                                        <http://www.w3.org/2003/11/swrl#argument1> <http://www.semanticweb.org/stevek/ontologies/2021/6/objectPropertiesV1#p1> ;
                                                                                        <http://www.w3.org/2003/11/swrl#argument2> <http://www.semanticweb.org/stevek/ontologies/2021/6/objectPropertiesV1#p1h>
                                                                                      ] ;
                                                                            rdf:rest [ rdf:type <http://www.w3.org/2003/11/swrl#AtomList> ;
                                                                                       rdf:first [ rdf:type <http://www.w3.org/2003/11/swrl#ClassAtom> ;
                                                                                                   <http://www.w3.org/2003/11/swrl#classPredicate> <http://ontology.asam.net/ontologies/Core#SpatialRelation> ;
                                                                                                   <http://www.w3.org/2003/11/swrl#argument1> <http://www.semanticweb.org/stevek/ontologies/2021/6/objectPropertiesV1#r>
                                                                                                 ] ;
                                                                                       rdf:rest [ rdf:type <http://www.w3.org/2003/11/swrl#AtomList> ;
                                                                                                  rdf:first [ rdf:type <http://www.w3.org/2003/11/swrl#IndividualPropertyAtom> ;
                                                                                                              <http://www.w3.org/2003/11/swrl#propertyPredicate> <http://ontology.asam.net/ontologies/Core#hasSpatialSubject> ;
                                                                                                              <http://www.w3.org/2003/11/swrl#argument1> <http://www.semanticweb.org/stevek/ontologies/2021/6/objectPropertiesV1#r> ;
                                                                                                              <http://www.w3.org/2003/11/swrl#argument2> <http://www.semanticweb.org/stevek/ontologies/2021/6/objectPropertiesV1#p1>
                                                                                                            ] ;
                                                                                                  rdf:rest [ rdf:type <http://www.w3.org/2003/11/swrl#AtomList> ;
                                                                                                             rdf:first [ rdf:type <http://www.w3.org/2003/11/swrl#IndividualPropertyAtom> ;
                                                                                                                         <http://www.w3.org/2003/11/swrl#propertyPredicate> <http://ontology.asam.net/ontologies/Core#hasSpatialObject> ;
                                                                                                                         <http://www.w3.org/2003/11/swrl#argument1> <http://www.semanticweb.org/stevek/ontologies/2021/6/objectPropertiesV1#r> ;
                                                                                                                         <http://www.w3.org/2003/11/swrl#argument2> <http://www.semanticweb.org/stevek/ontologies/2021/6/objectPropertiesV1#p2>
                                                                                                                       ] ;
                                                                                                             rdf:rest [ rdf:type <http://www.w3.org/2003/11/swrl#AtomList> ;
                                                                                                                        rdf:first [ rdf:type <http://www.w3.org/2003/11/swrl#ClassAtom> ;
                                                                                                                                    <http://www.w3.org/2003/11/swrl#classPredicate> <http://ontology.asam.net/ontologies/Core#DirectionQuantity> ;
                                                                                                                                    <http://www.w3.org/2003/11/swrl#argument1> <http://www.semanticweb.org/stevek/ontologies/2021/6/objectPropertiesV1#rdir1>
                                                                                                                                  ] ;
                                                                                                                        rdf:rest [ rdf:type <http://www.w3.org/2003/11/swrl#AtomList> ;
                                                                                                                                   rdf:first [ rdf:type <http://www.w3.org/2003/11/swrl#ClassAtom> ;
                                                                                                                                               <http://www.w3.org/2003/11/swrl#classPredicate> <http://ontology.asam.net/ontologies/Core#DirectionQuantity> ;
                                                                                                                                               <http://www.w3.org/2003/11/swrl#argument1> <http://www.semanticweb.org/stevek/ontologies/2021/6/objectPropertiesV1#rdir2>
                                                                                                                                             ] ;
                                                                                                                                   rdf:rest [ rdf:type <http://www.w3.org/2003/11/swrl#AtomList> ;
                                                                                                                                              rdf:first [ rdf:type <http://www.w3.org/2003/11/swrl#IndividualPropertyAtom> ;
                                                                                                                                                          <http://www.w3.org/2003/11/swrl#propertyPredicate> <http://ontology.asam.net/ontologies/Core#hasRelationDirection> ;
                                                                                                                                                          <http://www.w3.org/2003/11/swrl#argument1> <http://www.semanticweb.org/stevek/ontologies/2021/6/objectPropertiesV1#r> ;
                                                                                                                                                          <http://www.w3.org/2003/11/swrl#argument2> <http://www.semanticweb.org/stevek/ontologies/2021/6/objectPropertiesV1#rdir1>
                                                                                                                                                        ] ;
                                                                                                                                              rdf:rest [ rdf:type <http://www.w3.org/2003/11/swrl#AtomList> ;
                                                                                                                                                         rdf:first [ rdf:type <http://www.w3.org/2003/11/swrl#DatavaluedPropertyAtom> ;
                                                                                                                                                                     <http://www.w3.org/2003/11/swrl#propertyPredicate> <http://ontology.asam.net/ontologies/Core#hasValue> ;
                                                                                                                                                                     <http://www.w3.org/2003/11/swrl#argument1> <http://www.semanticweb.org/stevek/ontologies/2021/6/objectPropertiesV1#p1h> ;
                                                                                                                                                                     <http://www.w3.org/2003/11/swrl#argument2> <http://www.semanticweb.org/stevek/ontologies/2021/6/objectPropertiesV1#p1hvalue>
                                                                                                                                                                   ] ;
                                                                                                                                                         rdf:rest [ rdf:type <http://www.w3.org/2003/11/swrl#AtomList> ;
                                                                                                                                                                    rdf:first [ rdf:type <http://www.w3.org/2003/11/swrl#DatavaluedPropertyAtom> ;
                                                                                                                                                                                <http://www.w3.org/2003/11/swrl#propertyPredicate> <http://ontology.asam.net/ontologies/Core#hasValue> ;
                                                                                                                                                                                <http://www.w3.org/2003/11/swrl#argument1> <http://www.semanticweb.org/stevek/ontologies/2021/6/objectPropertiesV1#rdir1> ;
                                                                                                                                                                                <http://www.w3.org/2003/11/swrl#argument2> <http://www.semanticweb.org/stevek/ontologies/2021/6/objectPropertiesV1#rdir1value>
                                                                                                                                                                              ] ;
                                                                                                                                                                    rdf:rest [ rdf:type <http://www.w3.org/2003/11/swrl#AtomList> ;
                                                                                                                                                                               rdf:first [ rdf:type <http://www.w3.org/2003/11/swrl#BuiltinAtom> ;
                                                                                                                                                                                           <http://www.w3.org/2003/11/swrl#builtin> <http://www.w3.org/2003/11/swrlb#subtract> ;
                                                                                                                                                                                           <http://www.w3.org/2003/11/swrl#arguments> ( <http://www.semanticweb.org/stevek/ontologies/2021/6/objectPropertiesV1#dirDiff>
                                                                                                                                                                                                                                        <http://www.semanticweb.org/stevek/ontologies/2021/6/objectPropertiesV1#rdir1value>
                                                                                                                                                                                                                                        <http://www.semanticweb.org/stevek/ontologies/2021/6/objectPropertiesV1#p1hvalue>
                                                                                                                                                                                                                                      )
                                                                                                                                                                                         ] ;
                                                                                                                                                                               rdf:rest [ rdf:type <http://www.w3.org/2003/11/swrl#AtomList> ;
                                                                                                                                                                                          rdf:first [ rdf:type <http://www.w3.org/2003/11/swrl#BuiltinAtom> ;
                                                                                                                                                                                                      <http://www.w3.org/2003/11/swrl#builtin> <http://www.w3.org/2003/11/swrlb#lessThan> ;
                                                                                                                                                                                                      <http://www.w3.org/2003/11/swrl#arguments> [ rdf:type rdf:List ;
                                                                                                                                                                                                                                                   rdf:first <http://www.semanticweb.org/stevek/ontologies/2021/6/objectPropertiesV1#dirDiff> ;
                                                                                                                                                                                                                                                   rdf:rest [ rdf:type rdf:List ;
                                                                                                                                                                                                                                                              rdf:first -75 ;
                                                                                                                                                                                                                                                              rdf:rest rdf:nil
                                                                                                                                                                                                                                                            ]
                                                                                                                                                                                                                                                 ]
                                                                                                                                                                                                    ] ;
                                                                                                                                                                                          rdf:rest [ rdf:type <http://www.w3.org/2003/11/swrl#AtomList> ;
                                                                                                                                                                                                     rdf:first [ rdf:type <http://www.w3.org/2003/11/swrl#BuiltinAtom> ;
                                                                                                                                                                                                                 <http://www.w3.org/2003/11/swrl#builtin> <http://www.w3.org/2003/11/swrlb#greaterThan> ;
                                                                                                                                                                                                                 <http://www.w3.org/2003/11/swrl#arguments> [ rdf:type rdf:List ;
                                                                                                                                                                                                                                                              rdf:first <http://www.semanticweb.org/stevek/ontologies/2021/6/objectPropertiesV1#dirDiff> ;
                                                                                                                                                                                                                                                              rdf:rest [ rdf:type rdf:List ;
                                                                                                                                                                                                                                                                         rdf:first -105 ;
                                                                                                                                                                                                                                                                         rdf:rest rdf:nil
                                                                                                                                                                                                                                                                       ]
                                                                                                                                                                                                                                                            ]
                                                                                                                                                                                                               ] ;
                                                                                                                                                                                                     rdf:rest rdf:nil
                                                                                                                                                                                                   ]
                                                                                                                                                                                        ]
                                                                                                                                                                             ]
                                                                                                                                                                  ]
                                                                                                                                                       ]
                                                                                                                                            ]
                                                                                                                                 ]
                                                                                                                      ]
                                                                                                           ]
                                                                                                ]
                                                                                     ]
                                                                          ]
                                                               ]
                                                    ]
                                         ] ;
   <http://www.w3.org/2003/11/swrl#head> [ rdf:type <http://www.w3.org/2003/11/swrl#AtomList> ;
                                           rdf:first [ rdf:type <http://www.w3.org/2003/11/swrl#IndividualPropertyAtom> ;
                                                       <http://www.w3.org/2003/11/swrl#propertyPredicate> <http://ontology.asam.net/ontologies/Core#leftOf> ;
                                                       <http://www.w3.org/2003/11/swrl#argument1> <http://www.semanticweb.org/stevek/ontologies/2021/6/objectPropertiesV1#p2> ;
                                                       <http://www.w3.org/2003/11/swrl#argument2> <http://www.semanticweb.org/stevek/ontologies/2021/6/objectPropertiesV1#p1>
                                                     ] ;
                                           rdf:rest rdf:nil
                                         ]
 ] .

[ <http://swrl.stanford.edu/ontologies/3.3/swrla.owl#isRuleEnabled> "true"^^xsd:boolean ;
   rdfs:comment ""^^xsd:string ;
   rdfs:label "behind transitivity"^^xsd:string ;
   rdf:type <http://www.w3.org/2003/11/swrl#Imp> ;
   <http://www.w3.org/2003/11/swrl#body> [ rdf:type <http://www.w3.org/2003/11/swrl#AtomList> ;
                                           rdf:first [ rdf:type <http://www.w3.org/2003/11/swrl#IndividualPropertyAtom> ;
                                                       <http://www.w3.org/2003/11/swrl#propertyPredicate> <http://ontology.asam.net/ontologies/Core#behind> ;
                                                       <http://www.w3.org/2003/11/swrl#argument1> <http://www.semanticweb.org/stevek/ontologies/2021/6/objectPropertiesV1#x> ;
                                                       <http://www.w3.org/2003/11/swrl#argument2> <http://www.semanticweb.org/stevek/ontologies/2021/6/objectPropertiesV1#y>
                                                     ] ;
                                           rdf:rest [ rdf:type <http://www.w3.org/2003/11/swrl#AtomList> ;
                                                      rdf:first [ rdf:type <http://www.w3.org/2003/11/swrl#IndividualPropertyAtom> ;
                                                                  <http://www.w3.org/2003/11/swrl#propertyPredicate> <http://ontology.asam.net/ontologies/Core#behind> ;
                                                                  <http://www.w3.org/2003/11/swrl#argument1> <http://www.semanticweb.org/stevek/ontologies/2021/6/objectPropertiesV1#y> ;
                                                                  <http://www.w3.org/2003/11/swrl#argument2> <http://www.semanticweb.org/stevek/ontologies/2021/6/objectPropertiesV1#z>
                                                                ] ;
                                                      rdf:rest rdf:nil
                                                    ]
                                         ] ;
   <http://www.w3.org/2003/11/swrl#head> [ rdf:type <http://www.w3.org/2003/11/swrl#AtomList> ;
                                           rdf:first [ rdf:type <http://www.w3.org/2003/11/swrl#IndividualPropertyAtom> ;
                                                       <http://www.w3.org/2003/11/swrl#propertyPredicate> <http://ontology.asam.net/ontologies/Core#behind> ;
                                                       <http://www.w3.org/2003/11/swrl#argument1> <http://www.semanticweb.org/stevek/ontologies/2021/6/objectPropertiesV1#x> ;
                                                       <http://www.w3.org/2003/11/swrl#argument2> <http://www.semanticweb.org/stevek/ontologies/2021/6/objectPropertiesV1#z>
                                                     ] ;
                                           rdf:rest rdf:nil
                                         ]
 ] .

[ <http://swrl.stanford.edu/ontologies/3.3/swrla.owl#isRuleEnabled> "true"^^xsd:boolean ;
   rdfs:comment ""^^xsd:string ;
   rdfs:label "front of transitivity"^^xsd:string ;
   rdf:type <http://www.w3.org/2003/11/swrl#Imp> ;
   <http://www.w3.org/2003/11/swrl#body> [ rdf:type <http://www.w3.org/2003/11/swrl#AtomList> ;
                                           rdf:first [ rdf:type <http://www.w3.org/2003/11/swrl#IndividualPropertyAtom> ;
                                                       <http://www.w3.org/2003/11/swrl#propertyPredicate> <http://ontology.asam.net/ontologies/Core#inFrontOf> ;
                                                       <http://www.w3.org/2003/11/swrl#argument1> <http://www.semanticweb.org/stevek/ontologies/2021/6/objectPropertiesV1#x> ;
                                                       <http://www.w3.org/2003/11/swrl#argument2> <http://www.semanticweb.org/stevek/ontologies/2021/6/objectPropertiesV1#y>
                                                     ] ;
                                           rdf:rest [ rdf:type <http://www.w3.org/2003/11/swrl#AtomList> ;
                                                      rdf:first [ rdf:type <http://www.w3.org/2003/11/swrl#IndividualPropertyAtom> ;
                                                                  <http://www.w3.org/2003/11/swrl#propertyPredicate> <http://ontology.asam.net/ontologies/Core#inFrontOf> ;
                                                                  <http://www.w3.org/2003/11/swrl#argument1> <http://www.semanticweb.org/stevek/ontologies/2021/6/objectPropertiesV1#y> ;
                                                                  <http://www.w3.org/2003/11/swrl#argument2> <http://www.semanticweb.org/stevek/ontologies/2021/6/objectPropertiesV1#z>
                                                                ] ;
                                                      rdf:rest rdf:nil
                                                    ]
                                         ] ;
   <http://www.w3.org/2003/11/swrl#head> [ rdf:type <http://www.w3.org/2003/11/swrl#AtomList> ;
                                           rdf:first [ rdf:type <http://www.w3.org/2003/11/swrl#IndividualPropertyAtom> ;
                                                       <http://www.w3.org/2003/11/swrl#propertyPredicate> <http://ontology.asam.net/ontologies/Core#inFrontOf> ;
                                                       <http://www.w3.org/2003/11/swrl#argument1> <http://www.semanticweb.org/stevek/ontologies/2021/6/objectPropertiesV1#x> ;
                                                       <http://www.w3.org/2003/11/swrl#argument2> <http://www.semanticweb.org/stevek/ontologies/2021/6/objectPropertiesV1#z>
                                                     ] ;
                                           rdf:rest rdf:nil
                                         ]
 ] .

[ <http://swrl.stanford.edu/ontologies/3.3/swrla.owl#isRuleEnabled> "true"^^xsd:boolean ;
   rdfs:comment ""^^xsd:string ;
   rdfs:label "left of transitivity"^^xsd:string ;
   rdf:type <http://www.w3.org/2003/11/swrl#Imp> ;
   <http://www.w3.org/2003/11/swrl#body> [ rdf:type <http://www.w3.org/2003/11/swrl#AtomList> ;
                                           rdf:first [ rdf:type <http://www.w3.org/2003/11/swrl#IndividualPropertyAtom> ;
                                                       <http://www.w3.org/2003/11/swrl#propertyPredicate> <http://ontology.asam.net/ontologies/Core#leftOf> ;
                                                       <http://www.w3.org/2003/11/swrl#argument1> <http://www.semanticweb.org/stevek/ontologies/2021/6/objectPropertiesV1#x> ;
                                                       <http://www.w3.org/2003/11/swrl#argument2> <http://www.semanticweb.org/stevek/ontologies/2021/6/objectPropertiesV1#y>
                                                     ] ;
                                           rdf:rest [ rdf:type <http://www.w3.org/2003/11/swrl#AtomList> ;
                                                      rdf:first [ rdf:type <http://www.w3.org/2003/11/swrl#IndividualPropertyAtom> ;
                                                                  <http://www.w3.org/2003/11/swrl#propertyPredicate> <http://ontology.asam.net/ontologies/Core#leftOf> ;
                                                                  <http://www.w3.org/2003/11/swrl#argument1> <http://www.semanticweb.org/stevek/ontologies/2021/6/objectPropertiesV1#y> ;
                                                                  <http://www.w3.org/2003/11/swrl#argument2> <http://www.semanticweb.org/stevek/ontologies/2021/6/objectPropertiesV1#z>
                                                                ] ;
                                                      rdf:rest rdf:nil
                                                    ]
                                         ] ;
   <http://www.w3.org/2003/11/swrl#head> [ rdf:type <http://www.w3.org/2003/11/swrl#AtomList> ;
                                           rdf:first [ rdf:type <http://www.w3.org/2003/11/swrl#IndividualPropertyAtom> ;
                                                       <http://www.w3.org/2003/11/swrl#propertyPredicate> <http://ontology.asam.net/ontologies/Core#leftOf> ;
                                                       <http://www.w3.org/2003/11/swrl#argument1> <http://www.semanticweb.org/stevek/ontologies/2021/6/objectPropertiesV1#x> ;
                                                       <http://www.w3.org/2003/11/swrl#argument2> <http://www.semanticweb.org/stevek/ontologies/2021/6/objectPropertiesV1#z>
                                                     ] ;
                                           rdf:rest rdf:nil
                                         ]
 ] .

[ <http://swrl.stanford.edu/ontologies/3.3/swrla.owl#isRuleEnabled> "true"^^xsd:boolean ;
   rdfs:comment ""^^xsd:string ;
   rdfs:label "occurs after transitivity"^^xsd:string ;
   rdf:type <http://www.w3.org/2003/11/swrl#Imp> ;
   <http://www.w3.org/2003/11/swrl#body> [ rdf:type <http://www.w3.org/2003/11/swrl#AtomList> ;
                                           rdf:first [ rdf:type <http://www.w3.org/2003/11/swrl#IndividualPropertyAtom> ;
                                                       <http://www.w3.org/2003/11/swrl#propertyPredicate> <http://ontology.asam.net/ontologies/Core#occursAfter> ;
                                                       <http://www.w3.org/2003/11/swrl#argument1> <http://www.semanticweb.org/stevek/ontologies/2021/6/objectPropertiesV1#x> ;
                                                       <http://www.w3.org/2003/11/swrl#argument2> <http://www.semanticweb.org/stevek/ontologies/2021/6/objectPropertiesV1#y>
                                                     ] ;
                                           rdf:rest [ rdf:type <http://www.w3.org/2003/11/swrl#AtomList> ;
                                                      rdf:first [ rdf:type <http://www.w3.org/2003/11/swrl#IndividualPropertyAtom> ;
                                                                  <http://www.w3.org/2003/11/swrl#propertyPredicate> <http://ontology.asam.net/ontologies/Core#occursAfter> ;
                                                                  <http://www.w3.org/2003/11/swrl#argument1> <http://www.semanticweb.org/stevek/ontologies/2021/6/objectPropertiesV1#y> ;
                                                                  <http://www.w3.org/2003/11/swrl#argument2> <http://www.semanticweb.org/stevek/ontologies/2021/6/objectPropertiesV1#z>
                                                                ] ;
                                                      rdf:rest rdf:nil
                                                    ]
                                         ] ;
   <http://www.w3.org/2003/11/swrl#head> [ rdf:type <http://www.w3.org/2003/11/swrl#AtomList> ;
                                           rdf:first [ rdf:type <http://www.w3.org/2003/11/swrl#IndividualPropertyAtom> ;
                                                       <http://www.w3.org/2003/11/swrl#propertyPredicate> <http://ontology.asam.net/ontologies/Core#occursAfter> ;
                                                       <http://www.w3.org/2003/11/swrl#argument1> <http://www.semanticweb.org/stevek/ontologies/2021/6/objectPropertiesV1#x> ;
                                                       <http://www.w3.org/2003/11/swrl#argument2> <http://www.semanticweb.org/stevek/ontologies/2021/6/objectPropertiesV1#z>
                                                     ] ;
                                           rdf:rest rdf:nil
                                         ]
 ] .

[ <http://swrl.stanford.edu/ontologies/3.3/swrla.owl#isRuleEnabled> "true"^^xsd:boolean ;
   rdfs:comment ""^^xsd:string ;
   rdfs:label "occurs before transitivity"^^xsd:string ;
   rdf:type <http://www.w3.org/2003/11/swrl#Imp> ;
   <http://www.w3.org/2003/11/swrl#body> [ rdf:type <http://www.w3.org/2003/11/swrl#AtomList> ;
                                           rdf:first [ rdf:type <http://www.w3.org/2003/11/swrl#IndividualPropertyAtom> ;
                                                       <http://www.w3.org/2003/11/swrl#propertyPredicate> <http://ontology.asam.net/ontologies/Core#occursBefore> ;
                                                       <http://www.w3.org/2003/11/swrl#argument1> <http://www.semanticweb.org/stevek/ontologies/2021/6/objectPropertiesV1#x> ;
                                                       <http://www.w3.org/2003/11/swrl#argument2> <http://www.semanticweb.org/stevek/ontologies/2021/6/objectPropertiesV1#y>
                                                     ] ;
                                           rdf:rest [ rdf:type <http://www.w3.org/2003/11/swrl#AtomList> ;
                                                      rdf:first [ rdf:type <http://www.w3.org/2003/11/swrl#IndividualPropertyAtom> ;
                                                                  <http://www.w3.org/2003/11/swrl#propertyPredicate> <http://ontology.asam.net/ontologies/Core#occursBefore> ;
                                                                  <http://www.w3.org/2003/11/swrl#argument1> <http://www.semanticweb.org/stevek/ontologies/2021/6/objectPropertiesV1#y> ;
                                                                  <http://www.w3.org/2003/11/swrl#argument2> <http://www.semanticweb.org/stevek/ontologies/2021/6/objectPropertiesV1#z>
                                                                ] ;
                                                      rdf:rest rdf:nil
                                                    ]
                                         ] ;
   <http://www.w3.org/2003/11/swrl#head> [ rdf:type <http://www.w3.org/2003/11/swrl#AtomList> ;
                                           rdf:first [ rdf:type <http://www.w3.org/2003/11/swrl#IndividualPropertyAtom> ;
                                                       <http://www.w3.org/2003/11/swrl#propertyPredicate> <http://ontology.asam.net/ontologies/Core#occursBefore> ;
                                                       <http://www.w3.org/2003/11/swrl#argument1> <http://www.semanticweb.org/stevek/ontologies/2021/6/objectPropertiesV1#x> ;
                                                       <http://www.w3.org/2003/11/swrl#argument2> <http://www.semanticweb.org/stevek/ontologies/2021/6/objectPropertiesV1#z>
                                                     ] ;
                                           rdf:rest rdf:nil
                                         ]
 ] .

[ <http://swrl.stanford.edu/ontologies/3.3/swrla.owl#isRuleEnabled> "true"^^xsd:boolean ;
   rdfs:comment ""^^xsd:string ;
   rdfs:label "right of transitivity"^^xsd:string ;
   rdf:type <http://www.w3.org/2003/11/swrl#Imp> ;
   <http://www.w3.org/2003/11/swrl#body> [ rdf:type <http://www.w3.org/2003/11/swrl#AtomList> ;
                                           rdf:first [ rdf:type <http://www.w3.org/2003/11/swrl#IndividualPropertyAtom> ;
                                                       <http://www.w3.org/2003/11/swrl#propertyPredicate> <http://ontology.asam.net/ontologies/Core#rightOf> ;
                                                       <http://www.w3.org/2003/11/swrl#argument1> <http://www.semanticweb.org/stevek/ontologies/2021/6/objectPropertiesV1#x> ;
                                                       <http://www.w3.org/2003/11/swrl#argument2> <http://www.semanticweb.org/stevek/ontologies/2021/6/objectPropertiesV1#y>
                                                     ] ;
                                           rdf:rest [ rdf:type <http://www.w3.org/2003/11/swrl#AtomList> ;
                                                      rdf:first [ rdf:type <http://www.w3.org/2003/11/swrl#IndividualPropertyAtom> ;
                                                                  <http://www.w3.org/2003/11/swrl#propertyPredicate> <http://ontology.asam.net/ontologies/Core#rightOf> ;
                                                                  <http://www.w3.org/2003/11/swrl#argument1> <http://www.semanticweb.org/stevek/ontologies/2021/6/objectPropertiesV1#y> ;
                                                                  <http://www.w3.org/2003/11/swrl#argument2> <http://www.semanticweb.org/stevek/ontologies/2021/6/objectPropertiesV1#z>
                                                                ] ;
                                                      rdf:rest rdf:nil
                                                    ]
                                         ] ;
   <http://www.w3.org/2003/11/swrl#head> [ rdf:type <http://www.w3.org/2003/11/swrl#AtomList> ;
                                           rdf:first [ rdf:type <http://www.w3.org/2003/11/swrl#IndividualPropertyAtom> ;
                                                       <http://www.w3.org/2003/11/swrl#propertyPredicate> <http://ontology.asam.net/ontologies/Core#rightOf> ;
                                                       <http://www.w3.org/2003/11/swrl#argument1> <http://www.semanticweb.org/stevek/ontologies/2021/6/objectPropertiesV1#x> ;
                                                       <http://www.w3.org/2003/11/swrl#argument2> <http://www.semanticweb.org/stevek/ontologies/2021/6/objectPropertiesV1#z>
                                                     ] ;
                                           rdf:rest rdf:nil
                                         ]
 ] .

[ <http://swrl.stanford.edu/ontologies/3.3/swrla.owl#isRuleEnabled> "true"^^xsd:boolean ;
   rdfs:comment ""^^xsd:string ;
   rdfs:label "new in front of"^^xsd:string ;
   rdf:type <http://www.w3.org/2003/11/swrl#Imp> ;
   <http://www.w3.org/2003/11/swrl#body> [ rdf:type <http://www.w3.org/2003/11/swrl#AtomList> ;
                                           rdf:first [ rdf:type <http://www.w3.org/2003/11/swrl#ClassAtom> ;
                                                       <http://www.w3.org/2003/11/swrl#classPredicate> <http://ontology.asam.net/ontologies/Core#PhysicalObjectState> ;
                                                       <http://www.w3.org/2003/11/swrl#argument1> <http://www.semanticweb.org/stevek/ontologies/2021/6/objectPropertiesV1#p1>
                                                     ] ;
                                           rdf:rest [ rdf:type <http://www.w3.org/2003/11/swrl#AtomList> ;
                                                      rdf:first [ rdf:type <http://www.w3.org/2003/11/swrl#ClassAtom> ;
                                                                  <http://www.w3.org/2003/11/swrl#classPredicate> <http://ontology.asam.net/ontologies/Core#PhysicalObjectState> ;
                                                                  <http://www.w3.org/2003/11/swrl#argument1> <http://www.semanticweb.org/stevek/ontologies/2021/6/objectPropertiesV1#p2>
                                                                ] ;
                                                      rdf:rest [ rdf:type <http://www.w3.org/2003/11/swrl#AtomList> ;
                                                                 rdf:first [ rdf:type <http://www.w3.org/2003/11/swrl#ClassAtom> ;
                                                                             <http://www.w3.org/2003/11/swrl#classPredicate> <http://ontology.asam.net/ontologies/Core#DirectionQuantity> ;
                                                                             <http://www.w3.org/2003/11/swrl#argument1> <http://www.semanticweb.org/stevek/ontologies/2021/6/objectPropertiesV1#p1h>
                                                                           ] ;
                                                                 rdf:rest [ rdf:type <http://www.w3.org/2003/11/swrl#AtomList> ;
                                                                            rdf:first [ rdf:type <http://www.w3.org/2003/11/swrl#IndividualPropertyAtom> ;
                                                                                        <http://www.w3.org/2003/11/swrl#propertyPredicate> <http://ontology.asam.net/ontologies/Core#hasHeading> ;
                                                                                        <http://www.w3.org/2003/11/swrl#argument1> <http://www.semanticweb.org/stevek/ontologies/2021/6/objectPropertiesV1#p1> ;
                                                                                        <http://www.w3.org/2003/11/swrl#argument2> <http://www.semanticweb.org/stevek/ontologies/2021/6/objectPropertiesV1#p1h>
                                                                                      ] ;
                                                                            rdf:rest [ rdf:type <http://www.w3.org/2003/11/swrl#AtomList> ;
                                                                                       rdf:first [ rdf:type <http://www.w3.org/2003/11/swrl#ClassAtom> ;
                                                                                                   <http://www.w3.org/2003/11/swrl#classPredicate> <http://ontology.asam.net/ontologies/Core#SpatialRelation> ;
                                                                                                   <http://www.w3.org/2003/11/swrl#argument1> <http://www.semanticweb.org/stevek/ontologies/2021/6/objectPropertiesV1#r>
                                                                                                 ] ;
                                                                                       rdf:rest [ rdf:type <http://www.w3.org/2003/11/swrl#AtomList> ;
                                                                                                  rdf:first [ rdf:type <http://www.w3.org/2003/11/swrl#IndividualPropertyAtom> ;
                                                                                                              <http://www.w3.org/2003/11/swrl#propertyPredicate> <http://ontology.asam.net/ontologies/Core#hasSpatialSubject> ;
                                                                                                              <http://www.w3.org/2003/11/swrl#argument1> <http://www.semanticweb.org/stevek/ontologies/2021/6/objectPropertiesV1#r> ;
                                                                                                              <http://www.w3.org/2003/11/swrl#argument2> <http://www.semanticweb.org/stevek/ontologies/2021/6/objectPropertiesV1#p1>
                                                                                                            ] ;
                                                                                                  rdf:rest [ rdf:type <http://www.w3.org/2003/11/swrl#AtomList> ;
                                                                                                             rdf:first [ rdf:type <http://www.w3.org/2003/11/swrl#IndividualPropertyAtom> ;
                                                                                                                         <http://www.w3.org/2003/11/swrl#propertyPredicate> <http://ontology.asam.net/ontologies/Core#hasSpatialObject> ;
                                                                                                                         <http://www.w3.org/2003/11/swrl#argument1> <http://www.semanticweb.org/stevek/ontologies/2021/6/objectPropertiesV1#r> ;
                                                                                                                         <http://www.w3.org/2003/11/swrl#argument2> <http://www.semanticweb.org/stevek/ontologies/2021/6/objectPropertiesV1#p2>
                                                                                                                       ] ;
                                                                                                             rdf:rest [ rdf:type <http://www.w3.org/2003/11/swrl#AtomList> ;
                                                                                                                        rdf:first [ rdf:type <http://www.w3.org/2003/11/swrl#ClassAtom> ;
                                                                                                                                    <http://www.w3.org/2003/11/swrl#classPredicate> <http://ontology.asam.net/ontologies/Core#DirectionQuantity> ;
                                                                                                                                    <http://www.w3.org/2003/11/swrl#argument1> <http://www.semanticweb.org/stevek/ontologies/2021/6/objectPropertiesV1#rdir1>
                                                                                                                                  ] ;
                                                                                                                        rdf:rest [ rdf:type <http://www.w3.org/2003/11/swrl#AtomList> ;
                                                                                                                                   rdf:first [ rdf:type <http://www.w3.org/2003/11/swrl#ClassAtom> ;
                                                                                                                                               <http://www.w3.org/2003/11/swrl#classPredicate> <http://ontology.asam.net/ontologies/Core#DirectionQuantity> ;
                                                                                                                                               <http://www.w3.org/2003/11/swrl#argument1> <http://www.semanticweb.org/stevek/ontologies/2021/6/objectPropertiesV1#rdir2>
                                                                                                                                             ] ;
                                                                                                                                   rdf:rest [ rdf:type <http://www.w3.org/2003/11/swrl#AtomList> ;
                                                                                                                                              rdf:first [ rdf:type <http://www.w3.org/2003/11/swrl#IndividualPropertyAtom> ;
                                                                                                                                                          <http://www.w3.org/2003/11/swrl#propertyPredicate> <http://ontology.asam.net/ontologies/Core#hasRelationDirection> ;
                                                                                                                                                          <http://www.w3.org/2003/11/swrl#argument1> <http://www.semanticweb.org/stevek/ontologies/2021/6/objectPropertiesV1#r> ;
                                                                                                                                                          <http://www.w3.org/2003/11/swrl#argument2> <http://www.semanticweb.org/stevek/ontologies/2021/6/objectPropertiesV1#rdir1>
                                                                                                                                                        ] ;
                                                                                                                                              rdf:rest [ rdf:type <http://www.w3.org/2003/11/swrl#AtomList> ;
                                                                                                                                                         rdf:first [ rdf:type <http://www.w3.org/2003/11/swrl#DatavaluedPropertyAtom> ;
                                                                                                                                                                     <http://www.w3.org/2003/11/swrl#propertyPredicate> <http://ontology.asam.net/ontologies/Core#hasValue> ;
                                                                                                                                                                     <http://www.w3.org/2003/11/swrl#argument1> <http://www.semanticweb.org/stevek/ontologies/2021/6/objectPropertiesV1#p1h> ;
                                                                                                                                                                     <http://www.w3.org/2003/11/swrl#argument2> <http://www.semanticweb.org/stevek/ontologies/2021/6/objectPropertiesV1#p1hvalue>
                                                                                                                                                                   ] ;
                                                                                                                                                         rdf:rest [ rdf:type <http://www.w3.org/2003/11/swrl#AtomList> ;
                                                                                                                                                                    rdf:first [ rdf:type <http://www.w3.org/2003/11/swrl#DatavaluedPropertyAtom> ;
                                                                                                                                                                                <http://www.w3.org/2003/11/swrl#propertyPredicate> <http://ontology.asam.net/ontologies/Core#hasValue> ;
                                                                                                                                                                                <http://www.w3.org/2003/11/swrl#argument1> <http://www.semanticweb.org/stevek/ontologies/2021/6/objectPropertiesV1#rdir1> ;
                                                                                                                                                                                <http://www.w3.org/2003/11/swrl#argument2> <http://www.semanticweb.org/stevek/ontologies/2021/6/objectPropertiesV1#rdir1value>
                                                                                                                                                                              ] ;
                                                                                                                                                                    rdf:rest [ rdf:type <http://www.w3.org/2003/11/swrl#AtomList> ;
                                                                                                                                                                               rdf:first [ rdf:type <http://www.w3.org/2003/11/swrl#BuiltinAtom> ;
                                                                                                                                                                                           <http://www.w3.org/2003/11/swrl#builtin> <http://www.w3.org/2003/11/swrlb#subtract> ;
                                                                                                                                                                                           <http://www.w3.org/2003/11/swrl#arguments> ( <http://www.semanticweb.org/stevek/ontologies/2021/6/objectPropertiesV1#dirDiff>
                                                                                                                                                                                                                                        <http://www.semanticweb.org/stevek/ontologies/2021/6/objectPropertiesV1#rdir1value>
                                                                                                                                                                                                                                        <http://www.semanticweb.org/stevek/ontologies/2021/6/objectPropertiesV1#p1hvalue>
                                                                                                                                                                                                                                      )
                                                                                                                                                                                         ] ;
                                                                                                                                                                               rdf:rest [ rdf:type <http://www.w3.org/2003/11/swrl#AtomList> ;
                                                                                                                                                                                          rdf:first [ rdf:type <http://www.w3.org/2003/11/swrl#BuiltinAtom> ;
                                                                                                                                                                                                      <http://www.w3.org/2003/11/swrl#builtin> <http://www.w3.org/2003/11/swrlb#lessThan> ;
                                                                                                                                                                                                      <http://www.w3.org/2003/11/swrl#arguments> [ rdf:type rdf:List ;
                                                                                                                                                                                                                                                   rdf:first <http://www.semanticweb.org/stevek/ontologies/2021/6/objectPropertiesV1#dirDiff> ;
                                                                                                                                                                                                                                                   rdf:rest [ rdf:type rdf:List ;
                                                                                                                                                                                                                                                              rdf:first 15 ;
                                                                                                                                                                                                                                                              rdf:rest rdf:nil
                                                                                                                                                                                                                                                            ]
                                                                                                                                                                                                                                                 ]
                                                                                                                                                                                                    ] ;
                                                                                                                                                                                          rdf:rest [ rdf:type <http://www.w3.org/2003/11/swrl#AtomList> ;
                                                                                                                                                                                                     rdf:first [ rdf:type <http://www.w3.org/2003/11/swrl#BuiltinAtom> ;
                                                                                                                                                                                                                 <http://www.w3.org/2003/11/swrl#builtin> <http://www.w3.org/2003/11/swrlb#greaterThan> ;
                                                                                                                                                                                                                 <http://www.w3.org/2003/11/swrl#arguments> [ rdf:type rdf:List ;
                                                                                                                                                                                                                                                              rdf:first <http://www.semanticweb.org/stevek/ontologies/2021/6/objectPropertiesV1#dirDiff> ;
                                                                                                                                                                                                                                                              rdf:rest [ rdf:type rdf:List ;
                                                                                                                                                                                                                                                                         rdf:first -15 ;
                                                                                                                                                                                                                                                                         rdf:rest rdf:nil
                                                                                                                                                                                                                                                                       ]
                                                                                                                                                                                                                                                            ]
                                                                                                                                                                                                               ] ;
                                                                                                                                                                                                     rdf:rest rdf:nil
                                                                                                                                                                                                   ]
                                                                                                                                                                                        ]
                                                                                                                                                                             ]
                                                                                                                                                                  ]
                                                                                                                                                       ]
                                                                                                                                            ]
                                                                                                                                 ]
                                                                                                                      ]
                                                                                                           ]
                                                                                                ]
                                                                                     ]
                                                                          ]
                                                               ]
                                                    ]
                                         ] ;
   <http://www.w3.org/2003/11/swrl#head> [ rdf:type <http://www.w3.org/2003/11/swrl#AtomList> ;
                                           rdf:first [ rdf:type <http://www.w3.org/2003/11/swrl#IndividualPropertyAtom> ;
                                                       <http://www.w3.org/2003/11/swrl#propertyPredicate> <http://ontology.asam.net/ontologies/Core#inFrontOf> ;
                                                       <http://www.w3.org/2003/11/swrl#argument1> <http://www.semanticweb.org/stevek/ontologies/2021/6/objectPropertiesV1#p2> ;
                                                       <http://www.w3.org/2003/11/swrl#argument2> <http://www.semanticweb.org/stevek/ontologies/2021/6/objectPropertiesV1#p1>
                                                     ] ;
                                           rdf:rest rdf:nil
                                         ]
 ] .

###  Generated by the OWL API (version 4.5.9.2019-02-01T07:24:44Z) https://github.com/owlcs/owlapi
